<?xml version="1.0" encoding="UTF-8"?>
<rdf:RDF xmlns:dct="http://purl.org/dc/terms/" xmlns:owl="http://www.w3.org/2002/07/owl#" xmlns:rdf="http://www.w3.org/1999/02/22-rdf-syntax-ns#" xmlns:rdfs="http://www.w3.org/2000/01/rdf-schema#" xmlns:skos="http://www.w3.org/2004/02/skos/core#" xml:base="http://www.earthobservations.org/GEOSS/EO_Vocabulary/" xml:lang="en">
	<skos:ConceptScheme rdf:about="http://www.earthobservations.org/GEOSS/EO_Vocabulary">
		<skos:prefLabel xml:lang="en">GEOSS - Earth Observation Vocabulary, version 1.0</skos:prefLabel>
		<dct:title>GEOSS - Earth Observation Vocabulary, version 1.0</dct:title>
		<dct:issued>2011-05-01</dct:issued>
		<skos:hasTopConcept rdf:resource="http://www.earthobservations.org/GEOSS/EO_Vocabulary/atmosphere"/>
		<skos:hasTopConcept rdf:resource="http://www.earthobservations.org/GEOSS/EO_Vocabulary/agriculture"/>
		<skos:hasTopConcept rdf:resource="http://www.earthobservations.org/GEOSS/EO_Vocabulary/land%20surface"/>
		<skos:hasTopConcept rdf:resource="http://www.earthobservations.org/GEOSS/EO_Vocabulary/oceans"/>
		<skos:hasTopConcept rdf:resource="http://www.earthobservations.org/GEOSS/EO_Vocabulary/human%20dimensions"/>
		<skos:hasTopConcept rdf:resource="http://www.earthobservations.org/GEOSS/EO_Vocabulary/biosphere"/>
		<skos:hasTopConcept rdf:resource="http://www.earthobservations.org/GEOSS/EO_Vocabulary/terrestrial%20hydrosphere"/>
		<skos:hasTopConcept rdf:resource="http://www.earthobservations.org/GEOSS/EO_Vocabulary/cryosphere"/>
		<skos:hasTopConcept rdf:resource="http://www.earthobservations.org/GEOSS/EO_Vocabulary/paleoclimate"/>
		<skos:hasTopConcept rdf:resource="http://www.earthobservations.org/GEOSS/EO_Vocabulary/solid%20earth"/>
		<skos:hasTopConcept rdf:resource="http://www.earthobservations.org/GEOSS/EO_Vocabulary/biological%20classification"/>
	</skos:ConceptScheme>
	<skos:Concept rdf:about="http://www.earthobservations.org/GEOSS/EO_Vocabulary/atmosphere">
		<skos:prefLabel>ATMOSPHERE</skos:prefLabel>
		<skos:narrower rdf:resource="http://www.earthobservations.org/GEOSS/EO_Vocabulary/atmospheric%20temperature"/>
		<skos:narrower rdf:resource="http://www.earthobservations.org/GEOSS/EO_Vocabulary/atmospheric%20winds"/>
		<skos:narrower rdf:resource="http://www.earthobservations.org/GEOSS/EO_Vocabulary/atmospheric%20water%20vapor"/>
		<skos:narrower rdf:resource="http://www.earthobservations.org/GEOSS/EO_Vocabulary/atmospheric%20pressure"/>
		<skos:narrower rdf:resource="http://www.earthobservations.org/GEOSS/EO_Vocabulary/aerosols"/>
		<skos:narrower rdf:resource="http://www.earthobservations.org/GEOSS/EO_Vocabulary/atmospheric%20radiation"/>
		<skos:narrower rdf:resource="http://www.earthobservations.org/GEOSS/EO_Vocabulary/clouds"/>
		<skos:narrower rdf:resource="http://www.earthobservations.org/GEOSS/EO_Vocabulary/atmospheric%20chemistry"/>
		<skos:narrower rdf:resource="http://www.earthobservations.org/GEOSS/EO_Vocabulary/air%20quality"/>
		<skos:inScheme rdf:resource="http://www.earthobservations.org/GEOSS/EO_Vocabulary"/>
	</skos:Concept>
	<skos:Concept rdf:about="http://www.earthobservations.org/GEOSS/EO_Vocabulary/agriculture">
		<skos:prefLabel>AGRICULTURE</skos:prefLabel>
		<skos:narrower rdf:resource="http://www.earthobservations.org/GEOSS/EO_Vocabulary/soils"/>
		<skos:narrower rdf:resource="http://www.earthobservations.org/GEOSS/EO_Vocabulary/agricultural%20engineering"/>
		<skos:narrower rdf:resource="http://www.earthobservations.org/GEOSS/EO_Vocabulary/agricultural%20plant%20science"/>
		<skos:narrower rdf:resource="http://www.earthobservations.org/GEOSS/EO_Vocabulary/forest%20science"/>
		<skos:narrower rdf:resource="http://www.earthobservations.org/GEOSS/EO_Vocabulary/animal%20science"/>
		<skos:narrower rdf:resource="http://www.earthobservations.org/GEOSS/EO_Vocabulary/agricultural%20aquatic%20sciences"/>
		<skos:narrower rdf:resource="http://www.earthobservations.org/GEOSS/EO_Vocabulary/plant%20commodities"/>
		<skos:inScheme rdf:resource="http://www.earthobservations.org/GEOSS/EO_Vocabulary"/>
	</skos:Concept>
	<skos:Concept rdf:about="http://www.earthobservations.org/GEOSS/EO_Vocabulary/land%20surface">
		<skos:prefLabel>LAND SURFACE</skos:prefLabel>
		<skos:narrower rdf:resource="http://www.earthobservations.org/GEOSS/EO_Vocabulary/soils"/>
		<skos:narrower rdf:resource="http://www.earthobservations.org/GEOSS/EO_Vocabulary/land%20use%2Fland%20cover"/>
		<skos:narrower rdf:resource="http://www.earthobservations.org/GEOSS/EO_Vocabulary/land%20temperature"/>
		<skos:narrower rdf:resource="http://www.earthobservations.org/GEOSS/EO_Vocabulary/frozen%20ground"/>
		<skos:narrower rdf:resource="http://www.earthobservations.org/GEOSS/EO_Vocabulary/topography"/>
		<skos:narrower rdf:resource="http://www.earthobservations.org/GEOSS/EO_Vocabulary/surface%20radiative%20properties"/>
		<skos:narrower rdf:resource="http://www.earthobservations.org/GEOSS/EO_Vocabulary/erosion%2Fsedimentation"/>
		<skos:narrower rdf:resource="http://www.earthobservations.org/GEOSS/EO_Vocabulary/geomorphology"/>
		<skos:inScheme rdf:resource="http://www.earthobservations.org/GEOSS/EO_Vocabulary"/>
	</skos:Concept>
	<skos:Concept rdf:about="http://www.earthobservations.org/GEOSS/EO_Vocabulary/oceans">
		<skos:prefLabel>OCEANS</skos:prefLabel>
		<skos:narrower rdf:resource="http://www.earthobservations.org/GEOSS/EO_Vocabulary/ocean%20winds"/>
		<skos:narrower rdf:resource="http://www.earthobservations.org/GEOSS/EO_Vocabulary/ocean%20temperature"/>
		<skos:narrower rdf:resource="http://www.earthobservations.org/GEOSS/EO_Vocabulary/sea%20ice"/>
		<skos:narrower rdf:resource="http://www.earthobservations.org/GEOSS/EO_Vocabulary/coastal%20processes"/>
		<skos:narrower rdf:resource="http://www.earthobservations.org/GEOSS/EO_Vocabulary/bathymetry%2Fseafloor%20topography"/>
		<skos:narrower rdf:resource="http://www.earthobservations.org/GEOSS/EO_Vocabulary/ocean%20heat%20budget"/>
		<skos:narrower rdf:resource="http://www.earthobservations.org/GEOSS/EO_Vocabulary/ocean%20optics"/>
		<skos:narrower rdf:resource="http://www.earthobservations.org/GEOSS/EO_Vocabulary/water%20quality"/>
		<skos:narrower rdf:resource="http://www.earthobservations.org/GEOSS/EO_Vocabulary/ocean%20chemistry"/>
		<skos:narrower rdf:resource="http://www.earthobservations.org/GEOSS/EO_Vocabulary/salinity%2Fdensity"/>
		<skos:narrower rdf:resource="http://www.earthobservations.org/GEOSS/EO_Vocabulary/ocean%20circulation"/>
		<skos:narrower rdf:resource="http://www.earthobservations.org/GEOSS/EO_Vocabulary/sea%20surface%20topography"/>
		<skos:narrower rdf:resource="http://www.earthobservations.org/GEOSS/EO_Vocabulary/marine%20sediments"/>
		<skos:narrower rdf:resource="http://www.earthobservations.org/GEOSS/EO_Vocabulary/ocean%20waves"/>
		<skos:narrower rdf:resource="http://www.earthobservations.org/GEOSS/EO_Vocabulary/aquatic%20sciences"/>
		<skos:narrower rdf:resource="http://www.earthobservations.org/GEOSS/EO_Vocabulary/marine%20geophysics"/>
		<skos:inScheme rdf:resource="http://www.earthobservations.org/GEOSS/EO_Vocabulary"/>
	</skos:Concept>
	<skos:Concept rdf:about="http://www.earthobservations.org/GEOSS/EO_Vocabulary/human%20dimensions">
		<skos:prefLabel>HUMAN DIMENSIONS</skos:prefLabel>
		<skos:narrower rdf:resource="http://www.earthobservations.org/GEOSS/EO_Vocabulary/land%20use%2Fland%20cover"/>
		<skos:narrower rdf:resource="http://www.earthobservations.org/GEOSS/EO_Vocabulary/environmental%20impacts"/>
		<skos:narrower rdf:resource="http://www.earthobservations.org/GEOSS/EO_Vocabulary/habitat%20conversion%2Ffragmentation"/>
		<skos:narrower rdf:resource="http://www.earthobservations.org/GEOSS/EO_Vocabulary/natural%20hazards"/>
		<skos:narrower rdf:resource="http://www.earthobservations.org/GEOSS/EO_Vocabulary/boundaries"/>
		<skos:narrower rdf:resource="http://www.earthobservations.org/GEOSS/EO_Vocabulary/human%20health"/>
		<skos:narrower rdf:resource="http://www.earthobservations.org/GEOSS/EO_Vocabulary/land%20use%2Fland%C2%A0cover"/>
		<skos:narrower rdf:resource="http://www.earthobservations.org/GEOSS/EO_Vocabulary/attitudes%2Cpreferences%2Cbehavior"/>
		<skos:inScheme rdf:resource="http://www.earthobservations.org/GEOSS/EO_Vocabulary"/>
	</skos:Concept>
	<skos:Concept rdf:about="http://www.earthobservations.org/GEOSS/EO_Vocabulary/biosphere">
		<skos:prefLabel>BIOSPHERE</skos:prefLabel>
		<skos:narrower rdf:resource="http://www.earthobservations.org/GEOSS/EO_Vocabulary/vegetation"/>
		<skos:narrower rdf:resource="http://www.earthobservations.org/GEOSS/EO_Vocabulary/ecological%20dynamics"/>
		<skos:narrower rdf:resource="http://www.earthobservations.org/GEOSS/EO_Vocabulary/terrestrial%20ecosystems"/>
		<skos:narrower rdf:resource="http://www.earthobservations.org/GEOSS/EO_Vocabulary/ecological%20dynamics"/>
		<skos:narrower rdf:resource="http://www.earthobservations.org/GEOSS/EO_Vocabulary/aquatic%20ecosystems"/>
		<skos:narrower rdf:resource="http://www.earthobservations.org/GEOSS/EO_Vocabulary/fungi"/>
		<skos:narrower rdf:resource="http://www.earthobservations.org/GEOSS/EO_Vocabulary/aquatic%20ecosystems"/>
		<skos:inScheme rdf:resource="http://www.earthobservations.org/GEOSS/EO_Vocabulary"/>
	</skos:Concept>
	<skos:Concept rdf:about="http://www.earthobservations.org/GEOSS/EO_Vocabulary/terrestrial%20hydrosphere">
		<skos:prefLabel>TERRESTRIAL HYDROSPHERE</skos:prefLabel>
		<skos:narrower rdf:resource="http://www.earthobservations.org/GEOSS/EO_Vocabulary/glaciers%2Fice%20sheets"/>
		<skos:narrower rdf:resource="http://www.earthobservations.org/GEOSS/EO_Vocabulary/snow%2Fice"/>
		<skos:narrower rdf:resource="http://www.earthobservations.org/GEOSS/EO_Vocabulary/surface%20water"/>
		<skos:narrower rdf:resource="http://www.earthobservations.org/GEOSS/EO_Vocabulary/water%20quality%2Fwater%20chemistry"/>
		<skos:narrower rdf:resource="http://www.earthobservations.org/GEOSS/EO_Vocabulary/water%C2%A0quality%2Fwater%20chemistry"/>
		<skos:narrower rdf:resource="http://www.earthobservations.org/GEOSS/EO_Vocabulary/ground%20water"/>
		<skos:inScheme rdf:resource="http://www.earthobservations.org/GEOSS/EO_Vocabulary"/>
	</skos:Concept>
	<skos:Concept rdf:about="http://www.earthobservations.org/GEOSS/EO_Vocabulary/cryosphere">
		<skos:prefLabel>CRYOSPHERE</skos:prefLabel>
		<skos:narrower rdf:resource="http://www.earthobservations.org/GEOSS/EO_Vocabulary/frozen%20ground"/>
		<skos:narrower rdf:resource="http://www.earthobservations.org/GEOSS/EO_Vocabulary/glaciers%2Fice%20sheets"/>
		<skos:narrower rdf:resource="http://www.earthobservations.org/GEOSS/EO_Vocabulary/sea%20ice"/>
		<skos:narrower rdf:resource="http://www.earthobservations.org/GEOSS/EO_Vocabulary/snow%2Fice"/>
		<skos:inScheme rdf:resource="http://www.earthobservations.org/GEOSS/EO_Vocabulary"/>
	</skos:Concept>
	<skos:Concept rdf:about="http://www.earthobservations.org/GEOSS/EO_Vocabulary/paleoclimate">
		<skos:prefLabel>PALEOCLIMATE</skos:prefLabel>
		<skos:narrower rdf:resource="http://www.earthobservations.org/GEOSS/EO_Vocabulary/ocean%2Flake%20records"/>
		<skos:narrower rdf:resource="http://www.earthobservations.org/GEOSS/EO_Vocabulary/ice%20core%20records"/>
		<skos:inScheme rdf:resource="http://www.earthobservations.org/GEOSS/EO_Vocabulary"/>
	</skos:Concept>
	<skos:Concept rdf:about="http://www.earthobservations.org/GEOSS/EO_Vocabulary/solid%20earth">
		<skos:prefLabel>SOLID EARTH</skos:prefLabel>
		<skos:narrower rdf:resource="http://www.earthobservations.org/GEOSS/EO_Vocabulary/geodetics%2Fgravity"/>
		<skos:narrower rdf:resource="http://www.earthobservations.org/GEOSS/EO_Vocabulary/geomorphology"/>
		<skos:narrower rdf:resource="http://www.earthobservations.org/GEOSS/EO_Vocabulary/rocks%2Fminerals%C2%A0"/>
		<skos:narrower rdf:resource="http://www.earthobservations.org/GEOSS/EO_Vocabulary/seismology"/>
		<skos:narrower rdf:resource="http://www.earthobservations.org/GEOSS/EO_Vocabulary/tectonics%C2%A0"/>
		<skos:narrower rdf:resource="http://www.earthobservations.org/GEOSS/EO_Vocabulary/natural%20resources"/>
		<skos:narrower rdf:resource="http://www.earthobservations.org/GEOSS/EO_Vocabulary/geomagnetism"/>
		<skos:inScheme rdf:resource="http://www.earthobservations.org/GEOSS/EO_Vocabulary"/>
	</skos:Concept>
	<skos:Concept rdf:about="http://www.earthobservations.org/GEOSS/EO_Vocabulary/biological%20classification">
		<skos:prefLabel>BIOLOGICAL CLASSIFICATION</skos:prefLabel>
		<skos:narrower rdf:resource="http://www.earthobservations.org/GEOSS/EO_Vocabulary/animals%2Fvertebrates"/>
		<skos:narrower rdf:resource="http://www.earthobservations.org/GEOSS/EO_Vocabulary/bacteria%2Farchaea"/>
		<skos:narrower rdf:resource="http://www.earthobservations.org/GEOSS/EO_Vocabulary/plants"/>
		<skos:inScheme rdf:resource="http://www.earthobservations.org/GEOSS/EO_Vocabulary"/>
	</skos:Concept>
	<!-- fix duplicates -->
	<skos:Concept rdf:about="http://www.earthobservations.org/GEOSS/EO_Vocabulary/soils">
		<skos:prefLabel>SOILS</skos:prefLabel>
		<skos:broader rdf:resource="http://www.earthobservations.org/GEOSS/EO_Vocabulary/agriculture"/>
		<skos:broader rdf:resource="http://www.earthobservations.org/GEOSS/EO_Vocabulary/land%20surface"/>
		<skos:narrower rdf:resource="http://www.earthobservations.org/GEOSS/EO_Vocabulary/soil%20moisture"/>
		<skos:narrower rdf:resource="http://www.earthobservations.org/GEOSS/EO_Vocabulary/soil%20moisture"/>
		<skos:narrower rdf:resource="http://www.earthobservations.org/GEOSS/EO_Vocabulary/soil%20composition"/>
		<skos:narrower rdf:resource="http://www.earthobservations.org/GEOSS/EO_Vocabulary/soil%20type"/>
		<skos:narrower rdf:resource="http://www.earthobservations.org/GEOSS/EO_Vocabulary/soil%20type"/>
		<skos:narrower rdf:resource="http://www.earthobservations.org/GEOSS/EO_Vocabulary/soil%20carbon"/>
		<skos:narrower rdf:resource="http://www.earthobservations.org/GEOSS/EO_Vocabulary/soil%20carbon"/>
		<skos:narrower rdf:resource="http://www.earthobservations.org/GEOSS/EO_Vocabulary/permafrost"/>
		<skos:narrower rdf:resource="http://www.earthobservations.org/GEOSS/EO_Vocabulary/permafrost"/>
		<skos:narrower rdf:resource="http://www.earthobservations.org/GEOSS/EO_Vocabulary/carbon%20%28stores%2C%20uptake%2C%20flux%29"/>
		<skos:narrower rdf:resource="http://www.earthobservations.org/GEOSS/EO_Vocabulary/carbon%20%28stores%2C%20uptake%2C%20flux%29"/>
		<skos:narrower rdf:resource="http://www.earthobservations.org/GEOSS/EO_Vocabulary/soil%20thickness"/>
		<skos:narrower rdf:resource="http://www.earthobservations.org/GEOSS/EO_Vocabulary/soil%20thickness"/>
		<skos:narrower rdf:resource="http://www.earthobservations.org/GEOSS/EO_Vocabulary/thermokarst"/>
		<skos:narrower rdf:resource="http://www.earthobservations.org/GEOSS/EO_Vocabulary/carbon%20in%20subsurface%20ocean"/>
		<skos:narrower rdf:resource="http://www.earthobservations.org/GEOSS/EO_Vocabulary/carbon%20in%20subsurface%20ocean"/>
		<skos:inScheme rdf:resource="http://www.earthobservations.org/GEOSS/EO_Vocabulary"/>
	</skos:Concept>
	<skos:Concept rdf:about="http://www.earthobservations.org/GEOSS/EO_Vocabulary/atmospheric%20temperature">
		<skos:prefLabel>ATMOSPHERIC TEMPERATURE</skos:prefLabel>
		<skos:broader rdf:resource="http://www.earthobservations.org/GEOSS/EO_Vocabulary/atmosphere"/>
		<skos:narrower rdf:resource="http://www.earthobservations.org/GEOSS/EO_Vocabulary/surface%20air%20temperature"/>
		<skos:narrower rdf:resource="http://www.earthobservations.org/GEOSS/EO_Vocabulary/upper%20level%20temperature"/>
		<skos:narrower rdf:resource="http://www.earthobservations.org/GEOSS/EO_Vocabulary/surface%20albedo"/>
		<skos:narrower rdf:resource="http://www.earthobservations.org/GEOSS/EO_Vocabulary/sea%20ice%20surface%20%28skin%29%20temperature"/>
		<skos:narrower rdf:resource="http://www.earthobservations.org/GEOSS/EO_Vocabulary/soil%20thaw"/>
		<skos:inScheme rdf:resource="http://www.earthobservations.org/GEOSS/EO_Vocabulary"/>
	</skos:Concept>
	<skos:Concept rdf:about="http://www.earthobservations.org/GEOSS/EO_Vocabulary/atmospheric%20winds">
		<skos:prefLabel>ATMOSPHERIC WINDS</skos:prefLabel>
		<skos:broader rdf:resource="http://www.earthobservations.org/GEOSS/EO_Vocabulary/atmosphere"/>
		<skos:narrower rdf:resource="http://www.earthobservations.org/GEOSS/EO_Vocabulary/surface%20wind%20speed"/>
		<skos:narrower rdf:resource="http://www.earthobservations.org/GEOSS/EO_Vocabulary/surface%20wind%20direction"/>
		<skos:narrower rdf:resource="http://www.earthobservations.org/GEOSS/EO_Vocabulary/upper%20level%20winds"/>
		<skos:inScheme rdf:resource="http://www.earthobservations.org/GEOSS/EO_Vocabulary"/>
	</skos:Concept>
	<skos:Concept rdf:about="http://www.earthobservations.org/GEOSS/EO_Vocabulary/ocean%20winds">
		<skos:prefLabel>OCEAN WINDS</skos:prefLabel>
		<skos:broader rdf:resource="http://www.earthobservations.org/GEOSS/EO_Vocabulary/oceans"/>
		<skos:narrower rdf:resource="http://www.earthobservations.org/GEOSS/EO_Vocabulary/surface%20wind%20speed"/>
		<skos:narrower rdf:resource="http://www.earthobservations.org/GEOSS/EO_Vocabulary/surface%20wind%20direction"/>
		<skos:inScheme rdf:resource="http://www.earthobservations.org/GEOSS/EO_Vocabulary"/>
	</skos:Concept>
	<!-- fix duplicates -->
	<skos:Concept rdf:about="http://www.earthobservations.org/GEOSS/EO_Vocabulary/land%20use%2Fland%20cover">
		<skos:prefLabel>LAND USE/LAND COVER</skos:prefLabel>
		<skos:broader rdf:resource="http://www.earthobservations.org/GEOSS/EO_Vocabulary/human%20dimensions"/>
		<skos:broader rdf:resource="http://www.earthobservations.org/GEOSS/EO_Vocabulary/land%20surface"/>
		<skos:narrower rdf:resource="http://www.earthobservations.org/GEOSS/EO_Vocabulary/land%20cover"/>
		<skos:narrower rdf:resource="http://www.earthobservations.org/GEOSS/EO_Vocabulary/land%20cover"/>
		<skos:narrower rdf:resource="http://www.earthobservations.org/GEOSS/EO_Vocabulary/land%20use"/>
		<skos:narrower rdf:resource="http://www.earthobservations.org/GEOSS/EO_Vocabulary/land%20use"/>
		<skos:narrower rdf:resource="http://www.earthobservations.org/GEOSS/EO_Vocabulary/cultivation"/>
		<skos:narrower rdf:resource="http://www.earthobservations.org/GEOSS/EO_Vocabulary/vector%20population"/>
		<skos:narrower rdf:resource="http://www.earthobservations.org/GEOSS/EO_Vocabulary/field%20cover%20%28continuous%29"/>
		<skos:inScheme rdf:resource="http://www.earthobservations.org/GEOSS/EO_Vocabulary"/>
	</skos:Concept>
	<skos:Concept rdf:about="http://www.earthobservations.org/GEOSS/EO_Vocabulary/atmospheric%20water%20vapor">
		<skos:prefLabel>ATMOSPHERIC WATER VAPOR</skos:prefLabel>
		<skos:broader rdf:resource="http://www.earthobservations.org/GEOSS/EO_Vocabulary/atmosphere"/>
		<skos:narrower rdf:resource="http://www.earthobservations.org/GEOSS/EO_Vocabulary/surface%20humidity"/>
		<skos:narrower rdf:resource="http://www.earthobservations.org/GEOSS/EO_Vocabulary/upper%20level%20humidity"/>
		<skos:narrower rdf:resource="http://www.earthobservations.org/GEOSS/EO_Vocabulary/evaporation"/>
		<skos:narrower rdf:resource="http://www.earthobservations.org/GEOSS/EO_Vocabulary/evapotranspiration"/>
		<skos:narrower rdf:resource="http://www.earthobservations.org/GEOSS/EO_Vocabulary/aerosol%20properties"/>
		<skos:inScheme rdf:resource="http://www.earthobservations.org/GEOSS/EO_Vocabulary"/>
	</skos:Concept>
	<!-- fix duplicates -->
	<skos:Concept rdf:about="http://www.earthobservations.org/GEOSS/EO_Vocabulary/vegetation">
		<skos:prefLabel>VEGETATION</skos:prefLabel>
		<skos:broader rdf:resource="http://www.earthobservations.org/GEOSS/EO_Vocabulary/biosphere"/>
		<skos:narrower rdf:resource="http://www.earthobservations.org/GEOSS/EO_Vocabulary/vegetation%20cover"/>
		<skos:narrower rdf:resource="http://www.earthobservations.org/GEOSS/EO_Vocabulary/normalized%20difference%20vegetation%20index%20%28ndvi%29"/>
		<skos:narrower rdf:resource="http://www.earthobservations.org/GEOSS/EO_Vocabulary/vegetation%20type"/>
		<skos:narrower rdf:resource="http://www.earthobservations.org/GEOSS/EO_Vocabulary/leaf%20area%20index%20%28lai%29"/>
		<skos:narrower rdf:resource="http://www.earthobservations.org/GEOSS/EO_Vocabulary/biomass"/>
		<skos:narrower rdf:resource="http://www.earthobservations.org/GEOSS/EO_Vocabulary/enhanced%20vegetation%20index%20%28evi%29"/>
		<skos:narrower rdf:resource="http://www.earthobservations.org/GEOSS/EO_Vocabulary/soil%20adjusted%20vegetation%20index%20%28savi%29%2Bc29"/>
		<skos:narrower rdf:resource="http://www.earthobservations.org/GEOSS/EO_Vocabulary/photosynthetically%20active%20radiation%20%28par%29"/>
		<skos:narrower rdf:resource="http://www.earthobservations.org/GEOSS/EO_Vocabulary/fraction%20of%20absorbed%20photosynthetically%20active%20radiation%20%28fapar%29"/>
		<skos:narrower rdf:resource="http://www.earthobservations.org/GEOSS/EO_Vocabulary/non-native%20species"/>
		<skos:narrower rdf:resource="http://www.earthobservations.org/GEOSS/EO_Vocabulary/forest%20litter"/>
		<skos:narrower rdf:resource="http://www.earthobservations.org/GEOSS/EO_Vocabulary/nutrients%20%28phosphorous%2C%20nitrogen%2C%20potassium%2C%20nitrates%2Csulfates%29"/>
		<skos:narrower rdf:resource="http://www.earthobservations.org/GEOSS/EO_Vocabulary/forest%20structure"/>
		<skos:narrower rdf:resource="http://www.earthobservations.org/GEOSS/EO_Vocabulary/species%20composition"/>
		<skos:narrower rdf:resource="http://www.earthobservations.org/GEOSS/EO_Vocabulary/chlorophyll"/>
		<skos:narrower rdf:resource="http://www.earthobservations.org/GEOSS/EO_Vocabulary/phenology"/>
		<skos:narrower rdf:resource="http://www.earthobservations.org/GEOSS/EO_Vocabulary/phenology"/>
		<skos:narrower rdf:resource="http://www.earthobservations.org/GEOSS/EO_Vocabulary/stand%20density%2Fheight%2Fvolume"/>
		<skos:narrower rdf:resource="http://www.earthobservations.org/GEOSS/EO_Vocabulary/geologic%20stratification"/>
		<skos:narrower rdf:resource="http://www.earthobservations.org/GEOSS/EO_Vocabulary/inundated%20vegetation"/>
		<skos:inScheme rdf:resource="http://www.earthobservations.org/GEOSS/EO_Vocabulary"/>
	</skos:Concept>
	<skos:Concept rdf:about="http://www.earthobservations.org/GEOSS/EO_Vocabulary/ocean%20temperature">
		<skos:prefLabel>OCEAN TEMPERATURE</skos:prefLabel>
		<skos:broader rdf:resource="http://www.earthobservations.org/GEOSS/EO_Vocabulary/oceans"/>
		<skos:narrower rdf:resource="http://www.earthobservations.org/GEOSS/EO_Vocabulary/sea%20surface%20temperature"/>
		<skos:inScheme rdf:resource="http://www.earthobservations.org/GEOSS/EO_Vocabulary"/>
	</skos:Concept>
	<skos:Concept rdf:about="http://www.earthobservations.org/GEOSS/EO_Vocabulary/environmental%20impacts">
		<skos:prefLabel>ENVIRONMENTAL IMPACTS</skos:prefLabel>
		<skos:broader rdf:resource="http://www.earthobservations.org/GEOSS/EO_Vocabulary/human%20dimensions"/>
		<skos:narrower rdf:resource="http://www.earthobservations.org/GEOSS/EO_Vocabulary/urbanization"/>
		<skos:narrower rdf:resource="http://www.earthobservations.org/GEOSS/EO_Vocabulary/contaminants%2Fpollutants%20%28inorganic%2Forganic%29"/>
		<skos:narrower rdf:resource="http://www.earthobservations.org/GEOSS/EO_Vocabulary/fuel%20load%2Fcharacteristics"/>
		<skos:inScheme rdf:resource="http://www.earthobservations.org/GEOSS/EO_Vocabulary"/>
	</skos:Concept>
	<skos:Concept rdf:about="http://www.earthobservations.org/GEOSS/EO_Vocabulary/land%20temperature">
		<skos:prefLabel>LAND TEMPERATURE</skos:prefLabel>
		<skos:broader rdf:resource="http://www.earthobservations.org/GEOSS/EO_Vocabulary/land%20surface"/>
		<skos:narrower rdf:resource="http://www.earthobservations.org/GEOSS/EO_Vocabulary/land%20surface%20temperature"/>
		<skos:narrower rdf:resource="http://www.earthobservations.org/GEOSS/EO_Vocabulary/sea%20ice%20surface%20%28skin%29%20temperature"/>
		<skos:inScheme rdf:resource="http://www.earthobservations.org/GEOSS/EO_Vocabulary"/>
	</skos:Concept>
	<skos:Concept rdf:about="http://www.earthobservations.org/GEOSS/EO_Vocabulary/atmospheric%20pressure">
		<skos:prefLabel>ATMOSPHERIC PRESSURE</skos:prefLabel>
		<skos:broader rdf:resource="http://www.earthobservations.org/GEOSS/EO_Vocabulary/atmosphere"/>
		<skos:narrower rdf:resource="http://www.earthobservations.org/GEOSS/EO_Vocabulary/surface%20atmospheric%20pressure"/>
		<skos:narrower rdf:resource="http://www.earthobservations.org/GEOSS/EO_Vocabulary/surface%20radiation%20budget"/>
		<skos:inScheme rdf:resource="http://www.earthobservations.org/GEOSS/EO_Vocabulary"/>
	</skos:Concept>
	<skos:Concept rdf:about="http://www.earthobservations.org/GEOSS/EO_Vocabulary/frozen%20ground">
		<skos:prefLabel>FROZEN GROUND</skos:prefLabel>
		<skos:broader rdf:resource="http://www.earthobservations.org/GEOSS/EO_Vocabulary/land%20surface"/>
		<skos:broader rdf:resource="http://www.earthobservations.org/GEOSS/EO_Vocabulary/cryosphere"/>
		<skos:narrower rdf:resource="http://www.earthobservations.org/GEOSS/EO_Vocabulary/glacier%2Fice%20sheet%20extent"/>
		<skos:inScheme rdf:resource="http://www.earthobservations.org/GEOSS/EO_Vocabulary"/>
	</skos:Concept>
	<!-- fix duplicates -->
	<skos:Concept rdf:about="http://www.earthobservations.org/GEOSS/EO_Vocabulary/sea%20ice">
		<skos:prefLabel>SEA ICE</skos:prefLabel>
		<skos:broader rdf:resource="http://www.earthobservations.org/GEOSS/EO_Vocabulary/oceans"/>
		<skos:broader rdf:resource="http://www.earthobservations.org/GEOSS/EO_Vocabulary/cryosphere"/>
		<skos:narrower rdf:resource="http://www.earthobservations.org/GEOSS/EO_Vocabulary/glacier%2Fice%20sheet%20extent"/>
		<skos:narrower rdf:resource="http://www.earthobservations.org/GEOSS/EO_Vocabulary/elevation"/>
		<skos:narrower rdf:resource="http://www.earthobservations.org/GEOSS/EO_Vocabulary/ocean%20salinity"/>
		<skos:narrower rdf:resource="http://www.earthobservations.org/GEOSS/EO_Vocabulary/ocean%20salinity"/>
		<skos:narrower rdf:resource="http://www.earthobservations.org/GEOSS/EO_Vocabulary/ice"/>
		<skos:narrower rdf:resource="http://www.earthobservations.org/GEOSS/EO_Vocabulary/snow%20depth"/>
		<skos:narrower rdf:resource="http://www.earthobservations.org/GEOSS/EO_Vocabulary/sea%20ice%20cover"/>
		<skos:narrower rdf:resource="http://www.earthobservations.org/GEOSS/EO_Vocabulary/sea%20ice%20cover"/>
		<skos:narrower rdf:resource="http://www.earthobservations.org/GEOSS/EO_Vocabulary/ice%20depth"/>
		<skos:narrower rdf:resource="http://www.earthobservations.org/GEOSS/EO_Vocabulary/ice%20depth"/>
		<skos:narrower rdf:resource="http://www.earthobservations.org/GEOSS/EO_Vocabulary/impervious%20surface%20extent"/>
		<skos:inScheme rdf:resource="http://www.earthobservations.org/GEOSS/EO_Vocabulary"/>
	</skos:Concept>
	<skos:Concept rdf:about="http://www.earthobservations.org/GEOSS/EO_Vocabulary/glaciers%2Fice%20sheets">
		<skos:prefLabel>GLACIERS/ICE SHEETS</skos:prefLabel>
		<skos:broader rdf:resource="http://www.earthobservations.org/GEOSS/EO_Vocabulary/terrestrial%20hydrosphere"/>
		<skos:broader rdf:resource="http://www.earthobservations.org/GEOSS/EO_Vocabulary/cryosphere"/>
		<skos:narrower rdf:resource="http://www.earthobservations.org/GEOSS/EO_Vocabulary/glacier%2Fice%20sheet%20depth"/>
		<skos:narrower rdf:resource="http://www.earthobservations.org/GEOSS/EO_Vocabulary/glacier%2Fice%20cap%20elevation"/>
		<skos:inScheme rdf:resource="http://www.earthobservations.org/GEOSS/EO_Vocabulary"/>
	</skos:Concept>
	<!-- fix duplicates -->
	<skos:Concept rdf:about="http://www.earthobservations.org/GEOSS/EO_Vocabulary/snow%2Fice">
		<skos:prefLabel>SNOW/ICE</skos:prefLabel>
		<skos:broader rdf:resource="http://www.earthobservations.org/GEOSS/EO_Vocabulary/terrestrial%20hydrosphere"/>
		<skos:broader rdf:resource="http://www.earthobservations.org/GEOSS/EO_Vocabulary/cryosphere"/>
		<skos:narrower rdf:resource="http://www.earthobservations.org/GEOSS/EO_Vocabulary/snow%20cover%20extent"/>
		<skos:narrower rdf:resource="http://www.earthobservations.org/GEOSS/EO_Vocabulary/snow%20cover%20extent"/>
		<skos:narrower rdf:resource="http://www.earthobservations.org/GEOSS/EO_Vocabulary/glacier%2Fice%20sheet%20depth"/>
		<skos:narrower rdf:resource="http://www.earthobservations.org/GEOSS/EO_Vocabulary/glacier%2Fice%20cap%20elevation"/>
		<skos:narrower rdf:resource="http://www.earthobservations.org/GEOSS/EO_Vocabulary/snow%20water%20equivalent%20%28swe%29"/>
		<skos:narrower rdf:resource="http://www.earthobservations.org/GEOSS/EO_Vocabulary/snow%20water%20equivalent%20%28swe%29"/>
		<skos:narrower rdf:resource="http://www.earthobservations.org/GEOSS/EO_Vocabulary/snow%20depth"/>
		<skos:narrower rdf:resource="http://www.earthobservations.org/GEOSS/EO_Vocabulary/impervious%20surface%20extent"/>
		<skos:narrower rdf:resource="http://www.earthobservations.org/GEOSS/EO_Vocabulary/soil%20thaw"/>
		<skos:inScheme rdf:resource="http://www.earthobservations.org/GEOSS/EO_Vocabulary"/>
	</skos:Concept>
	<skos:Concept rdf:about="http://www.earthobservations.org/GEOSS/EO_Vocabulary/topography">
		<skos:prefLabel>TOPOGRAPHY</skos:prefLabel>
		<skos:broader rdf:resource="http://www.earthobservations.org/GEOSS/EO_Vocabulary/land%20surface"/>
		<skos:narrower rdf:resource="http://www.earthobservations.org/GEOSS/EO_Vocabulary/elevation"/>
		<skos:inScheme rdf:resource="http://www.earthobservations.org/GEOSS/EO_Vocabulary"/>
	</skos:Concept>
	<skos:Concept rdf:about="http://www.earthobservations.org/GEOSS/EO_Vocabulary/surface%20water">
		<skos:prefLabel>SURFACE WATER</skos:prefLabel>
		<skos:broader rdf:resource="http://www.earthobservations.org/GEOSS/EO_Vocabulary/terrestrial%20hydrosphere"/>
		<skos:narrower rdf:resource="http://www.earthobservations.org/GEOSS/EO_Vocabulary/river%20flow%20observations"/>
		<skos:narrower rdf:resource="http://www.earthobservations.org/GEOSS/EO_Vocabulary/groundwater"/>
		<skos:narrower rdf:resource="http://www.earthobservations.org/GEOSS/EO_Vocabulary/water%20run-off"/>
		<skos:narrower rdf:resource="http://www.earthobservations.org/GEOSS/EO_Vocabulary/floods"/>
		<skos:narrower rdf:resource="http://www.earthobservations.org/GEOSS/EO_Vocabulary/water%20depth%20%28shallow%20near-shore%29"/>
		<skos:narrower rdf:resource="http://www.earthobservations.org/GEOSS/EO_Vocabulary/source%20of%20drinking%20water"/>
		<skos:narrower rdf:resource="http://www.earthobservations.org/GEOSS/EO_Vocabulary/hydrology"/>
		<skos:narrower rdf:resource="http://www.earthobservations.org/GEOSS/EO_Vocabulary/thermokarst"/>
		<skos:inScheme rdf:resource="http://www.earthobservations.org/GEOSS/EO_Vocabulary"/>
	</skos:Concept>
	<skos:Concept rdf:about="http://www.earthobservations.org/GEOSS/EO_Vocabulary/ecological%20dynamics">
		<skos:prefLabel>ECOLOGICAL DYNAMICS</skos:prefLabel>
		<skos:broader rdf:resource="http://www.earthobservations.org/GEOSS/EO_Vocabulary/biosphere"/>
		<skos:narrower rdf:resource="http://www.earthobservations.org/GEOSS/EO_Vocabulary/net%20primary%20production"/>
		<skos:narrower rdf:resource="http://www.earthobservations.org/GEOSS/EO_Vocabulary/biodiversity"/>
		<skos:narrower rdf:resource="http://www.earthobservations.org/GEOSS/EO_Vocabulary/ecosystem%20function%2Fdynamics"/>
		<skos:narrower rdf:resource="http://www.earthobservations.org/GEOSS/EO_Vocabulary/animal%20activity%20%28range%2C%20season%20length%2C%20migration%20patterns%29"/>
		<skos:narrower rdf:resource="http://www.earthobservations.org/GEOSS/EO_Vocabulary/geologic%20stratification"/>
		<skos:narrower rdf:resource="http://www.earthobservations.org/GEOSS/EO_Vocabulary/pathogen%20population%20dynamic"/>
		<skos:inScheme rdf:resource="http://www.earthobservations.org/GEOSS/EO_Vocabulary"/>
	</skos:Concept>
	<skos:Concept rdf:about="http://www.earthobservations.org/GEOSS/EO_Vocabulary/coastal%20processes">
		<skos:prefLabel>COASTAL PROCESSES</skos:prefLabel>
		<skos:broader rdf:resource="http://www.earthobservations.org/GEOSS/EO_Vocabulary/oceans"/>
		<skos:narrower rdf:resource="http://www.earthobservations.org/GEOSS/EO_Vocabulary/sea%20level"/>
		<skos:narrower rdf:resource="http://www.earthobservations.org/GEOSS/EO_Vocabulary/currents"/>
		<skos:narrower rdf:resource="http://www.earthobservations.org/GEOSS/EO_Vocabulary/erosion%20%28reefs%2C%20sandbars%29"/>
		<skos:inScheme rdf:resource="http://www.earthobservations.org/GEOSS/EO_Vocabulary"/>
	</skos:Concept>
	<skos:Concept rdf:about="http://www.earthobservations.org/GEOSS/EO_Vocabulary/ocean%2Flake%20records">
		<skos:prefLabel>OCEAN/LAKE RECORDS</skos:prefLabel>
		<skos:broader rdf:resource="http://www.earthobservations.org/GEOSS/EO_Vocabulary/paleoclimate"/>
		<skos:narrower rdf:resource="http://www.earthobservations.org/GEOSS/EO_Vocabulary/lake%2Freservoir%20levels%20and%20area"/>
		<skos:inScheme rdf:resource="http://www.earthobservations.org/GEOSS/EO_Vocabulary"/>
	</skos:Concept>
	<skos:Concept rdf:about="http://www.earthobservations.org/GEOSS/EO_Vocabulary/agricultural%20engineering">
		<skos:prefLabel>AGRICULTURAL ENGINEERING</skos:prefLabel>
		<skos:broader rdf:resource="http://www.earthobservations.org/GEOSS/EO_Vocabulary/agriculture"/>
		<skos:narrower rdf:resource="http://www.earthobservations.org/GEOSS/EO_Vocabulary/cultivation"/>
		<skos:inScheme rdf:resource="http://www.earthobservations.org/GEOSS/EO_Vocabulary"/>
	</skos:Concept>
	<skos:Concept rdf:about="http://www.earthobservations.org/GEOSS/EO_Vocabulary/habitat%20conversion%2Ffragmentation">
		<skos:prefLabel>HABITAT CONVERSION/FRAGMENTATION</skos:prefLabel>
		<skos:broader rdf:resource="http://www.earthobservations.org/GEOSS/EO_Vocabulary/human%20dimensions"/>
		<skos:narrower rdf:resource="http://www.earthobservations.org/GEOSS/EO_Vocabulary/deforestation"/>
		<skos:narrower rdf:resource="http://www.earthobservations.org/GEOSS/EO_Vocabulary/desertification"/>
		<skos:inScheme rdf:resource="http://www.earthobservations.org/GEOSS/EO_Vocabulary"/>
	</skos:Concept>
	<skos:Concept rdf:about="http://www.earthobservations.org/GEOSS/EO_Vocabulary/terrestrial%20ecosystems">
		<skos:prefLabel>TERRESTRIAL ECOSYSTEMS</skos:prefLabel>
		<skos:broader rdf:resource="http://www.earthobservations.org/GEOSS/EO_Vocabulary/biosphere"/>
		<skos:narrower rdf:resource="http://www.earthobservations.org/GEOSS/EO_Vocabulary/forest%20cover"/>
		<skos:narrower rdf:resource="http://www.earthobservations.org/GEOSS/EO_Vocabulary/non-native%20species"/>
		<skos:narrower rdf:resource="http://www.earthobservations.org/GEOSS/EO_Vocabulary/water%20bodies%20%28location%29"/>
		<skos:narrower rdf:resource="http://www.earthobservations.org/GEOSS/EO_Vocabulary/fish%20harvest%20intensity"/>
		<skos:inScheme rdf:resource="http://www.earthobservations.org/GEOSS/EO_Vocabulary"/>
	</skos:Concept>
	<!-- fix duplicates -->
	<skos:Concept rdf:about="http://www.earthobservations.org/GEOSS/EO_Vocabulary/aerosols">
		<skos:prefLabel>AEROSOLS</skos:prefLabel>
		<skos:broader rdf:resource="http://www.earthobservations.org/GEOSS/EO_Vocabulary/atmosphere"/>
		<skos:narrower rdf:resource="http://www.earthobservations.org/GEOSS/EO_Vocabulary/cloud%20cover"/>
		<skos:narrower rdf:resource="http://www.earthobservations.org/GEOSS/EO_Vocabulary/ambient%20particulate%20matter%20concentration%20%28fine%29"/>
		<skos:narrower rdf:resource="http://www.earthobservations.org/GEOSS/EO_Vocabulary/column%20particulate%20matter%20concentration%20%28fine%29"/>
		<skos:narrower rdf:resource="http://www.earthobservations.org/GEOSS/EO_Vocabulary/ambient%20particulate%20matter%20%28fine%29%20composition"/>
		<skos:narrower rdf:resource="http://www.earthobservations.org/GEOSS/EO_Vocabulary/ambient%20particulate%20matter%20composition%20%28coarse%29"/>
		<skos:narrower rdf:resource="http://www.earthobservations.org/GEOSS/EO_Vocabulary/column%20particulate%20matter%20concentration%20%28coarse%29"/>
		<skos:narrower rdf:resource="http://www.earthobservations.org/GEOSS/EO_Vocabulary/aerosol%20properties"/>
		<skos:inScheme rdf:resource="http://www.earthobservations.org/GEOSS/EO_Vocabulary"/>
	</skos:Concept>
	<!-- fix duplicates -->
	<skos:Concept rdf:about="http://www.earthobservations.org/GEOSS/EO_Vocabulary/bathymetry%2Fseafloor%20topography">
		<skos:prefLabel>BATHYMETRY/SEAFLOOR TOPOGRAPHY</skos:prefLabel>
		<skos:broader rdf:resource="http://www.earthobservations.org/GEOSS/EO_Vocabulary/oceans"/>
		<skos:narrower rdf:resource="http://www.earthobservations.org/GEOSS/EO_Vocabulary/ocean%20topography"/>
		<skos:narrower rdf:resource="http://www.earthobservations.org/GEOSS/EO_Vocabulary/ocean%20topography"/>
		<skos:narrower rdf:resource="http://www.earthobservations.org/GEOSS/EO_Vocabulary/bathymetry"/>
		<skos:narrower rdf:resource="http://www.earthobservations.org/GEOSS/EO_Vocabulary/curvature"/>
		<skos:narrower rdf:resource="http://www.earthobservations.org/GEOSS/EO_Vocabulary/water%20depth%20%28shallow%20near-shore%29"/>
		<skos:inScheme rdf:resource="http://www.earthobservations.org/GEOSS/EO_Vocabulary"/>
	</skos:Concept>
	<skos:Concept rdf:about="http://www.earthobservations.org/GEOSS/EO_Vocabulary/agricultural%20plant%20science">
		<skos:prefLabel>AGRICULTURAL PLANT SCIENCE</skos:prefLabel>
		<skos:broader rdf:resource="http://www.earthobservations.org/GEOSS/EO_Vocabulary/agriculture"/>
		<skos:narrower rdf:resource="http://www.earthobservations.org/GEOSS/EO_Vocabulary/soil%20composition"/>
		<skos:narrower rdf:resource="http://www.earthobservations.org/GEOSS/EO_Vocabulary/crop%20emergence"/>
		<skos:narrower rdf:resource="http://www.earthobservations.org/GEOSS/EO_Vocabulary/crop%20yield"/>
		<skos:inScheme rdf:resource="http://www.earthobservations.org/GEOSS/EO_Vocabulary"/>
	</skos:Concept>
	<skos:Concept rdf:about="http://www.earthobservations.org/GEOSS/EO_Vocabulary/surface%20radiative%20properties">
		<skos:prefLabel>SURFACE RADIATIVE PROPERTIES</skos:prefLabel>
		<skos:broader rdf:resource="http://www.earthobservations.org/GEOSS/EO_Vocabulary/land%20surface"/>
		<skos:narrower rdf:resource="http://www.earthobservations.org/GEOSS/EO_Vocabulary/fraction%20of%20photosynthetically%20active%20radiation%20%28fpar%29"/>
		<skos:narrower rdf:resource="http://www.earthobservations.org/GEOSS/EO_Vocabulary/emissivity"/>
		<skos:inScheme rdf:resource="http://www.earthobservations.org/GEOSS/EO_Vocabulary"/>
	</skos:Concept>
	<skos:Concept rdf:about="http://www.earthobservations.org/GEOSS/EO_Vocabulary/atmospheric%20radiation">
		<skos:prefLabel>ATMOSPHERIC RADIATION</skos:prefLabel>
		<skos:broader rdf:resource="http://www.earthobservations.org/GEOSS/EO_Vocabulary/atmosphere"/>
		<skos:narrower rdf:resource="http://www.earthobservations.org/GEOSS/EO_Vocabulary/global%20horizontal%20irradiation%20%28ghi%29"/>
		<skos:narrower rdf:resource="http://www.earthobservations.org/GEOSS/EO_Vocabulary/direct%20normal%20irradiation%20%28dni%29"/>
		<skos:narrower rdf:resource="http://www.earthobservations.org/GEOSS/EO_Vocabulary/surface%20albedo"/>
		<skos:narrower rdf:resource="http://www.earthobservations.org/GEOSS/EO_Vocabulary/emissivity"/>
		<skos:narrower rdf:resource="http://www.earthobservations.org/GEOSS/EO_Vocabulary/outgoing%20longwave%20radiation%20%28top%20of%20atmosphere%20%29"/>
		<skos:inScheme rdf:resource="http://www.earthobservations.org/GEOSS/EO_Vocabulary"/>
	</skos:Concept>
	<skos:Concept rdf:about="http://www.earthobservations.org/GEOSS/EO_Vocabulary/water%20quality%2Fwater%20chemistry">
		<skos:prefLabel>WATER QUALITY/WATER CHEMISTRY</skos:prefLabel>
		<skos:broader rdf:resource="http://www.earthobservations.org/GEOSS/EO_Vocabulary/terrestrial%20hydrosphere"/>
		<skos:narrower rdf:resource="http://www.earthobservations.org/GEOSS/EO_Vocabulary/groundwater"/>
		<skos:narrower rdf:resource="http://www.earthobservations.org/GEOSS/EO_Vocabulary/contaminants%2Fpollutants%20%28inorganic%2Forganic%29"/>
		<skos:narrower rdf:resource="http://www.earthobservations.org/GEOSS/EO_Vocabulary/nutrients%20%28phosphorous%2C%20nitrogen%2C%20potassium%2C%20nitrates%2Csulfates%29"/>
		<skos:narrower rdf:resource="http://www.earthobservations.org/GEOSS/EO_Vocabulary/carbon%20dioxide%20concentration"/>
		<skos:inScheme rdf:resource="http://www.earthobservations.org/GEOSS/EO_Vocabulary"/>
	</skos:Concept>
	<!-- fix duplicates -->
	<skos:Concept rdf:about="http://www.earthobservations.org/GEOSS/EO_Vocabulary/ice%20core%20records">
		<skos:prefLabel>ICE CORE RECORDS</skos:prefLabel>
		<skos:broader rdf:resource="http://www.earthobservations.org/GEOSS/EO_Vocabulary/paleoclimate"/>
		<skos:narrower rdf:resource="http://www.earthobservations.org/GEOSS/EO_Vocabulary/ambient%20particulate%20matter%20concentration%20%28fine%29"/>
		<skos:narrower rdf:resource="http://www.earthobservations.org/GEOSS/EO_Vocabulary/column%20particulate%20matter%20concentration%20%28fine%29"/>
		<skos:narrower rdf:resource="http://www.earthobservations.org/GEOSS/EO_Vocabulary/ambient%20particulate%20matter%20%28fine%29%20composition"/>
		<skos:narrower rdf:resource="http://www.earthobservations.org/GEOSS/EO_Vocabulary/ambient%20particulate%20matter%20composition%20%28coarse%29"/>
		<skos:narrower rdf:resource="http://www.earthobservations.org/GEOSS/EO_Vocabulary/column%20particulate%20matter%20concentration%20%28coarse%29"/>
		<skos:narrower rdf:resource="http://www.earthobservations.org/GEOSS/EO_Vocabulary/methane%20concentration"/>
		<skos:inScheme rdf:resource="http://www.earthobservations.org/GEOSS/EO_Vocabulary"/>
	</skos:Concept>
	<skos:Concept rdf:about="http://www.earthobservations.org/GEOSS/EO_Vocabulary/ecological%20dynamics">
		<skos:prefLabel>ECOLOGICAL DYNAMICS </skos:prefLabel>
		<skos:broader rdf:resource="http://www.earthobservations.org/GEOSS/EO_Vocabulary/biosphere"/>
		<skos:narrower rdf:resource="http://www.earthobservations.org/GEOSS/EO_Vocabulary/gross%20primary%20productivity"/>
		<skos:inScheme rdf:resource="http://www.earthobservations.org/GEOSS/EO_Vocabulary"/>
	</skos:Concept>
	<!-- fix duplicates -->
	<skos:Concept rdf:about="http://www.earthobservations.org/GEOSS/EO_Vocabulary/clouds">
		<skos:prefLabel>CLOUDS</skos:prefLabel>
		<skos:broader rdf:resource="http://www.earthobservations.org/GEOSS/EO_Vocabulary/atmosphere"/>
		<skos:narrower rdf:resource="http://www.earthobservations.org/GEOSS/EO_Vocabulary/cloud%20water%2Fice%20amounts"/>
		<skos:narrower rdf:resource="http://www.earthobservations.org/GEOSS/EO_Vocabulary/cloud%20water%2Fice%20amounts"/>
		<skos:narrower rdf:resource="http://www.earthobservations.org/GEOSS/EO_Vocabulary/cloud%20parameters%20%28other%29"/>
		<skos:inScheme rdf:resource="http://www.earthobservations.org/GEOSS/EO_Vocabulary"/>
	</skos:Concept>
	<skos:Concept rdf:about="http://www.earthobservations.org/GEOSS/EO_Vocabulary/ocean%20heat%20budget">
		<skos:prefLabel>OCEAN HEAT BUDGET</skos:prefLabel>
		<skos:broader rdf:resource="http://www.earthobservations.org/GEOSS/EO_Vocabulary/oceans"/>
		<skos:narrower rdf:resource="http://www.earthobservations.org/GEOSS/EO_Vocabulary/evaporation"/>
		<skos:inScheme rdf:resource="http://www.earthobservations.org/GEOSS/EO_Vocabulary"/>
	</skos:Concept>
	<skos:Concept rdf:about="http://www.earthobservations.org/GEOSS/EO_Vocabulary/atmospheric%20chemistry">
		<skos:prefLabel>ATMOSPHERIC CHEMISTRY</skos:prefLabel>
		<skos:broader rdf:resource="http://www.earthobservations.org/GEOSS/EO_Vocabulary/atmosphere"/>
		<skos:narrower rdf:resource="http://www.earthobservations.org/GEOSS/EO_Vocabulary/ambient%20ozone%20concentration"/>
		<skos:narrower rdf:resource="http://www.earthobservations.org/GEOSS/EO_Vocabulary/column%20ozone%20concentration"/>
		<skos:narrower rdf:resource="http://www.earthobservations.org/GEOSS/EO_Vocabulary/column%20nitrogen%20dioxide%20concentration"/>
		<skos:narrower rdf:resource="http://www.earthobservations.org/GEOSS/EO_Vocabulary/ambient%20nitrogen%20dioxide%20concentration"/>
		<skos:narrower rdf:resource="http://www.earthobservations.org/GEOSS/EO_Vocabulary/ambient%20sulfur%20dioxide%20concentration"/>
		<skos:narrower rdf:resource="http://www.earthobservations.org/GEOSS/EO_Vocabulary/carbon%20dioxide%20concentration"/>
		<skos:narrower rdf:resource="http://www.earthobservations.org/GEOSS/EO_Vocabulary/column%20sulfur%20dioxide%20concentration"/>
		<skos:narrower rdf:resource="http://www.earthobservations.org/GEOSS/EO_Vocabulary/methane%20concentration"/>
		<skos:narrower rdf:resource="http://www.earthobservations.org/GEOSS/EO_Vocabulary/carbon%20dioxide%20partial%20pressure"/>
		<skos:narrower rdf:resource="http://www.earthobservations.org/GEOSS/EO_Vocabulary/stratospheric%20ozone"/>
		<skos:inScheme rdf:resource="http://www.earthobservations.org/GEOSS/EO_Vocabulary"/>
	</skos:Concept>
	<skos:Concept rdf:about="http://www.earthobservations.org/GEOSS/EO_Vocabulary/natural%20hazards">
		<skos:prefLabel>NATURAL HAZARDS</skos:prefLabel>
		<skos:broader rdf:resource="http://www.earthobservations.org/GEOSS/EO_Vocabulary/human%20dimensions"/>
		<skos:narrower rdf:resource="http://www.earthobservations.org/GEOSS/EO_Vocabulary/burned%20area%2Ffires"/>
		<skos:inScheme rdf:resource="http://www.earthobservations.org/GEOSS/EO_Vocabulary"/>
	</skos:Concept>
	<skos:Concept rdf:about="http://www.earthobservations.org/GEOSS/EO_Vocabulary/ocean%20optics">
		<skos:prefLabel>OCEAN OPTICS</skos:prefLabel>
		<skos:broader rdf:resource="http://www.earthobservations.org/GEOSS/EO_Vocabulary/oceans"/>
		<skos:narrower rdf:resource="http://www.earthobservations.org/GEOSS/EO_Vocabulary/photosynthetically%20active%20radiation%20%28par%29"/>
		<skos:narrower rdf:resource="http://www.earthobservations.org/GEOSS/EO_Vocabulary/fraction%20of%20absorbed%20photosynthetically%20active%20radiation%20%28fapar%29"/>
		<skos:inScheme rdf:resource="http://www.earthobservations.org/GEOSS/EO_Vocabulary"/>
	</skos:Concept>
	<skos:Concept rdf:about="http://www.earthobservations.org/GEOSS/EO_Vocabulary/water%20quality">
		<skos:prefLabel>WATER QUALITY</skos:prefLabel>
		<skos:broader rdf:resource="http://www.earthobservations.org/GEOSS/EO_Vocabulary/oceans"/>
		<skos:narrower rdf:resource="http://www.earthobservations.org/GEOSS/EO_Vocabulary/water%20quality%20%26%20composition%2C%20ph%20and%20salinity%2C%20dissolved%20oxygen%20content"/>
		<skos:inScheme rdf:resource="http://www.earthobservations.org/GEOSS/EO_Vocabulary"/>
	</skos:Concept>
	<skos:Concept rdf:about="http://www.earthobservations.org/GEOSS/EO_Vocabulary/ocean%20chemistry">
		<skos:prefLabel>OCEAN CHEMISTRY</skos:prefLabel>
		<skos:broader rdf:resource="http://www.earthobservations.org/GEOSS/EO_Vocabulary/oceans"/>
		<skos:narrower rdf:resource="http://www.earthobservations.org/GEOSS/EO_Vocabulary/water%20quality%20%26%20composition%2C%20ph%20and%20salinity%2C%20dissolved%20oxygen%20content"/>
		<skos:narrower rdf:resource="http://www.earthobservations.org/GEOSS/EO_Vocabulary/column%20nitrogen%20dioxide%20concentration"/>
		<skos:narrower rdf:resource="http://www.earthobservations.org/GEOSS/EO_Vocabulary/ambient%20nitrogen%20dioxide%20concentration"/>
		<skos:narrower rdf:resource="http://www.earthobservations.org/GEOSS/EO_Vocabulary/chlorophyll"/>
		<skos:narrower rdf:resource="http://www.earthobservations.org/GEOSS/EO_Vocabulary/carbon%20dioxide%20partial%20pressure"/>
		<skos:inScheme rdf:resource="http://www.earthobservations.org/GEOSS/EO_Vocabulary"/>
	</skos:Concept>
	<skos:Concept rdf:about="http://www.earthobservations.org/GEOSS/EO_Vocabulary/salinity%2Fdensity">
		<skos:prefLabel>SALINITY/DENSITY</skos:prefLabel>
		<skos:broader rdf:resource="http://www.earthobservations.org/GEOSS/EO_Vocabulary/oceans"/>
		<skos:narrower rdf:resource="http://www.earthobservations.org/GEOSS/EO_Vocabulary/stand%20density%2Fheight%2Fvolume"/>
		<skos:narrower rdf:resource="http://www.earthobservations.org/GEOSS/EO_Vocabulary/density%20of%20animal%20hosts"/>
		<skos:inScheme rdf:resource="http://www.earthobservations.org/GEOSS/EO_Vocabulary"/>
	</skos:Concept>
	<skos:Concept rdf:about="http://www.earthobservations.org/GEOSS/EO_Vocabulary/aquatic%20ecosystems">
		<skos:prefLabel>AQUATIC ECOSYSTEMS </skos:prefLabel>
		<skos:broader rdf:resource="http://www.earthobservations.org/GEOSS/EO_Vocabulary/biosphere"/>
		<skos:inScheme rdf:resource="http://www.earthobservations.org/GEOSS/EO_Vocabulary"/>
	</skos:Concept>
	<skos:Concept rdf:about="http://www.earthobservations.org/GEOSS/EO_Vocabulary/fungi">
		<skos:prefLabel>FUNGI</skos:prefLabel>
		<skos:broader rdf:resource="http://www.earthobservations.org/GEOSS/EO_Vocabulary/biosphere"/>
		<skos:narrower rdf:resource="http://www.earthobservations.org/GEOSS/EO_Vocabulary/biodiversity"/>
		<skos:inScheme rdf:resource="http://www.earthobservations.org/GEOSS/EO_Vocabulary"/>
	</skos:Concept>
	<skos:Concept rdf:about="http://www.earthobservations.org/GEOSS/EO_Vocabulary/ocean%20circulation">
		<skos:prefLabel>OCEAN CIRCULATION</skos:prefLabel>
		<skos:broader rdf:resource="http://www.earthobservations.org/GEOSS/EO_Vocabulary/oceans"/>
		<skos:narrower rdf:resource="http://www.earthobservations.org/GEOSS/EO_Vocabulary/currents"/>
		<skos:inScheme rdf:resource="http://www.earthobservations.org/GEOSS/EO_Vocabulary"/>
	</skos:Concept>
	<skos:Concept rdf:about="http://www.earthobservations.org/GEOSS/EO_Vocabulary/erosion%2Fsedimentation">
		<skos:prefLabel>EROSION/SEDIMENTATION</skos:prefLabel>
		<skos:broader rdf:resource="http://www.earthobservations.org/GEOSS/EO_Vocabulary/land%20surface"/>
		<skos:narrower rdf:resource="http://www.earthobservations.org/GEOSS/EO_Vocabulary/slope%20angle"/>
		<skos:narrower rdf:resource="http://www.earthobservations.org/GEOSS/EO_Vocabulary/slope%20movement"/>
		<skos:narrower rdf:resource="http://www.earthobservations.org/GEOSS/EO_Vocabulary/erosion%20%28reefs%2C%20sandbars%29"/>
		<skos:inScheme rdf:resource="http://www.earthobservations.org/GEOSS/EO_Vocabulary"/>
	</skos:Concept>
	<skos:Concept rdf:about="http://www.earthobservations.org/GEOSS/EO_Vocabulary/sea%20surface%20topography">
		<skos:prefLabel>SEA SURFACE TOPOGRAPHY</skos:prefLabel>
		<skos:broader rdf:resource="http://www.earthobservations.org/GEOSS/EO_Vocabulary/oceans"/>
		<skos:narrower rdf:resource="http://www.earthobservations.org/GEOSS/EO_Vocabulary/slope%20angle"/>
		<skos:inScheme rdf:resource="http://www.earthobservations.org/GEOSS/EO_Vocabulary"/>
	</skos:Concept>
	<skos:Concept rdf:about="http://www.earthobservations.org/GEOSS/EO_Vocabulary/aquatic%20ecosystems">
		<skos:prefLabel>AQUATIC ECOSYSTEMS</skos:prefLabel>
		<skos:broader rdf:resource="http://www.earthobservations.org/GEOSS/EO_Vocabulary/biosphere"/>
		<skos:narrower rdf:resource="http://www.earthobservations.org/GEOSS/EO_Vocabulary/water%20bodies%20%28location%29"/>
		<skos:narrower rdf:resource="http://www.earthobservations.org/GEOSS/EO_Vocabulary/fish%20harvest%20intensity"/>
		<skos:narrower rdf:resource="http://www.earthobservations.org/GEOSS/EO_Vocabulary/animal%20activity%20%28range%2C%20season%20length%2C%20migration%20patterns%29"/>
		<skos:narrower rdf:resource="http://www.earthobservations.org/GEOSS/EO_Vocabulary/coral%20reef%20classification%2Fmetabolism"/>
		<skos:inScheme rdf:resource="http://www.earthobservations.org/GEOSS/EO_Vocabulary"/>
	</skos:Concept>
	<skos:Concept rdf:about="http://www.earthobservations.org/GEOSS/EO_Vocabulary/forest%20science">
		<skos:prefLabel>FOREST SCIENCE</skos:prefLabel>
		<skos:broader rdf:resource="http://www.earthobservations.org/GEOSS/EO_Vocabulary/agriculture"/>
		<skos:narrower rdf:resource="http://www.earthobservations.org/GEOSS/EO_Vocabulary/forest%20management%20practices"/>
		<skos:narrower rdf:resource="http://www.earthobservations.org/GEOSS/EO_Vocabulary/forest%20structure"/>
		<skos:inScheme rdf:resource="http://www.earthobservations.org/GEOSS/EO_Vocabulary"/>
	</skos:Concept>
	<skos:Concept rdf:about="http://www.earthobservations.org/GEOSS/EO_Vocabulary/geodetics%2Fgravity">
		<skos:prefLabel>GEODETICS/GRAVITY</skos:prefLabel>
		<skos:broader rdf:resource="http://www.earthobservations.org/GEOSS/EO_Vocabulary/solid%20earth"/>
		<skos:narrower rdf:resource="http://www.earthobservations.org/GEOSS/EO_Vocabulary/surface%20deformation"/>
		<skos:narrower rdf:resource="http://www.earthobservations.org/GEOSS/EO_Vocabulary/surface%20deformation"/>
		<skos:narrower rdf:resource="http://www.earthobservations.org/GEOSS/EO_Vocabulary/gravity%20field"/>
		<skos:narrower rdf:resource="http://www.earthobservations.org/GEOSS/EO_Vocabulary/gravity%20field"/>
		<skos:inScheme rdf:resource="http://www.earthobservations.org/GEOSS/EO_Vocabulary"/>
	</skos:Concept>
	<skos:Concept rdf:about="http://www.earthobservations.org/GEOSS/EO_Vocabulary/geomorphology">
		<skos:prefLabel>GEOMORPHOLOGY</skos:prefLabel>
		<skos:broader rdf:resource="http://www.earthobservations.org/GEOSS/EO_Vocabulary/land%20surface"/>
		<skos:broader rdf:resource="http://www.earthobservations.org/GEOSS/EO_Vocabulary/solid%20earth"/>
		<skos:inScheme rdf:resource="http://www.earthobservations.org/GEOSS/EO_Vocabulary"/>
	</skos:Concept>
	<skos:Concept rdf:about="http://www.earthobservations.org/GEOSS/EO_Vocabulary/marine%20sediments">
		<skos:prefLabel>MARINE SEDIMENTS</skos:prefLabel>
		<skos:broader rdf:resource="http://www.earthobservations.org/GEOSS/EO_Vocabulary/oceans"/>
		<skos:narrower rdf:resource="http://www.earthobservations.org/GEOSS/EO_Vocabulary/pore%20pressure"/>
		<skos:inScheme rdf:resource="http://www.earthobservations.org/GEOSS/EO_Vocabulary"/>
	</skos:Concept>
	<skos:Concept rdf:about="http://www.earthobservations.org/GEOSS/EO_Vocabulary/rocks%2Fminerals%C2%A0">
		<skos:prefLabel>ROCKS/MINERALS </skos:prefLabel>
		<skos:broader rdf:resource="http://www.earthobservations.org/GEOSS/EO_Vocabulary/solid%20earth"/>
		<skos:narrower rdf:resource="http://www.earthobservations.org/GEOSS/EO_Vocabulary/rock%20strength%2C%20permeability%2C%20spacing%2C%20orientation"/>
		<skos:inScheme rdf:resource="http://www.earthobservations.org/GEOSS/EO_Vocabulary"/>
	</skos:Concept>
	<skos:Concept rdf:about="http://www.earthobservations.org/GEOSS/EO_Vocabulary/seismology">
		<skos:prefLabel>SEISMOLOGY</skos:prefLabel>
		<skos:broader rdf:resource="http://www.earthobservations.org/GEOSS/EO_Vocabulary/solid%20earth"/>
		<skos:narrower rdf:resource="http://www.earthobservations.org/GEOSS/EO_Vocabulary/slip"/>
		<skos:inScheme rdf:resource="http://www.earthobservations.org/GEOSS/EO_Vocabulary"/>
	</skos:Concept>
	<skos:Concept rdf:about="http://www.earthobservations.org/GEOSS/EO_Vocabulary/tectonics%C2%A0">
		<skos:prefLabel>TECTONICS </skos:prefLabel>
		<skos:broader rdf:resource="http://www.earthobservations.org/GEOSS/EO_Vocabulary/solid%20earth"/>
		<skos:narrower rdf:resource="http://www.earthobservations.org/GEOSS/EO_Vocabulary/strain"/>
		<skos:inScheme rdf:resource="http://www.earthobservations.org/GEOSS/EO_Vocabulary"/>
	</skos:Concept>
	<skos:Concept rdf:about="http://www.earthobservations.org/GEOSS/EO_Vocabulary/ocean%20waves">
		<skos:prefLabel>OCEAN WAVES</skos:prefLabel>
		<skos:broader rdf:resource="http://www.earthobservations.org/GEOSS/EO_Vocabulary/oceans"/>
		<skos:narrower rdf:resource="http://www.earthobservations.org/GEOSS/EO_Vocabulary/wave%20direction"/>
		<skos:narrower rdf:resource="http://www.earthobservations.org/GEOSS/EO_Vocabulary/wave%20height"/>
		<skos:narrower rdf:resource="http://www.earthobservations.org/GEOSS/EO_Vocabulary/wave%20period"/>
		<skos:inScheme rdf:resource="http://www.earthobservations.org/GEOSS/EO_Vocabulary"/>
	</skos:Concept>
	<skos:Concept rdf:about="http://www.earthobservations.org/GEOSS/EO_Vocabulary/boundaries">
		<skos:prefLabel>BOUNDARIES</skos:prefLabel>
		<skos:broader rdf:resource="http://www.earthobservations.org/GEOSS/EO_Vocabulary/human%20dimensions"/>
		<skos:narrower rdf:resource="http://www.earthobservations.org/GEOSS/EO_Vocabulary/vector%20population"/>
		<skos:inScheme rdf:resource="http://www.earthobservations.org/GEOSS/EO_Vocabulary"/>
	</skos:Concept>
	<skos:Concept rdf:about="http://www.earthobservations.org/GEOSS/EO_Vocabulary/natural%20resources">
		<skos:prefLabel>NATURAL RESOURCES </skos:prefLabel>
		<skos:broader rdf:resource="http://www.earthobservations.org/GEOSS/EO_Vocabulary/solid%20earth"/>
		<skos:narrower rdf:resource="http://www.earthobservations.org/GEOSS/EO_Vocabulary/fuel%20load%2Fcharacteristics"/>
		<skos:inScheme rdf:resource="http://www.earthobservations.org/GEOSS/EO_Vocabulary"/>
	</skos:Concept>
	<skos:Concept rdf:about="http://www.earthobservations.org/GEOSS/EO_Vocabulary/human%20health">
		<skos:prefLabel>HUMAN HEALTH</skos:prefLabel>
		<skos:broader rdf:resource="http://www.earthobservations.org/GEOSS/EO_Vocabulary/human%20dimensions"/>
		<skos:narrower rdf:resource="http://www.earthobservations.org/GEOSS/EO_Vocabulary/source%20of%20drinking%20water"/>
		<skos:narrower rdf:resource="http://www.earthobservations.org/GEOSS/EO_Vocabulary/density%20of%20animal%20hosts"/>
		<skos:narrower rdf:resource="http://www.earthobservations.org/GEOSS/EO_Vocabulary/health%20care%20access"/>
		<skos:narrower rdf:resource="http://www.earthobservations.org/GEOSS/EO_Vocabulary/pathogen%20population%20dynamic"/>
		<skos:inScheme rdf:resource="http://www.earthobservations.org/GEOSS/EO_Vocabulary"/>
	</skos:Concept>
	<skos:Concept rdf:about="http://www.earthobservations.org/GEOSS/EO_Vocabulary/water%C2%A0quality%2Fwater%20chemistry">
		<skos:prefLabel>WATER QUALITY/WATER CHEMISTRY</skos:prefLabel>
		<skos:broader rdf:resource="http://www.earthobservations.org/GEOSS/EO_Vocabulary/terrestrial%20hydrosphere"/>
		<skos:narrower rdf:resource="http://www.earthobservations.org/GEOSS/EO_Vocabulary/ecosystem%20demand%20for%20water"/>
		<skos:inScheme rdf:resource="http://www.earthobservations.org/GEOSS/EO_Vocabulary"/>
	</skos:Concept>
	<skos:Concept rdf:about="http://www.earthobservations.org/GEOSS/EO_Vocabulary/air%20quality">
		<skos:prefLabel>AIR QUALITY</skos:prefLabel>
		<skos:broader rdf:resource="http://www.earthobservations.org/GEOSS/EO_Vocabulary/atmosphere"/>
		<skos:narrower rdf:resource="http://www.earthobservations.org/GEOSS/EO_Vocabulary/suspended%20particulates%2Fturbidity%2Fwater%20attenuation%20coefficient"/>
		<skos:narrower rdf:resource="http://www.earthobservations.org/GEOSS/EO_Vocabulary/suspended%20particulates%2Fturbidity%2Fwater%20attenuation%20coefficient"/>
		<skos:narrower rdf:resource="http://www.earthobservations.org/GEOSS/EO_Vocabulary/ambient%20volatile%20organic%20compounds"/>
		<skos:narrower rdf:resource="http://www.earthobservations.org/GEOSS/EO_Vocabulary/other%20long-lived%20ghgs"/>
		<skos:inScheme rdf:resource="http://www.earthobservations.org/GEOSS/EO_Vocabulary"/>
	</skos:Concept>
	<skos:Concept rdf:about="http://www.earthobservations.org/GEOSS/EO_Vocabulary/animals%2Fvertebrates">
		<skos:prefLabel>ANIMALS/VERTEBRATES</skos:prefLabel>
		<skos:broader rdf:resource="http://www.earthobservations.org/GEOSS/EO_Vocabulary/biological%20classification"/>
		<skos:inScheme rdf:resource="http://www.earthobservations.org/GEOSS/EO_Vocabulary"/>
	</skos:Concept>
	<skos:Concept rdf:about="http://www.earthobservations.org/GEOSS/EO_Vocabulary/animal%20science">
		<skos:prefLabel>ANIMAL SCIENCE</skos:prefLabel>
		<skos:broader rdf:resource="http://www.earthobservations.org/GEOSS/EO_Vocabulary/agriculture"/>
		<skos:inScheme rdf:resource="http://www.earthobservations.org/GEOSS/EO_Vocabulary"/>
	</skos:Concept>
	<skos:Concept rdf:about="http://www.earthobservations.org/GEOSS/EO_Vocabulary/aquatic%20sciences">
		<skos:prefLabel>AQUATIC SCIENCES</skos:prefLabel>
		<skos:broader rdf:resource="http://www.earthobservations.org/GEOSS/EO_Vocabulary/oceans"/>
		<skos:narrower rdf:resource="http://www.earthobservations.org/GEOSS/EO_Vocabulary/aquatic%20ecosystem%20condition"/>
		<skos:inScheme rdf:resource="http://www.earthobservations.org/GEOSS/EO_Vocabulary"/>
	</skos:Concept>
	<skos:Concept rdf:about="http://www.earthobservations.org/GEOSS/EO_Vocabulary/agricultural%20aquatic%20sciences">
		<skos:prefLabel>AGRICULTURAL AQUATIC SCIENCES</skos:prefLabel>
		<skos:broader rdf:resource="http://www.earthobservations.org/GEOSS/EO_Vocabulary/agriculture"/>
		<skos:narrower rdf:resource="http://www.earthobservations.org/GEOSS/EO_Vocabulary/aquatic%20ecosystem%20condition"/>
		<skos:inScheme rdf:resource="http://www.earthobservations.org/GEOSS/EO_Vocabulary"/>
	</skos:Concept>
	<skos:Concept rdf:about="http://www.earthobservations.org/GEOSS/EO_Vocabulary/plant%20commodities">
		<skos:prefLabel>PLANT COMMODITIES</skos:prefLabel>
		<skos:broader rdf:resource="http://www.earthobservations.org/GEOSS/EO_Vocabulary/agriculture"/>
		<skos:narrower rdf:resource="http://www.earthobservations.org/GEOSS/EO_Vocabulary/crop%20emergence"/>
		<skos:inScheme rdf:resource="http://www.earthobservations.org/GEOSS/EO_Vocabulary"/>
	</skos:Concept>
	<skos:Concept rdf:about="http://www.earthobservations.org/GEOSS/EO_Vocabulary/land%20use%2Fland%C2%A0cover">
		<skos:prefLabel>LAND USE/LAND COVER</skos:prefLabel>
		<skos:broader rdf:resource="http://www.earthobservations.org/GEOSS/EO_Vocabulary/human%20dimensions"/>
		<skos:narrower rdf:resource="http://www.earthobservations.org/GEOSS/EO_Vocabulary/field%20cover%20%28continuous%29"/>
		<skos:inScheme rdf:resource="http://www.earthobservations.org/GEOSS/EO_Vocabulary"/>
	</skos:Concept>
	<skos:Concept rdf:about="http://www.earthobservations.org/GEOSS/EO_Vocabulary/marine%20geophysics">
		<skos:prefLabel>MARINE GEOPHYSICS</skos:prefLabel>
		<skos:broader rdf:resource="http://www.earthobservations.org/GEOSS/EO_Vocabulary/oceans"/>
		<skos:inScheme rdf:resource="http://www.earthobservations.org/GEOSS/EO_Vocabulary"/>
	</skos:Concept>
	<skos:Concept rdf:about="http://www.earthobservations.org/GEOSS/EO_Vocabulary/attitudes%2Cpreferences%2Cbehavior">
		<skos:prefLabel>ATTITUDES,PREFERENCES,BEHAVIOR</skos:prefLabel>
		<skos:broader rdf:resource="http://www.earthobservations.org/GEOSS/EO_Vocabulary/human%20dimensions"/>
		<skos:narrower rdf:resource="http://www.earthobservations.org/GEOSS/EO_Vocabulary/health%20care%20access"/>
		<skos:inScheme rdf:resource="http://www.earthobservations.org/GEOSS/EO_Vocabulary"/>
	</skos:Concept>
	<skos:Concept rdf:about="http://www.earthobservations.org/GEOSS/EO_Vocabulary/geomagnetism">
		<skos:prefLabel>GEOMAGNETISM</skos:prefLabel>
		<skos:broader rdf:resource="http://www.earthobservations.org/GEOSS/EO_Vocabulary/solid%20earth"/>
		<skos:narrower rdf:resource="http://www.earthobservations.org/GEOSS/EO_Vocabulary/magnetic%20field"/>
		<skos:inScheme rdf:resource="http://www.earthobservations.org/GEOSS/EO_Vocabulary"/>
	</skos:Concept>
	<skos:Concept rdf:about="http://www.earthobservations.org/GEOSS/EO_Vocabulary/bacteria%2Farchaea">
		<skos:prefLabel>BACTERIA/ARCHAEA</skos:prefLabel>
		<skos:broader rdf:resource="http://www.earthobservations.org/GEOSS/EO_Vocabulary/biological%20classification"/>
		<skos:narrower rdf:resource="http://www.earthobservations.org/GEOSS/EO_Vocabulary/water%20algal%20blooms"/>
		<skos:inScheme rdf:resource="http://www.earthobservations.org/GEOSS/EO_Vocabulary"/>
	</skos:Concept>
	<skos:Concept rdf:about="http://www.earthobservations.org/GEOSS/EO_Vocabulary/plants">
		<skos:prefLabel>PLANTS</skos:prefLabel>
		<skos:broader rdf:resource="http://www.earthobservations.org/GEOSS/EO_Vocabulary/biological%20classification"/>
		<skos:narrower rdf:resource="http://www.earthobservations.org/GEOSS/EO_Vocabulary/water%20algal%20blooms"/>
		<skos:inScheme rdf:resource="http://www.earthobservations.org/GEOSS/EO_Vocabulary"/>
	</skos:Concept>
	<skos:Concept rdf:about="http://www.earthobservations.org/GEOSS/EO_Vocabulary/ground%20water">
		<skos:prefLabel>GROUND WATER</skos:prefLabel>
		<skos:broader rdf:resource="http://www.earthobservations.org/GEOSS/EO_Vocabulary/terrestrial%20hydrosphere"/>
		<skos:narrower rdf:resource="http://www.earthobservations.org/GEOSS/EO_Vocabulary/water%20infiltration%2Fpercolation-land%20surface"/>
		<skos:narrower rdf:resource="http://www.earthobservations.org/GEOSS/EO_Vocabulary/water%20infiltration%2Fpercolation-land%20surface"/>
		<skos:inScheme rdf:resource="http://www.earthobservations.org/GEOSS/EO_Vocabulary"/>
	</skos:Concept>
	<skos:Concept rdf:about="http://www.earthobservations.org/GEOSS/EO_Vocabulary/precipitation">
		<skos:prefLabel>Precipitation</skos:prefLabel>
		<skos:definition>1) Liquid or solid products of the condensation of water vapour falling from clouds or deposited from air on the ground.(2) Amount of precipitation (as defined under (1)) on a unit of horizontal surface per unit time.</skos:definition>
		<skos:scopeNote>UNESCO</skos:scopeNote>
		<skos:broader rdf:resource="http://www.earthobservations.org/GEOSS/EO_Vocabulary/atmosphere"/>
		<rdfs:seeAlso rdf:resource="http://webworld.unesco.org/water/ihp/db/glossary/glu/EN/GF0933EN.HTM"/>
		<rdfs:seeAlso rdf:resource="http://gcmd.nasa.gov/Resources/valids/archives/keyword_list.html"/>
		<skos:inScheme rdf:resource="http://www.earthobservations.org/GEOSS/EO_Vocabulary"/>
	</skos:Concept>
	<skos:Concept rdf:about="http://www.earthobservations.org/GEOSS/EO_Vocabulary/soil%20moisture">
		<skos:prefLabel>Soil Moisture</skos:prefLabel>
		<skos:definition>Moisture contained in the portion of the soil which is above the water table, including water vapour, which is present in the soil pores.</skos:definition>
		<skos:scopeNote>UNESCO</skos:scopeNote>
		<skos:broader rdf:resource="http://www.earthobservations.org/GEOSS/EO_Vocabulary/soils"/>
		<skos:broader rdf:resource="http://www.earthobservations.org/GEOSS/EO_Vocabulary/soils"/>
		<rdfs:seeAlso rdf:resource="http://cf-pcmdi.llnl.gov/documents/cf-standard-names/standard-name-table/17/cf-standard-name-table.html"/>
		<rdfs:seeAlso rdf:resource="http://webworld.unesco.org/water/ihp/db/glossary/glu/EN/GF1151EN.HTM"/>
		<rdfs:seeAlso rdf:resource="http://gcmd.nasa.gov/Resources/valids/archives/keyword_list.html"/>
		<skos:inScheme rdf:resource="http://www.earthobservations.org/GEOSS/EO_Vocabulary"/>
	</skos:Concept>
	<skos:Concept rdf:about="http://www.earthobservations.org/GEOSS/EO_Vocabulary/surface%20air%20temperature">
		<skos:prefLabel>Surface Air Temperature</skos:prefLabel>
		<skos:definition>The temperature of the atmosphere which represents the average kinetic energy of the molecular motion in a small region and is defined in terms of a standard or calibrated thermometer in thermal equilibrium with the air. (Source: MGH)</skos:definition>
		<skos:scopeNote>GEMET</skos:scopeNote>
		<skos:broader rdf:resource="http://www.earthobservations.org/GEOSS/EO_Vocabulary/atmospheric%20temperature"/>
		<rdfs:seeAlso rdf:resource="http://cf-pcmdi.llnl.gov/documents/cf-standard-names/standard-name-table/17/cf-standard-name-table.html "/>
		<rdfs:seeAlso rdf:resource="http://gcmd.nasa.gov/Resources/valids/archives/keyword_list.html"/>
		<skos:inScheme rdf:resource="http://www.earthobservations.org/GEOSS/EO_Vocabulary"/>
	</skos:Concept>
	<skos:Concept rdf:about="http://www.earthobservations.org/GEOSS/EO_Vocabulary/surface%20wind%20speed">
		<skos:prefLabel>Surface Wind Speed</skos:prefLabel>
		<skos:definition>The motion of air relative to the earths surface; usually means horizontal air motion, as distinguished from vertical motion. (Source: MGH)</skos:definition>
		<skos:scopeNote>GEMET</skos:scopeNote>
		<skos:broader rdf:resource="http://www.earthobservations.org/GEOSS/EO_Vocabulary/atmospheric%20winds"/>
		<skos:broader rdf:resource="http://www.earthobservations.org/GEOSS/EO_Vocabulary/ocean%20winds"/>
		<skos:inScheme rdf:resource="http://www.earthobservations.org/GEOSS/EO_Vocabulary"/>
	</skos:Concept>
	<skos:Concept rdf:about="http://www.earthobservations.org/GEOSS/EO_Vocabulary/land%20cover">
		<skos:prefLabel>Land Cover</skos:prefLabel>
		<skos:definition>Land cover is the physical state of the land surface. It is the combination of vegetation, soil, rock, water and human-made structures, which make up the earths landscape. The land cover is the interface between the earths crust and the atmosphere, influencing the exchange of energy and matter in the climatic system and biogeochemical cycles. (Source: BRS)</skos:definition>
		<skos:scopeNote>GEMET</skos:scopeNote>
		<skos:broader rdf:resource="http://www.earthobservations.org/GEOSS/EO_Vocabulary/land%20use%2Fland%20cover"/>
		<skos:broader rdf:resource="http://www.earthobservations.org/GEOSS/EO_Vocabulary/land%20use%2Fland%20cover"/>
		<rdfs:seeAlso rdf:resource="http://gcmd.nasa.gov/Resources/valids/archives/keyword_list.html"/>
		<rdfs:seeAlso rdf:resource="http://gcmd.nasa.gov/Resources/valids/archives/keyword_list.html"/>
		<rdfs:seeAlso rdf:resource="http://gcmd.nasa.gov/Resources/valids/archives/keyword_list.html"/>
		<skos:inScheme rdf:resource="http://www.earthobservations.org/GEOSS/EO_Vocabulary"/>
	</skos:Concept>
	<skos:Concept rdf:about="http://www.earthobservations.org/GEOSS/EO_Vocabulary/surface%20humidity">
		<skos:prefLabel>Surface Humidity</skos:prefLabel>
		<skos:definition>The surface called "surface" means the lower boundary of the atmosphere. "specific" means per unit mass. Specific humidity is the mass fraction of water vapor in (moist) air. 1</skos:definition>
		<skos:scopeNote>CF Standard Names</skos:scopeNote>
		<skos:broader rdf:resource="http://www.earthobservations.org/GEOSS/EO_Vocabulary/atmospheric%20water%20vapor"/>
		<rdfs:seeAlso rdf:resource="http://sweet.jpl.nasa.gov/"/>
		<rdfs:seeAlso rdf:resource="http://gcmd.nasa.gov/Resources/valids/archives/keyword_list.html"/>
		<rdfs:seeAlso rdf:resource="http://cf-pcmdi.llnl.gov/documents/cf-standard-names/standard-name-table/17/cf-standard-name-table.html "/>
		<rdfs:seeAlso rdf:resource="http://webworld.unesco.org/water/ihp/db/glossary/glu/EN/GF0031EN.HTM"/>
		<rdfs:seeAlso rdf:resource="http://webworld.unesco.org/water/ihp/db/glossary/glu/EN/GF0033EN.HTM"/>
		<skos:inScheme rdf:resource="http://www.earthobservations.org/GEOSS/EO_Vocabulary"/>
	</skos:Concept>
	<skos:Concept rdf:about="http://www.earthobservations.org/GEOSS/EO_Vocabulary/vegetation%20cover">
		<skos:prefLabel>Vegetation Cover</skos:prefLabel>
		<skos:definition>Number of plants growing on a certain area of land. (Source: PHC) </skos:definition>
		<skos:scopeNote>GEMET</skos:scopeNote>
		<skos:broader rdf:resource="http://www.earthobservations.org/GEOSS/EO_Vocabulary/vegetation"/>
		<rdfs:seeAlso rdf:resource="http://cf-pcmdi.llnl.gov/documents/cf-standard-names/standard-name-table/17/cf-standard-name-table.html "/>
		<rdfs:seeAlso rdf:resource="http://gcmd.nasa.gov/Resources/valids/archives/keyword_list.html"/>
		<skos:inScheme rdf:resource="http://www.earthobservations.org/GEOSS/EO_Vocabulary"/>
	</skos:Concept>
	<skos:Concept rdf:about="http://www.earthobservations.org/GEOSS/EO_Vocabulary/surface%20wind%20direction">
		<skos:prefLabel>Surface Wind Direction</skos:prefLabel>
		<skos:definition>Wind is defined as a two-dimensional (horizontal) air velocity vector, with no vertical component. (Vertical motion in the atmosphere has the standard name upward_air_velocity.) In meteorological reports, the direction of the wind vector is usually (but not always) given as the direction from which it is blowing (wind_from_direction) (westerly, northerly, etc.). In other contexts, such as atmospheric modelling, it is often natural to give the direction in the usual manner of vectors as the heading or the direction to which it is blowing (wind_to_direction) (eastward, southward, etc.) "from_direction" is used in the construction X_from_direction and indicates the direction from which the velocity vector of X is coming.</skos:definition>
		<skos:scopeNote>CF Standard Names</skos:scopeNote>
		<skos:broader rdf:resource="http://www.earthobservations.org/GEOSS/EO_Vocabulary/atmospheric%20winds"/>
		<skos:broader rdf:resource="http://www.earthobservations.org/GEOSS/EO_Vocabulary/ocean%20winds"/>
		<rdfs:seeAlso rdf:resource="http://cf-pcmdi.llnl.gov/documents/cf-standard-names/standard-name-table/17/cf-standard-name-table.html"/>
		<rdfs:seeAlso rdf:resource="http://cf-pcmdi.llnl.gov/documents/cf-standard-names/standard-name-table/17/cf-standard-name-table.html"/>
		<rdfs:seeAlso rdf:resource="http://gcmd.nasa.gov/Resources/valids/archives/keyword_list.html"/>
		<rdfs:seeAlso rdf:resource="http://gcmd.nasa.gov/Resources/valids/archives/keyword_list.html"/>
		<skos:inScheme rdf:resource="http://www.earthobservations.org/GEOSS/EO_Vocabulary"/>
	</skos:Concept>
	<skos:Concept rdf:about="http://www.earthobservations.org/GEOSS/EO_Vocabulary/normalized%20difference%20vegetation%20index%20%28ndvi%29">
		<skos:prefLabel>Normalized Difference Vegetation Index (NDVI)</skos:prefLabel>
		<skos:definition>"Normalized_difference_vegetation_index", usually abbreviated to NDVI, is an index calculated from reflectances measured in the visible and near infrared channels. It is calculated as NDVI = (NIR - R) / (NIR + R) where NIR is the reflectance in the near-infrared band and R is the reflectance in the red visible band. Reflectance is the ratio of the reflected over the incoming radiation in each spectral band. The calculated value of NDVI depends on the precise definitions of the spectral bands and these definitions may vary between different models and remote sensing instruments.</skos:definition>
		<skos:scopeNote>CF Standard Names</skos:scopeNote>
		<skos:broader rdf:resource="http://www.earthobservations.org/GEOSS/EO_Vocabulary/vegetation"/>
		<rdfs:seeAlso rdf:resource="http://cf-pcmdi.llnl.gov/documents/cf-standard-names/standard-name-table/17/cf-standard-name-table.html"/>
		<skos:inScheme rdf:resource="http://www.earthobservations.org/GEOSS/EO_Vocabulary"/>
	</skos:Concept>
	<skos:Concept rdf:about="http://www.earthobservations.org/GEOSS/EO_Vocabulary/sea%20surface%20temperature">
		<skos:prefLabel>Sea Surface Temperature</skos:prefLabel>
		<skos:definition>Sea surface temperature is usually abbreviated as "SST". It is the temperature of sea water near the surface (including the part under sea-ice, if any), and not the skin temperature, whose standard name is surface_temperature. For the temperature of sea water at a particular depth or layer, a data variable of sea_water_temperature with a vertical coordinate axis should be used.</skos:definition>
		<skos:scopeNote>CF Standard Names</skos:scopeNote>
		<skos:broader rdf:resource="http://www.earthobservations.org/GEOSS/EO_Vocabulary/ocean%20temperature"/>
		<rdfs:seeAlso rdf:resource="http://cf-pcmdi.llnl.gov/documents/cf-standard-names/standard-name-table/17/cf-standard-name-table.html"/>
		<rdfs:seeAlso rdf:resource="http://gcmd.nasa.gov/Resources/valids/archives/keyword_list.html"/>
		<skos:inScheme rdf:resource="http://www.earthobservations.org/GEOSS/EO_Vocabulary"/>
	</skos:Concept>
	<skos:Concept rdf:about="http://www.earthobservations.org/GEOSS/EO_Vocabulary/urbanization">
		<skos:prefLabel>Urbanization</skos:prefLabel>
		<skos:definition>Urbanization is the expansion of metropolitan areas by building housing developments and shopping centers farther and farther from urban centers and lacing them together with more major highways. An outcome of urbanization is the fact that as more highways are built, surfaces are sealed with pavement, increasing stormwater runoff and quickening concentration times.</skos:definition>
		<skos:scopeNote>GCMD</skos:scopeNote>
		<skos:broader rdf:resource="http://www.earthobservations.org/GEOSS/EO_Vocabulary/environmental%20impacts"/>
		<rdfs:seeAlso rdf:resource="http://gcmd.nasa.gov/Resources/valids/archives/keyword_list.html"/>
		<skos:inScheme rdf:resource="http://www.earthobservations.org/GEOSS/EO_Vocabulary"/>
	</skos:Concept>
	<skos:Concept rdf:about="http://www.earthobservations.org/GEOSS/EO_Vocabulary/vegetation%20type">
		<skos:prefLabel>Vegetation Type</skos:prefLabel>
		<skos:definition>A community of plants or plant life that share distinguishable characteristics. (Source: PEM) </skos:definition>
		<skos:scopeNote>GEMET</skos:scopeNote>
		<skos:broader rdf:resource="http://www.earthobservations.org/GEOSS/EO_Vocabulary/vegetation"/>
		<skos:inScheme rdf:resource="http://www.earthobservations.org/GEOSS/EO_Vocabulary"/>
	</skos:Concept>
	<skos:Concept rdf:about="http://www.earthobservations.org/GEOSS/EO_Vocabulary/land%20surface%20temperature">
		<skos:prefLabel>Land Surface Temperature</skos:prefLabel>
		<skos:definition>The surface called "surface" means the lower boundary of the atmosphere. The surface temperature is the temperature at the interface, not the bulk temperature of the medium above or below. Unless indicated in the cell_methods attribute, a quantity is assumed to apply to the whole area of each horizontal grid box. Previously, the qualifier where_type was used to specify that the quantity applies only to the part of the grid box of the named type. Names containing the where_type qualifier are deprecated and newly created data should use the cell_methods attribute to indicate the horizontal area to which the quantity applies. K E139 ts</skos:definition>
		<skos:scopeNote>CF Standard Names</skos:scopeNote>
		<skos:broader rdf:resource="http://www.earthobservations.org/GEOSS/EO_Vocabulary/land%20temperature"/>
		<rdfs:seeAlso rdf:resource="http://cf-pcmdi.llnl.gov/documents/cf-standard-names/standard-name-table/17/cf-standard-name-table.html"/>
		<rdfs:seeAlso rdf:resource="http://gcmd.nasa.gov/Resources/valids/archives/keyword_list.html"/>
		<skos:inScheme rdf:resource="http://www.earthobservations.org/GEOSS/EO_Vocabulary"/>
	</skos:Concept>
	<skos:Concept rdf:about="http://www.earthobservations.org/GEOSS/EO_Vocabulary/surface%20atmospheric%20pressure">
		<skos:prefLabel>Surface Atmospheric Pressure</skos:prefLabel>
		<skos:altLabel>Surface Pressure</skos:altLabel>
		<skos:definition>A type of stress which is exerted uniformly in all directions; its measure is the force exerted per unit area. (Source: MGH) </skos:definition>
		<skos:scopeNote>GEMET</skos:scopeNote>
		<skos:broader rdf:resource="http://www.earthobservations.org/GEOSS/EO_Vocabulary/atmospheric%20pressure"/>
		<rdfs:seeAlso rdf:resource="http://cf-pcmdi.llnl.gov/documents/cf-standard-names/standard-name-table/17/cf-standard-name-table.html "/>
		<rdfs:seeAlso rdf:resource="http://gcmd.nasa.gov/Resources/valids/archives/keyword_list.html"/>
		<skos:inScheme rdf:resource="http://www.earthobservations.org/GEOSS/EO_Vocabulary"/>
	</skos:Concept>
	<skos:Concept rdf:about="http://www.earthobservations.org/GEOSS/EO_Vocabulary/leaf%20area%20index%20%28lai%29">
		<skos:prefLabel>Leaf Area Index (LAI)</skos:prefLabel>
		<skos:definition>The area of foliage per unit area of ground. Conventionally this refers　to the ratio of the area of the upper side of the leaves in a canopy　projected onto a flat surface to the area of the surface under the　canopy. Occasionally this has been used in reference to both sides of the leaves.
</skos:definition>
		<skos:scopeNote>NASA Earth Observatory Glossary</skos:scopeNote>
		<skos:broader rdf:resource="http://www.earthobservations.org/GEOSS/EO_Vocabulary/vegetation"/>
		<rdfs:seeAlso rdf:resource="http://cf-pcmdi.llnl.gov/documents/cf-standard-names/standard-name-table/17/cf-standard-name-table.html"/>
		<rdfs:seeAlso rdf:resource="http://earthobservatory.nasa.gov/Glossary/?mode=alpha&amp;seg=l&amp;segend=n"/>
		<skos:inScheme rdf:resource="http://www.earthobservations.org/GEOSS/EO_Vocabulary"/>
	</skos:Concept>
	<skos:Concept rdf:about="http://www.earthobservations.org/GEOSS/EO_Vocabulary/glacier%2Fice%20sheet%20extent">
		<skos:prefLabel>Glacier/ice Sheet Extent</skos:prefLabel>
		<skos:definition>Slow moving masses of ice which have accumulated either on mountains or in polar regions. They are found where warm, moist air or warm water meets cold air or water. They move, influenced by the force of gravity and the pressure of the ice, above the underlying slush layers and slide downhill, eventually melting at lower levels to form rivers or reaching sea-level, where they form ice shelves or fall into the water as icebergs. (Source: WRIGHT) </skos:definition>
		<skos:scopeNote>GEMET</skos:scopeNote>
		<skos:broader rdf:resource="http://www.earthobservations.org/GEOSS/EO_Vocabulary/frozen%20ground"/>
		<skos:broader rdf:resource="http://www.earthobservations.org/GEOSS/EO_Vocabulary/sea%20ice"/>
		<skos:broader rdf:resource="http://www.earthobservations.org/GEOSS/EO_Vocabulary/glaciers%2Fice%20sheets"/>
		<skos:broader rdf:resource="http://www.earthobservations.org/GEOSS/EO_Vocabulary/snow%2Fice"/>
		<skos:broader rdf:resource="http://www.earthobservations.org/GEOSS/EO_Vocabulary/frozen%20ground"/>
		<skos:broader rdf:resource="http://www.earthobservations.org/GEOSS/EO_Vocabulary/glaciers%2Fice%20sheets"/>
		<skos:broader rdf:resource="http://www.earthobservations.org/GEOSS/EO_Vocabulary/sea%20ice"/>
		<skos:broader rdf:resource="http://www.earthobservations.org/GEOSS/EO_Vocabulary/snow%2Fice"/>
		<rdfs:seeAlso rdf:resource="http://inspire-registry.jrc.ec.europa.eu/"/>
		<rdfs:seeAlso rdf:resource="http://sweet.jpl.nasa.gov/ "/>
		<rdfs:seeAlso rdf:resource="http://cf-pcmdi.llnl.gov/documents/cf-standard-names/standard-name-table/17/cf-standard-name-table.html"/>
		<rdfs:seeAlso rdf:resource="http://cf-pcmdi.llnl.gov/documents/cf-standard-names/standard-name-table/17/cf-standard-name-table.html"/>
		<skos:inScheme rdf:resource="http://www.earthobservations.org/GEOSS/EO_Vocabulary"/>
	</skos:Concept>
	<skos:Concept rdf:about="http://www.earthobservations.org/GEOSS/EO_Vocabulary/upper%20level%20humidity">
		<skos:prefLabel>Upper Level Humidity</skos:prefLabel>
		<skos:definition>A measurable quantity of the moisture content found in the earths atmosphere. (Source: RHW) </skos:definition>
		<skos:scopeNote>GEMET</skos:scopeNote>
		<skos:broader rdf:resource="http://www.earthobservations.org/GEOSS/EO_Vocabulary/atmospheric%20water%20vapor"/>
		<rdfs:seeAlso rdf:resource="http://gcmd.nasa.gov/Resources/valids/archives/keyword_list.html"/>
		<skos:inScheme rdf:resource="http://www.earthobservations.org/GEOSS/EO_Vocabulary"/>
	</skos:Concept>
	<skos:Concept rdf:about="http://www.earthobservations.org/GEOSS/EO_Vocabulary/elevation">
		<skos:prefLabel>Elevation</skos:prefLabel>
		<skos:definition>The theme includes: • Terrestrial elevation, generally represented as - the terrain data, ground surface topography, called Digital Terrain Model describing the threedimensional shape of the Earth's surface - the surface data, named Digital Elevation Model, including the three dimensional shape of every feature placed on the soil (buildings, bridges, trees, ...). • Bathymetry, e.g. a gridded bottom model </skos:definition>
		<skos:scopeNote>INSPIRE Registry </skos:scopeNote>
		<skos:broader rdf:resource="http://www.earthobservations.org/GEOSS/EO_Vocabulary/topography"/>
		<skos:broader rdf:resource="http://www.earthobservations.org/GEOSS/EO_Vocabulary/sea%20ice"/>
		<skos:broader rdf:resource="http://www.earthobservations.org/GEOSS/EO_Vocabulary/sea%20ice"/>
		<rdfs:seeAlso rdf:resource="http://gcmd.nasa.gov/Resources/valids/archives/keyword_list.html"/>
		<skos:inScheme rdf:resource="http://www.earthobservations.org/GEOSS/EO_Vocabulary"/>
	</skos:Concept>
	<skos:Concept rdf:about="http://www.earthobservations.org/GEOSS/EO_Vocabulary/river%20flow%20observations">
		<skos:prefLabel>River Flow Observations</skos:prefLabel>
		<skos:altLabel>Runoff</skos:altLabel>
		<skos:definition>Rate at which water is removed by flowing over the soil surface. This rate is determined by the texture of the soil, slope, climate, and land use cover (e.g. paved surface, grass, forest, bare soil). (Source: LANDY)</skos:definition>
		<skos:scopeNote>GEMET</skos:scopeNote>
		<skos:broader rdf:resource="http://www.earthobservations.org/GEOSS/EO_Vocabulary/surface%20water"/>
		<rdfs:seeAlso rdf:resource="http://sweet.jpl.nasa.gov/"/>
		<rdfs:seeAlso rdf:resource="http://webworld.unesco.org/water/ihp/db/glossary/glu/EN/GF1049EN.HTM"/>
		<rdfs:seeAlso rdf:resource="http://gcmd.nasa.gov/Resources/valids/archives/keyword_list.html"/>
		<skos:inScheme rdf:resource="http://www.earthobservations.org/GEOSS/EO_Vocabulary"/>
	</skos:Concept>
	<skos:Concept rdf:about="http://www.earthobservations.org/GEOSS/EO_Vocabulary/upper%20level%20winds">
		<skos:prefLabel>Upper Level Winds</skos:prefLabel>
		<skos:definition>The motion of air relative to the earth's surface; usually means horizontal air motion, as distinguished from vertical motion. (Source: MGH)</skos:definition>
		<skos:scopeNote>GEMET</skos:scopeNote>
		<skos:broader rdf:resource="http://www.earthobservations.org/GEOSS/EO_Vocabulary/atmospheric%20winds"/>
		<rdfs:seeAlso rdf:resource="http://gcmd.nasa.gov/Resources/valids/archives/keyword_list.html"/>
		<skos:inScheme rdf:resource="http://www.earthobservations.org/GEOSS/EO_Vocabulary"/>
	</skos:Concept>
	<skos:Concept rdf:about="http://www.earthobservations.org/GEOSS/EO_Vocabulary/land%20use">
		<skos:prefLabel>Land Use</skos:prefLabel>
		<skos:definition>The term land use deals with the spatial aspects of all human activities on the land and with the way in which theLAND SURFACE is adapted, or could be adapted, to serve human needs. (Source: GOOD)</skos:definition>
		<skos:scopeNote>GEMET</skos:scopeNote>
		<skos:broader rdf:resource="http://www.earthobservations.org/GEOSS/EO_Vocabulary/land%20use%2Fland%20cover"/>
		<skos:broader rdf:resource="http://www.earthobservations.org/GEOSS/EO_Vocabulary/land%20use%2Fland%20cover"/>
		<rdfs:seeAlso rdf:resource="http://gcmd.nasa.gov/Resources/valids/archives/keyword_list.html"/>
		<rdfs:seeAlso rdf:resource="http://gcmd.nasa.gov/Resources/valids/archives/keyword_list.html"/>
		<skos:inScheme rdf:resource="http://www.earthobservations.org/GEOSS/EO_Vocabulary"/>
	</skos:Concept>
	<skos:Concept rdf:about="http://www.earthobservations.org/GEOSS/EO_Vocabulary/upper%20level%20temperature">
		<skos:prefLabel>Upper Level Temperature</skos:prefLabel>
		<skos:definition>The temperature of the atmosphere which represents the average kinetic energy of the molecular motion in a small region and is defined in terms of a standard or calibrated thermometer in thermal equilibrium with the air. (Source: MGH)</skos:definition>
		<skos:scopeNote>GEMET</skos:scopeNote>
		<skos:broader rdf:resource="http://www.earthobservations.org/GEOSS/EO_Vocabulary/atmospheric%20temperature"/>
		<rdfs:seeAlso rdf:resource="http://www.eionet.europa.eu/gemet/concept/8366"/>
		<rdfs:seeAlso rdf:resource="http://gcmd.nasa.gov/Resources/valids/archives/keyword_list.html"/>
		<rdfs:seeAlso rdf:resource="http://gcmd.nasa.gov/Resources/valids/archives/keyword_list.html"/>
		<skos:inScheme rdf:resource="http://www.earthobservations.org/GEOSS/EO_Vocabulary"/>
	</skos:Concept>
	<skos:Concept rdf:about="http://www.earthobservations.org/GEOSS/EO_Vocabulary/net%20primary%20production">
		<skos:prefLabel>Net Primary Production</skos:prefLabel>
		<skos:definition>Net primary productivity is the excess of gross_primary_producivity (rate of synthesis of biomass per unit area from inorganic precursors by autotrophs, or "producers", especially by photosynthesising plants using sunlight for energy) over the rate at which they themselves respire some of this biomass (plant_respiration, assuming all producers to be plants). "Productivity of carbon" refers to the production of biomass expressed as the mass of carbon which it contains. "Productivity" means production per unit area.</skos:definition>
		<skos:scopeNote>CF Standard Names</skos:scopeNote>
		<skos:broader rdf:resource="http://www.earthobservations.org/GEOSS/EO_Vocabulary/ecological%20dynamics"/>
		<rdfs:seeAlso rdf:resource="http://cf-pcmdi.llnl.gov/documents/cf-standard-names/standard-name-table/17/cf-standard-name-table.html"/>
		<rdfs:seeAlso rdf:resource="http://gcmd.nasa.gov/Resources/valids/archives/keyword_list.html"/>
		<skos:inScheme rdf:resource="http://www.earthobservations.org/GEOSS/EO_Vocabulary"/>
	</skos:Concept>
	<skos:Concept rdf:about="http://www.earthobservations.org/GEOSS/EO_Vocabulary/sea%20level">
		<skos:prefLabel>Sea Level</skos:prefLabel>
		<skos:definition>The level of the surface of the ocean; especially, the mean level halfway between high and low tide, used as a standard in reckoning land elevation or sea depths. (Source: MGH)</skos:definition>
		<skos:scopeNote>GEMET</skos:scopeNote>
		<skos:broader rdf:resource="http://www.earthobservations.org/GEOSS/EO_Vocabulary/coastal%20processes"/>
		<rdfs:seeAlso rdf:resource="http://gcmd.nasa.gov/Resources/valids/archives/keyword_list.html"/>
		<skos:inScheme rdf:resource="http://www.earthobservations.org/GEOSS/EO_Vocabulary"/>
	</skos:Concept>
	<skos:Concept rdf:about="http://www.earthobservations.org/GEOSS/EO_Vocabulary/snow%20cover%20extent">
		<skos:prefLabel>Snow Cover Extent</skos:prefLabel>
		<skos:definition>The cryosphere collectively describes the portions of a planetary surface in frozen form, including sea ice, lake ice, river ice, snow cover, glaciers, ice caps and ice sheets, and frozen ground (which includes permafrost). [Wikipedia]</skos:definition>
		<skos:scopeNote>SWEET 2.0 </skos:scopeNote>
		<skos:broader rdf:resource="http://www.earthobservations.org/GEOSS/EO_Vocabulary/snow%2Fice"/>
		<skos:broader rdf:resource="http://www.earthobservations.org/GEOSS/EO_Vocabulary/snow%2Fice"/>
		<rdfs:seeAlso rdf:resource="http://sweet.jpl.nasa.gov/"/>
		<rdfs:seeAlso rdf:resource="http://webworld.unesco.org/water/ihp/db/glossary/glu/EN/GF1129EN.HTM"/>
		<rdfs:seeAlso rdf:resource="http://gcmd.nasa.gov/Resources/valids/archives/keyword_list.html"/>
		<skos:inScheme rdf:resource="http://www.earthobservations.org/GEOSS/EO_Vocabulary"/>
	</skos:Concept>
	<skos:Concept rdf:about="http://www.earthobservations.org/GEOSS/EO_Vocabulary/lake%2Freservoir%20levels%20and%20area">
		<skos:prefLabel>Lake/Reservoir Levels and Area</skos:prefLabel>
		<skos:definition>An artificial or natural storage place for water, such as a lake or pond, from which the water may be withdrawn as for irrigation, municipal water supply, or flood control. (Source: BJGEO)</skos:definition>
		<skos:scopeNote>GEMET</skos:scopeNote>
		<skos:broader rdf:resource="http://www.earthobservations.org/GEOSS/EO_Vocabulary/ocean%2Flake%20records"/>
		<rdfs:seeAlso rdf:resource="http://www.eionet.europa.eu/gemet/concept/4594"/>
		<rdfs:seeAlso rdf:resource="http://www.eionet.europa.eu/gemet/concept/12248"/>
		<rdfs:seeAlso rdf:resource="http://sweet.jpl.nasa.gov/"/>
		<rdfs:seeAlso rdf:resource="http://sweet.jpl.nasa.gov/"/>
		<rdfs:seeAlso rdf:resource="http://his.cuahsi.org/ontologyfiles.html"/>
		<rdfs:seeAlso rdf:resource="http://webworld.unesco.org/water/ihp/db/glossary/glu/EN/GF0729EN.HTM"/>
		<rdfs:seeAlso rdf:resource="http://webworld.unesco.org/water/ihp/db/glossary/glu/EN/GF1011EN.HTM"/>
		<rdfs:seeAlso rdf:resource="http://gcmd.nasa.gov/Resources/valids/archives/keyword_list.html"/>
		<skos:inScheme rdf:resource="http://www.earthobservations.org/GEOSS/EO_Vocabulary"/>
	</skos:Concept>
	<skos:Concept rdf:about="http://www.earthobservations.org/GEOSS/EO_Vocabulary/cultivation">
		<skos:prefLabel>Cultivation</skos:prefLabel>
		<skos:definition>The practice of growing and nurturing plants outside of their wild habitat (i.e., in gardens, nurseries, arboreta). (Source: DUNSTE) </skos:definition>
		<skos:scopeNote>GEMET</skos:scopeNote>
		<skos:broader rdf:resource="http://www.earthobservations.org/GEOSS/EO_Vocabulary/agricultural%20engineering"/>
		<skos:broader rdf:resource="http://www.earthobservations.org/GEOSS/EO_Vocabulary/land%20use%2Fland%20cover"/>
		<skos:inScheme rdf:resource="http://www.earthobservations.org/GEOSS/EO_Vocabulary"/>
	</skos:Concept>
	<skos:Concept rdf:about="http://www.earthobservations.org/GEOSS/EO_Vocabulary/deforestation">
		<skos:prefLabel>Deforestation</skos:prefLabel>
		<skos:definition>The removal of forest and undergrowth to increase the surface of arable land or to use the timber for construction or industrial purposes. Forest and its undergrowth possess a very high water-retaining capacity, inhibiting runoff of rainwater. (Source: GILP) </skos:definition>
		<skos:scopeNote>GEMET</skos:scopeNote>
		<skos:broader rdf:resource="http://www.earthobservations.org/GEOSS/EO_Vocabulary/habitat%20conversion%2Ffragmentation"/>
		<rdfs:seeAlso rdf:resource="http://gcmd.nasa.gov/Resources/valids/archives/keyword_list.html"/>
		<skos:inScheme rdf:resource="http://www.earthobservations.org/GEOSS/EO_Vocabulary"/>
	</skos:Concept>
	<skos:Concept rdf:about="http://www.earthobservations.org/GEOSS/EO_Vocabulary/forest%20cover">
		<skos:prefLabel>Forest Cover</skos:prefLabel>
		<skos:definition>A vegetation community dominated by trees and other woody shrubs, growing close enough together that the tree tops touch or overlap, creating various degrees of shade on the forest floor. It may produce benefits such as timber, recreation, wildlife habitat, etc. (Source: DUNSTE) </skos:definition>
		<skos:scopeNote>GEMET</skos:scopeNote>
		<skos:broader rdf:resource="http://www.earthobservations.org/GEOSS/EO_Vocabulary/terrestrial%20ecosystems"/>
		<rdfs:seeAlso rdf:resource="http://gcmd.nasa.gov/Resources/valids/archives/keyword_list.html"/>
		<skos:inScheme rdf:resource="http://www.earthobservations.org/GEOSS/EO_Vocabulary"/>
	</skos:Concept>
	<skos:Concept rdf:about="http://www.earthobservations.org/GEOSS/EO_Vocabulary/cloud%20cover">
		<skos:prefLabel>Cloud Cover</skos:prefLabel>
		<skos:definition>Suspensions of minute water droplets or ice crystals produced by the condensation of water vapour. (Source: ZINZAN) </skos:definition>
		<skos:scopeNote>GEMET</skos:scopeNote>
		<skos:broader rdf:resource="http://www.earthobservations.org/GEOSS/EO_Vocabulary/aerosols"/>
		<rdfs:seeAlso rdf:resource="http://earthobservatory.nasa.gov/Glossary/index.php?mode=alpha&amp;seg=b&amp;segend=d"/>
		<rdfs:seeAlso rdf:resource="http://cf-pcmdi.llnl.gov/documents/cf-standard-names/standard-name-table/17/cf-standard-name-table.html "/>
		<skos:inScheme rdf:resource="http://www.earthobservations.org/GEOSS/EO_Vocabulary"/>
	</skos:Concept>
	<skos:Concept rdf:about="http://www.earthobservations.org/GEOSS/EO_Vocabulary/ocean%20topography">
		<skos:prefLabel>Ocean Topography</skos:prefLabel>
		<skos:definition>The general configuration of theLAND SURFACE, including its relief and the position of its natural features.</skos:definition>
		<skos:scopeNote>GCMD</skos:scopeNote>
		<skos:broader rdf:resource="http://www.earthobservations.org/GEOSS/EO_Vocabulary/bathymetry%2Fseafloor%20topography"/>
		<skos:broader rdf:resource="http://www.earthobservations.org/GEOSS/EO_Vocabulary/bathymetry%2Fseafloor%20topography"/>
		<rdfs:seeAlso rdf:resource="http://sweet.jpl.nasa.gov/"/>
		<rdfs:seeAlso rdf:resource="http://earthobservatory.nasa.gov/Glossary/?mode=alpha&amp;seg=t"/>
		<rdfs:seeAlso rdf:resource="http://gcmd.nasa.gov/Resources/valids/archives/keyword_list.html\"/>
		<rdfs:seeAlso rdf:resource="http://inspire-registry.jrc.ec.europa.eu/"/>
		<rdfs:seeAlso rdf:resource="http://gcmd.nasa.gov/Resources/valids/archives/keyword_list.html"/>
		<rdfs:seeAlso rdf:resource="http://gcmd.nasa.gov/Resources/valids/archives/keyword_list.html"/>
		<skos:inScheme rdf:resource="http://www.earthobservations.org/GEOSS/EO_Vocabulary"/>
	</skos:Concept>
	<skos:Concept rdf:about="http://www.earthobservations.org/GEOSS/EO_Vocabulary/soil%20composition">
		<skos:prefLabel>Soil Composition</skos:prefLabel>
		<skos:definition>1) Refers to the relative proportions of the various size groups (sand, silt and clay) of the individual soil grains in a mass of soil. 2) Classification of soil by the proportion and graduations of the three size groups of soil grains, i.e., sand, silt and clay, present in the soil. (Source: LANDY)</skos:definition>
		<skos:scopeNote>GEMET</skos:scopeNote>
		<skos:broader rdf:resource="http://www.earthobservations.org/GEOSS/EO_Vocabulary/agricultural%20plant%20science"/>
		<skos:broader rdf:resource="http://www.earthobservations.org/GEOSS/EO_Vocabulary/soils"/>
		<rdfs:seeAlso rdf:resource="http://sweet.jpl.nasa.gov/"/>
		<rdfs:seeAlso rdf:resource="http://his.cuahsi.org/ontologyfiles.html"/>
		<rdfs:seeAlso rdf:resource="http://inspire-registry.jrc.ec.europa.eu/"/>
		<skos:inScheme rdf:resource="http://www.earthobservations.org/GEOSS/EO_Vocabulary"/>
	</skos:Concept>
	<skos:Concept rdf:about="http://www.earthobservations.org/GEOSS/EO_Vocabulary/fraction%20of%20photosynthetically%20active%20radiation%20%28fpar%29">
		<skos:prefLabel>Fraction of Photosynthetically Active Radiation (fPAR)</skos:prefLabel>
		<skos:definition>Radiation between 400 and 700 nm used by the green canopy in the photosynthetic process.</skos:definition>
		<skos:scopeNote>NASA</skos:scopeNote>
		<skos:broader rdf:resource="http://www.earthobservations.org/GEOSS/EO_Vocabulary/surface%20radiative%20properties"/>
		<rdfs:seeAlso rdf:resource="http://sweet.jpl.nasa.gov/"/>
		<rdfs:seeAlso rdf:resource="http://earthobservatory.nasa.gov/Glossary/index.php?mode=alpha&amp;seg=f&amp;segend=h"/>
		<skos:inScheme rdf:resource="http://www.earthobservations.org/GEOSS/EO_Vocabulary"/>
	</skos:Concept>
	<skos:Concept rdf:about="http://www.earthobservations.org/GEOSS/EO_Vocabulary/soil%20type">
		<skos:prefLabel>Soil Type</skos:prefLabel>
		<skos:definition>1) Refers to the relative proportions of the various size groups (sand, silt and clay) of the individual soil grains in a mass of soil. 2) Classification of soil by the proportion and graduations of the three size groups of soil grains, i.e., sand, silt and clay, present in the soil. (Source: LANDY)</skos:definition>
		<skos:scopeNote>GEMET</skos:scopeNote>
		<skos:broader rdf:resource="http://www.earthobservations.org/GEOSS/EO_Vocabulary/soils"/>
		<skos:broader rdf:resource="http://www.earthobservations.org/GEOSS/EO_Vocabulary/soils"/>
		<rdfs:seeAlso rdf:resource="http://sweet.jpl.nasa.gov/"/>
		<rdfs:seeAlso rdf:resource="http://his.cuahsi.org/ontologyfiles.html"/>
		<skos:inScheme rdf:resource="http://www.earthobservations.org/GEOSS/EO_Vocabulary"/>
	</skos:Concept>
	<skos:Concept rdf:about="http://www.earthobservations.org/GEOSS/EO_Vocabulary/global%20horizontal%20irradiation%20%28ghi%29">
		<skos:prefLabel>Global Horizontal Irradiation (GHI)</skos:prefLabel>
		<skos:definition>To subject to or treat with light or other electromagnetic radiation or with beams of particles. (Source: CED)</skos:definition>
		<skos:scopeNote>GEMET</skos:scopeNote>
		<skos:broader rdf:resource="http://www.earthobservations.org/GEOSS/EO_Vocabulary/atmospheric%20radiation"/>
		<skos:inScheme rdf:resource="http://www.earthobservations.org/GEOSS/EO_Vocabulary"/>
	</skos:Concept>
	<skos:Concept rdf:about="http://www.earthobservations.org/GEOSS/EO_Vocabulary/groundwater">
		<skos:prefLabel>Groundwater</skos:prefLabel>
		<skos:definition>Subsurface water occupying the saturated zone.</skos:definition>
		<skos:scopeNote>UNESCO</skos:scopeNote>
		<skos:broader rdf:resource="http://www.earthobservations.org/GEOSS/EO_Vocabulary/surface%20water"/>
		<skos:broader rdf:resource="http://www.earthobservations.org/GEOSS/EO_Vocabulary/water%20quality%2Fwater%20chemistry"/>
		<rdfs:seeAlso rdf:resource="http://sweet.jpl.nasa.gov/"/>
		<rdfs:seeAlso rdf:resource="http://webworld.unesco.org/water/ihp/db/glossary/glu/EN/GF0551EN.HTM"/>
		<skos:inScheme rdf:resource="http://www.earthobservations.org/GEOSS/EO_Vocabulary"/>
	</skos:Concept>
	<skos:Concept rdf:about="http://www.earthobservations.org/GEOSS/EO_Vocabulary/ambient%20particulate%20matter%20concentration%20%28fine%29">
		<skos:prefLabel>Ambient Particulate Matter Concentration (fine)</skos:prefLabel>
		<skos:definition>Particulate matter in ice cores (continental dust, volcanic ash, diatoms, and pollen)can provide information on past climate conditions and climate variability.</skos:definition>
		<skos:scopeNote>GCMD</skos:scopeNote>
		<skos:broader rdf:resource="http://www.earthobservations.org/GEOSS/EO_Vocabulary/aerosols"/>
		<skos:broader rdf:resource="http://www.earthobservations.org/GEOSS/EO_Vocabulary/ice%20core%20records"/>
		<rdfs:seeAlso rdf:resource="http://gcmd.nasa.gov/Resources/valids/archives/keyword_list.html"/>
		<rdfs:seeAlso rdf:resource="http://gcmd.nasa.gov/Resources/valids/archives/keyword_list.html"/>
		<skos:inScheme rdf:resource="http://www.earthobservations.org/GEOSS/EO_Vocabulary"/>
	</skos:Concept>
	<skos:Concept rdf:about="http://www.earthobservations.org/GEOSS/EO_Vocabulary/gross%20primary%20productivity">
		<skos:prefLabel>Gross Primary Productivity</skos:prefLabel>
		<skos:definition>The rate at which new plant biomass is formed by photosynthesis. Gross primary productivity is the total rate of photosynthetic production of biomass; net primary productivity is gross primary productivity minus the respiration rate.</skos:definition>
		<skos:scopeNote>NASA</skos:scopeNote>
		<skos:broader rdf:resource="http://www.earthobservations.org/GEOSS/EO_Vocabulary/ecological%20dynamics"/>
		<rdfs:seeAlso rdf:resource="http://his.cuahsi.org/ontologyfiles.html"/>
		<rdfs:seeAlso rdf:resource="http://stommel.tamu.edu/~baum/paleo/paleogloss/node35.html#SECTION020310000000000000000"/>
		<rdfs:seeAlso rdf:resource="http://earthobservatory.nasa.gov/Glossary/?mode=alpha&amp;seg=p"/>
		<rdfs:seeAlso rdf:resource="http://gcmd.nasa.gov/Resources/valids/archives/keyword_list.html"/>
		<rdfs:seeAlso rdf:resource="http://dias.csis.u-tokyo.ac.jp/dict/cf_meta/index.php/Gross_primary_productivity_of_carbon"/>
		<skos:inScheme rdf:resource="http://www.earthobservations.org/GEOSS/EO_Vocabulary"/>
	</skos:Concept>
	<skos:Concept rdf:about="http://www.earthobservations.org/GEOSS/EO_Vocabulary/cloud%20water%2Fice%20amounts">
		<skos:prefLabel>Cloud Water/Ice Amounts</skos:prefLabel>
		<skos:definition>Liquid phase of a chemical compound consisting of approximately two parts by weight of hydrogen and 16 parts by weight of oxygen. In nature it contains small amounts of heavy water, gases and solids (mainly salts) in solution.</skos:definition>
		<skos:scopeNote>UNESCO</skos:scopeNote>
		<skos:broader rdf:resource="http://www.earthobservations.org/GEOSS/EO_Vocabulary/clouds"/>
		<skos:broader rdf:resource="http://www.earthobservations.org/GEOSS/EO_Vocabulary/clouds"/>
		<skos:broader rdf:resource="http://www.earthobservations.org/GEOSS/EO_Vocabulary/clouds"/>
		<rdfs:seeAlso rdf:resource="http://webworld.unesco.org/water/ihp/db/glossary/glu/EN/GF1353EN.HTM"/>
		<skos:inScheme rdf:resource="http://www.earthobservations.org/GEOSS/EO_Vocabulary"/>
	</skos:Concept>
	<skos:Concept rdf:about="http://www.earthobservations.org/GEOSS/EO_Vocabulary/evaporation">
		<skos:prefLabel>Evaporation</skos:prefLabel>
		<skos:definition>The physical process by which a liquid is transformed to the gaseous state. Evaporation also implies a loss of heat from the ocean surface and is an important term in determining the heat budget of the ocean.</skos:definition>
		<skos:scopeNote>GCMD</skos:scopeNote>
		<skos:broader rdf:resource="http://www.earthobservations.org/GEOSS/EO_Vocabulary/atmospheric%20water%20vapor"/>
		<skos:broader rdf:resource="http://www.earthobservations.org/GEOSS/EO_Vocabulary/ocean%20heat%20budget"/>
		<rdfs:seeAlso rdf:resource="http://webworld.unesco.org/water/ihp/db/glossary/glu/EN/GF0421EN.HTM"/>
		<rdfs:seeAlso rdf:resource="http://earthobservatory.nasa.gov/Glossary/?mode=alpha&amp;seg=e"/>
		<rdfs:seeAlso rdf:resource="http://gcmd.nasa.gov/Resources/valids/archives/keyword_list.html"/>
		<skos:inScheme rdf:resource="http://www.earthobservations.org/GEOSS/EO_Vocabulary"/>
	</skos:Concept>
	<skos:Concept rdf:about="http://www.earthobservations.org/GEOSS/EO_Vocabulary/evapotranspiration">
		<skos:prefLabel>Evapotranspiration</skos:prefLabel>
		<skos:definition>The vaporization of water through direct evaporation from wet surfaces plus the release of water vapor by plants through leaf pores.</skos:definition>
		<skos:scopeNote>x</skos:scopeNote>
		<skos:broader rdf:resource="http://www.earthobservations.org/GEOSS/EO_Vocabulary/atmospheric%20water%20vapor"/>
		<rdfs:seeAlso rdf:resource="http://webworld.unesco.org/water/ihp/db/glossary/glu/EN/GF0426EN.HTM"/>
		<rdfs:seeAlso rdf:resource="http://stommel.tamu.edu/~baum/paleo/paleogloss/node14.html#SECTION020100000000000000000"/>
		<rdfs:seeAlso rdf:resource="http://earthobservatory.nasa.gov/Glossary/?mode=alpha&amp;seg=e"/>
		<rdfs:seeAlso rdf:resource="http://gcmd.nasa.gov/Resources/valids/archives/keyword_list.html"/>
		<skos:inScheme rdf:resource="http://www.earthobservations.org/GEOSS/EO_Vocabulary"/>
	</skos:Concept>
	<skos:Concept rdf:about="http://www.earthobservations.org/GEOSS/EO_Vocabulary/ambient%20ozone%20concentration">
		<skos:prefLabel>Ambient Ozone Concentration</skos:prefLabel>
		<skos:definition>Ozone (O3) is a molecule that consists of three oxygen atoms bonded together. The ozone layer in the stratosphere absorbs UV radiation and creates a warm layer of air high in the stratosphere. Ozone that is present in the troposphere is mostly a result of anthropogenic pollution and therefore higher concentrations are found in urban areas. Ozone is involved with NOx in the photochemical production of many of the constituents of pollution environments (see nitrogen oxides and hydroxyl definitions) [Chemical and Engineering News; v72; 6-7; 1994.] [Aviation Week and Space Technology; v140; 20-21; 1994.]</skos:definition>
		<skos:scopeNote>GCMD</skos:scopeNote>
		<skos:broader rdf:resource="http://www.earthobservations.org/GEOSS/EO_Vocabulary/atmospheric%20chemistry"/>
		<rdfs:seeAlso rdf:resource="http://sweet.jpl.nasa.gov/ "/>
		<rdfs:seeAlso rdf:resource="http://stommel.tamu.edu/~baum/paleo/paleogloss/node33.html#SECTION020290000000000000000"/>
		<rdfs:seeAlso rdf:resource="http://earthobservatory.nasa.gov/Glossary/?mode=alpha&amp;seg=o"/>
		<rdfs:seeAlso rdf:resource="http://gcmd.nasa.gov/Resources/valids/archives/keyword_list.html"/>
		<rdfs:seeAlso rdf:resource="http://cf-pcmdi.llnl.gov/documents/cf-standard-names/ "/>
		<skos:inScheme rdf:resource="http://www.earthobservations.org/GEOSS/EO_Vocabulary"/>
	</skos:Concept>
	<skos:Concept rdf:about="http://www.earthobservations.org/GEOSS/EO_Vocabulary/biomass">
		<skos:prefLabel>Biomass</skos:prefLabel>
		<skos:definition>Mass of biological material. Usually the total mass of a particular group or category; for example, the biomass of producer organisms.</skos:definition>
		<skos:scopeNote>GCMD</skos:scopeNote>
		<skos:broader rdf:resource="http://www.earthobservations.org/GEOSS/EO_Vocabulary/vegetation"/>
		<rdfs:seeAlso rdf:resource="http://sweet.jpl.nasa.gov/ "/>
		<rdfs:seeAlso rdf:resource="http://webworld.unesco.org/water/ihp/db/glossary/glu/EN/GF0135EN.HTM"/>
		<rdfs:seeAlso rdf:resource="http://stommel.tamu.edu/~baum/paleo/paleogloss/node7.html#SECTION02030000000000000000"/>
		<rdfs:seeAlso rdf:resource="http://earthobservatory.nasa.gov/Glossary/?mode=alpha&amp;seg=b&amp;segend=d"/>
		<rdfs:seeAlso rdf:resource="http://gcmd.nasa.gov/Resources/valids/archives/keyword_list.html"/>
		<skos:inScheme rdf:resource="http://www.earthobservations.org/GEOSS/EO_Vocabulary"/>
	</skos:Concept>
	<skos:Concept rdf:about="http://www.earthobservations.org/GEOSS/EO_Vocabulary/burned%20area%2Ffires">
		<skos:prefLabel>Burned Area/Fires</skos:prefLabel>
		<skos:definition>Fire is a natural occurrence playing a very important role in many ecosystems. However, when fire threatens human life or property, it is considered a natural hazard. Besides the obvious hazard of hot flames causing materials to burn, fire can also send vast amounts of ash into the atmosphere+E518, inhibiting plant growth, reducing visibility, and interfering with breathing.</skos:definition>
		<skos:scopeNote>GCMD</skos:scopeNote>
		<skos:broader rdf:resource="http://www.earthobservations.org/GEOSS/EO_Vocabulary/natural%20hazards"/>
		<rdfs:seeAlso rdf:resource="http://gcmd.nasa.gov/Resources/valids/archives/keyword_list.html"/>
		<skos:inScheme rdf:resource="http://www.earthobservations.org/GEOSS/EO_Vocabulary"/>
	</skos:Concept>
	<skos:Concept rdf:about="http://www.earthobservations.org/GEOSS/EO_Vocabulary/desertification">
		<skos:prefLabel>Desertification</skos:prefLabel>
		<skos:definition> Desertification is the formation of deserts in arid and semi-arid regions from overgrazing, deforestation, poor agricultural practices, and climate change. Evidence of desertification can be found today in Africa, the Middle East, and the southwestern United States.</skos:definition>
		<skos:scopeNote>GCMD</skos:scopeNote>
		<skos:broader rdf:resource="http://www.earthobservations.org/GEOSS/EO_Vocabulary/habitat%20conversion%2Ffragmentation"/>
		<rdfs:seeAlso rdf:resource="http://sweet.jpl.nasa.gov/"/>
		<rdfs:seeAlso rdf:resource="http://stommel.tamu.edu/~baum/paleo/paleogloss/node11.html#SECTION02070000000000000000"/>
		<rdfs:seeAlso rdf:resource="http://earthobservatory.nasa.gov/Glossary/?mode=alpha&amp;seg=d"/>
		<rdfs:seeAlso rdf:resource="http://gcmd.nasa.gov/Resources/valids/archives/keyword_list.html"/>
		<skos:inScheme rdf:resource="http://www.earthobservations.org/GEOSS/EO_Vocabulary"/>
	</skos:Concept>
	<skos:Concept rdf:about="http://www.earthobservations.org/GEOSS/EO_Vocabulary/enhanced%20vegetation%20index%20%28evi%29">
		<skos:prefLabel>Enhanced Vegetation Index (EVI)</skos:prefLabel>
		<skos:definition>Includes Global Change Master Directory detailed variables under the variable, </skos:definition>
		<skos:scopeNote>GCMD</skos:scopeNote>
		<skos:broader rdf:resource="http://www.earthobservations.org/GEOSS/EO_Vocabulary/vegetation"/>
		<rdfs:seeAlso rdf:resource="http://gcmd.nasa.gov/Resources/valids/archives/keyword_list.html"/>
		<skos:inScheme rdf:resource="http://www.earthobservations.org/GEOSS/EO_Vocabulary"/>
	</skos:Concept>
	<skos:Concept rdf:about="http://www.earthobservations.org/GEOSS/EO_Vocabulary/glacier%2Fice%20sheet%20depth">
		<skos:prefLabel>Glacier/Ice Sheet Depth</skos:prefLabel>
		<skos:definition>A layer of ice covering an extensive tract of land for a long period of time.</skos:definition>
		<skos:scopeNote>Oxford Dictionaries</skos:scopeNote>
		<skos:broader rdf:resource="http://www.earthobservations.org/GEOSS/EO_Vocabulary/glaciers%2Fice%20sheets"/>
		<skos:broader rdf:resource="http://www.earthobservations.org/GEOSS/EO_Vocabulary/snow%2Fice"/>
		<skos:broader rdf:resource="http://www.earthobservations.org/GEOSS/EO_Vocabulary/glaciers%2Fice%20sheets"/>
		<skos:broader rdf:resource="http://www.earthobservations.org/GEOSS/EO_Vocabulary/snow%2Fice"/>
		<rdfs:seeAlso rdf:resource="http://sweet.jpl.nasa.gov/"/>
		<rdfs:seeAlso rdf:resource="http://oxforddictionaries.com/view/entry/m_en_gb0397550#m_en_gb0397550"/>
		<skos:inScheme rdf:resource="http://www.earthobservations.org/GEOSS/EO_Vocabulary"/>
	</skos:Concept>
	<skos:Concept rdf:about="http://www.earthobservations.org/GEOSS/EO_Vocabulary/soil%20adjusted%20vegetation%20index%20%28savi%29%2Bc29">
		<skos:prefLabel>Soil Adjusted Vegetation Index (SAVI)+C29</skos:prefLabel>
		<skos:definition>Includes Global Change Master Directory detailed variables under the variable, </skos:definition>
		<skos:scopeNote>GCMD</skos:scopeNote>
		<skos:broader rdf:resource="http://www.earthobservations.org/GEOSS/EO_Vocabulary/vegetation"/>
		<rdfs:seeAlso rdf:resource="http://gcmd.nasa.gov/Resources/valids/archives/keyword_list.html"/>
		<skos:inScheme rdf:resource="http://www.earthobservations.org/GEOSS/EO_Vocabulary"/>
	</skos:Concept>
	<skos:Concept rdf:about="http://www.earthobservations.org/GEOSS/EO_Vocabulary/water%20run-off">
		<skos:prefLabel>Water run-off</skos:prefLabel>
		<skos:definition>The measurment of the flow of water in a stream, usually expressed in cubic feet per second; the net effect of storms, accumulation, transpiration, meltage, seepage, evaporation, and percolation.</skos:definition>
		<skos:scopeNote>GCMD</skos:scopeNote>
		<skos:broader rdf:resource="http://www.earthobservations.org/GEOSS/EO_Vocabulary/surface%20water"/>
		<rdfs:seeAlso rdf:resource="http://sweet.jpl.nasa.gov/"/>
		<rdfs:seeAlso rdf:resource="http://webworld.unesco.org/water/ihp/db/glossary/glu/EN/GF1049EN.HTM"/>
		<rdfs:seeAlso rdf:resource="http://gcmd.nasa.gov/Resources/valids/archives/keyword_list.html"/>
		<rdfs:seeAlso rdf:resource="http://webworld.unesco.org/water/ihp/db/glossary/glu/EN/GF1252EN.HTM"/>
		<skos:inScheme rdf:resource="http://www.earthobservations.org/GEOSS/EO_Vocabulary"/>
	</skos:Concept>
	<skos:Concept rdf:about="http://www.earthobservations.org/GEOSS/EO_Vocabulary/column%20particulate%20matter%20concentration%20%28fine%29">
		<skos:prefLabel>Column Particulate Matter Concentration (fine)</skos:prefLabel>
		<skos:definition>Particulate matter in ice cores (continental dust, volcanic ash, diatoms, and pollen)can provide information on past climate conditions and climate variability.</skos:definition>
		<skos:scopeNote>GCMD</skos:scopeNote>
		<skos:broader rdf:resource="http://www.earthobservations.org/GEOSS/EO_Vocabulary/aerosols"/>
		<skos:broader rdf:resource="http://www.earthobservations.org/GEOSS/EO_Vocabulary/ice%20core%20records"/>
		<rdfs:seeAlso rdf:resource="http://gcmd.nasa.gov/Resources/valids/archives/keyword_list.html"/>
		<rdfs:seeAlso rdf:resource="http://gcmd.nasa.gov/Resources/valids/archives/keyword_list.html"/>
		<skos:inScheme rdf:resource="http://www.earthobservations.org/GEOSS/EO_Vocabulary"/>
	</skos:Concept>
	<skos:Concept rdf:about="http://www.earthobservations.org/GEOSS/EO_Vocabulary/floods">
		<skos:prefLabel>Floods</skos:prefLabel>
		<skos:definition> The condition that occurs when water overflows the natural or artificial confines of a stream or other body of water, or accumulates by drainage over low-lying areas.</skos:definition>
		<skos:scopeNote>GCMD</skos:scopeNote>
		<skos:broader rdf:resource="http://www.earthobservations.org/GEOSS/EO_Vocabulary/surface%20water"/>
		<skos:inScheme rdf:resource="http://www.earthobservations.org/GEOSS/EO_Vocabulary"/>
	</skos:Concept>
	<skos:Concept rdf:about="http://www.earthobservations.org/GEOSS/EO_Vocabulary/ambient%20particulate%20matter%20%28fine%29%20composition">
		<skos:prefLabel>Ambient Particulate Matter (fine) Composition</skos:prefLabel>
		<skos:definition>Particulate matter in ice cores (continental dust, volcanic ash, diatoms, and pollen)can provide information on past climate conditions and climate variability.</skos:definition>
		<skos:scopeNote>GCMD</skos:scopeNote>
		<skos:broader rdf:resource="http://www.earthobservations.org/GEOSS/EO_Vocabulary/aerosols"/>
		<skos:broader rdf:resource="http://www.earthobservations.org/GEOSS/EO_Vocabulary/ice%20core%20records"/>
		<rdfs:seeAlso rdf:resource="http://gcmd.nasa.gov/Resources/valids/archives/keyword_list.html"/>
		<rdfs:seeAlso rdf:resource="http://gcmd.nasa.gov/Resources/valids/archives/keyword_list.html"/>
		<skos:inScheme rdf:resource="http://www.earthobservations.org/GEOSS/EO_Vocabulary"/>
	</skos:Concept>
	<skos:Concept rdf:about="http://www.earthobservations.org/GEOSS/EO_Vocabulary/bathymetry">
		<skos:prefLabel>Bathymetry</skos:prefLabel>
		<skos:definition>The measurement and charting of the spatial variation of the ocean depths.</skos:definition>
		<skos:scopeNote>GCMD</skos:scopeNote>
		<skos:broader rdf:resource="http://www.earthobservations.org/GEOSS/EO_Vocabulary/bathymetry%2Fseafloor%20topography"/>
		<rdfs:seeAlso rdf:resource="http://stommel.tamu.edu/~baum/paleo/paleogloss/node7.html#SECTION02030000000000000000"/>
		<rdfs:seeAlso rdf:resource="http://gcmd.nasa.gov/Resources/valids/archives/keyword_list.html"/>
		<skos:inScheme rdf:resource="http://www.earthobservations.org/GEOSS/EO_Vocabulary"/>
	</skos:Concept>
	<skos:Concept rdf:about="http://www.earthobservations.org/GEOSS/EO_Vocabulary/photosynthetically%20active%20radiation%20%28par%29">
		<skos:prefLabel>Photosynthetically Active Radiation (PAR)</skos:prefLabel>
		<skos:definition>Photosynthetically Active Radiation is the light in the whole wavelength band from 400 nm (deep violet) to 700 nm (dark red) used by plants in photosynthesis.</skos:definition>
		<skos:scopeNote>GCMD</skos:scopeNote>
		<skos:broader rdf:resource="http://www.earthobservations.org/GEOSS/EO_Vocabulary/vegetation"/>
		<skos:broader rdf:resource="http://www.earthobservations.org/GEOSS/EO_Vocabulary/ocean%20optics"/>
		<skos:inScheme rdf:resource="http://www.earthobservations.org/GEOSS/EO_Vocabulary"/>
	</skos:Concept>
	<skos:Concept rdf:about="http://www.earthobservations.org/GEOSS/EO_Vocabulary/water%20quality%20%26%20composition%2C%20ph%20and%20salinity%2C%20dissolved%20oxygen%20content">
		<skos:prefLabel>Water Quality &amp; Composition, pH and salinity, Dissolved Oxygen Content</skos:prefLabel>
		<skos:definition>x</skos:definition>
		<skos:scopeNote>x</skos:scopeNote>
		<skos:broader rdf:resource="http://www.earthobservations.org/GEOSS/EO_Vocabulary/water%20quality"/>
		<skos:broader rdf:resource="http://www.earthobservations.org/GEOSS/EO_Vocabulary/ocean%20chemistry"/>
		<skos:broader rdf:resource="http://www.earthobservations.org/GEOSS/EO_Vocabulary/water%20quality%2Fwater%20chemistry"/>
		<skos:broader rdf:resource="http://www.earthobservations.org/GEOSS/EO_Vocabulary/sea%20ice"/>
		<skos:broader rdf:resource="http://www.earthobservations.org/GEOSS/EO_Vocabulary/sea%20ice"/>
		<skos:broader rdf:resource="http://www.earthobservations.org/GEOSS/EO_Vocabulary/salinity%2Fdensity"/>
		<skos:broader rdf:resource="http://www.earthobservations.org/GEOSS/EO_Vocabulary/aquatic%20ecosystems"/>
		<skos:broader rdf:resource="http://www.earthobservations.org/GEOSS/EO_Vocabulary/ecological%20dynamics"/>
		<rdfs:seeAlso rdf:resource="http://his.cuahsi.org/ontologyfiles.html"/>
		<rdfs:seeAlso rdf:resource="http://webworld.unesco.org/water/ihp/db/glossary/glu/EN/GF1374EN.HTM"/>
		<rdfs:seeAlso rdf:resource="http://gcmd.nasa.gov/Resources/valids/archives/keyword_list.html"/>
		<rdfs:seeAlso rdf:resource="http://webworld.unesco.org/water/ihp/db/glossary/glu/EN/GF1353EN.HTM"/>
		<rdfs:seeAlso rdf:resource="http://sweet.jpl.nasa.gov/"/>
		<rdfs:seeAlso rdf:resource="http://his.cuahsi.org/ontologyfiles.html"/>
		<rdfs:seeAlso rdf:resource="http://webworld.unesco.org/water/ihp/db/glossary/glu/EN/GF0902EN.HTM"/>
		<rdfs:seeAlso rdf:resource="http://earthobservatory.nasa.gov/Glossary/?mode=alpha&amp;seg=p"/>
		<rdfs:seeAlso rdf:resource="http://gcmd.nasa.gov/Resources/valids/archives/keyword_list.html"/>
		<rdfs:seeAlso rdf:resource="http://sweet.jpl.nasa.gov/"/>
		<rdfs:seeAlso rdf:resource="http://his.cuahsi.org/ontologyfiles.html"/>
		<rdfs:seeAlso rdf:resource="http://cf-pcmdi.llnl.gov/documents/cf-standard-names/"/>
		<rdfs:seeAlso rdf:resource="http://webworld.unesco.org/water/ihp/db/glossary/glu/EN/GF1054EN.HTM"/>
		<rdfs:seeAlso rdf:resource="http://stommel.tamu.edu/~baum/paleo/paleogloss/node39.html#SECTION020350000000000000000"/>
		<rdfs:seeAlso rdf:resource="http://earthobservatory.nasa.gov/Glossary/?mode=alpha&amp;seg=s"/>
		<rdfs:seeAlso rdf:resource="http://gcmd.nasa.gov/Resources/valids/archives/keyword_list.html"/>
		<rdfs:seeAlso rdf:resource="http://gcmd.nasa.gov/Resources/valids/archives/keyword_list.html"/>
		<skos:inScheme rdf:resource="http://www.earthobservations.org/GEOSS/EO_Vocabulary"/>
	</skos:Concept>
	<skos:Concept rdf:about="http://www.earthobservations.org/GEOSS/EO_Vocabulary/ambient%20particulate%20matter%20composition%20%28coarse%29">
		<skos:prefLabel>Ambient Particulate Matter Composition (coarse)</skos:prefLabel>
		<skos:definition>Particulate matter in ice cores (continental dust, volcanic ash, diatoms, and pollen)can provide information on past climate conditions and climate variability.</skos:definition>
		<skos:scopeNote>GCMD</skos:scopeNote>
		<skos:broader rdf:resource="http://www.earthobservations.org/GEOSS/EO_Vocabulary/aerosols"/>
		<skos:broader rdf:resource="http://www.earthobservations.org/GEOSS/EO_Vocabulary/ice%20core%20records"/>
		<rdfs:seeAlso rdf:resource="http://gcmd.nasa.gov/Resources/valids/archives/keyword_list.html"/>
		<rdfs:seeAlso rdf:resource="http://gcmd.nasa.gov/Resources/valids/archives/keyword_list.html"/>
		<skos:inScheme rdf:resource="http://www.earthobservations.org/GEOSS/EO_Vocabulary"/>
	</skos:Concept>
	<skos:Concept rdf:about="http://www.earthobservations.org/GEOSS/EO_Vocabulary/soil%20carbon">
		<skos:prefLabel>Soil Carbon</skos:prefLabel>
		<skos:definition>A nonmetallic element, with chemical symbol C, found combined with other elements in all organic matter and in a pure state as diamond or graphite.</skos:definition>
		<skos:scopeNote>GCMD</skos:scopeNote>
		<skos:broader rdf:resource="http://www.earthobservations.org/GEOSS/EO_Vocabulary/soils"/>
		<skos:broader rdf:resource="http://www.earthobservations.org/GEOSS/EO_Vocabulary/soils"/>
		<skos:broader rdf:resource="http://www.earthobservations.org/GEOSS/EO_Vocabulary/vegetation"/>
		<skos:broader rdf:resource="http://www.earthobservations.org/GEOSS/EO_Vocabulary/ocean%20chemistry"/>
		<rdfs:seeAlso rdf:resource="http://sweet.jpl.nasa.gov/"/>
		<rdfs:seeAlso rdf:resource="http://gcmd.nasa.gov/Resources/valids/archives/keyword_list.html"/>
		<rdfs:seeAlso rdf:resource="http://gcmd.nasa.gov/Resources/valids/archives/keyword_list.html"/>
		<rdfs:seeAlso rdf:resource="http://gcmd.nasa.gov/Resources/valids/archives/keyword_list.html"/>
		<rdfs:seeAlso rdf:resource="http://gcmd.nasa.gov/Resources/valids/archives/keyword_list.html"/>
		<skos:inScheme rdf:resource="http://www.earthobservations.org/GEOSS/EO_Vocabulary"/>
	</skos:Concept>
	<skos:Concept rdf:about="http://www.earthobservations.org/GEOSS/EO_Vocabulary/fraction%20of%20absorbed%20photosynthetically%20active%20radiation%20%28fapar%29">
		<skos:prefLabel>Fraction of Absorbed Photosynthetically Active Radiation (FAPAR)</skos:prefLabel>
		<skos:definition>Photosynthetically Active Radiation is the light in the whole wavelength band from 400 nm (deep violet) to 700 nm (dark red) used by plants in photosynthesis.</skos:definition>
		<skos:scopeNote>GCMD</skos:scopeNote>
		<skos:broader rdf:resource="http://www.earthobservations.org/GEOSS/EO_Vocabulary/vegetation"/>
		<skos:broader rdf:resource="http://www.earthobservations.org/GEOSS/EO_Vocabulary/ocean%20optics"/>
		<rdfs:seeAlso rdf:resource="http://www.wmo.int/pages/prog/sat/Glossary.html"/>
		<skos:inScheme rdf:resource="http://www.earthobservations.org/GEOSS/EO_Vocabulary"/>
	</skos:Concept>
	<skos:Concept rdf:about="http://www.earthobservations.org/GEOSS/EO_Vocabulary/biodiversity">
		<skos:prefLabel>Biodiversity</skos:prefLabel>
		<skos:definition>Biodiversity is the variety of life: the different plants, animals and micro-organisms, their genes and the ecosystems of which they are a part.</skos:definition>
		<skos:scopeNote>GCMD</skos:scopeNote>
		<skos:broader rdf:resource="http://www.earthobservations.org/GEOSS/EO_Vocabulary/ecological%20dynamics"/>
		<skos:broader rdf:resource="http://www.earthobservations.org/GEOSS/EO_Vocabulary/fungi"/>
		<rdfs:seeAlso rdf:resource="http://sweet.jpl.nasa.gov/"/>
		<rdfs:seeAlso rdf:resource="http://stommel.tamu.edu/~baum/paleo/paleogloss/node7.html#SECTION02030000000000000000"/>
		<rdfs:seeAlso rdf:resource="http://earthobservatory.nasa.gov/Glossary/?mode=alpha&amp;seg=b&amp;segend=d"/>
		<rdfs:seeAlso rdf:resource="http://gcmd.nasa.gov/Resources/valids/archives/keyword_list.html"/>
		<skos:inScheme rdf:resource="http://www.earthobservations.org/GEOSS/EO_Vocabulary"/>
	</skos:Concept>
	<skos:Concept rdf:about="http://www.earthobservations.org/GEOSS/EO_Vocabulary/non-native%20species">
		<skos:prefLabel>Non-native species</skos:prefLabel>
		<skos:definition>N/A</skos:definition>
		<skos:scopeNote>SWEET 2.0 </skos:scopeNote>
		<skos:broader rdf:resource="http://www.earthobservations.org/GEOSS/EO_Vocabulary/terrestrial%20ecosystems"/>
		<skos:broader rdf:resource="http://www.earthobservations.org/GEOSS/EO_Vocabulary/vegetation"/>
		<skos:broader rdf:resource="http://www.earthobservations.org/GEOSS/EO_Vocabulary/ecological%20dynamics"/>
		<rdfs:seeAlso rdf:resource="http://sweet.jpl.nasa.gov/"/>
		<rdfs:seeAlso rdf:resource="http://gcmd.nasa.gov/Resources/valids/archives/keyword_list.html"/>
		<skos:inScheme rdf:resource="http://www.earthobservations.org/GEOSS/EO_Vocabulary"/>
	</skos:Concept>
	<skos:Concept rdf:about="http://www.earthobservations.org/GEOSS/EO_Vocabulary/column%20ozone%20concentration">
		<skos:prefLabel>Column Ozone Concentration</skos:prefLabel>
		<skos:definition>Ozone (O3) is a molecule that consists of three oxygen atoms bonded together. The ozone layer in the stratosphere absorbs UV radiation and creates a warm layer of air high in the stratosphere. Ozone that is present in the troposphere is mostly a result of anthropogenic pollution and therefore higher concentrations are found in urban areas. Ozone is involved with NOx in the photochemical production of many of the constituents of pollution environments (see nitrogen oxides and hydroxyl definitions) [Chemical and Engineering News; v72; 6-7; 1994.] [Aviation Week and Space Technology; v140; 20-21; 1994.]</skos:definition>
		<skos:scopeNote>GCMD</skos:scopeNote>
		<skos:broader rdf:resource="http://www.earthobservations.org/GEOSS/EO_Vocabulary/atmospheric%20chemistry"/>
		<rdfs:seeAlso rdf:resource="http://sweet.jpl.nasa.gov/"/>
		<skos:inScheme rdf:resource="http://www.earthobservations.org/GEOSS/EO_Vocabulary"/>
	</skos:Concept>
	<skos:Concept rdf:about="http://www.earthobservations.org/GEOSS/EO_Vocabulary/currents">
		<skos:prefLabel>Currents</skos:prefLabel>
		<skos:definition>Pertaining to or measuring the movement of water in the marine environment. Variables include types of motion, as well as, circulation features. Proper names of oceanic currents are not included.</skos:definition>
		<skos:scopeNote>GCMD</skos:scopeNote>
		<skos:broader rdf:resource="http://www.earthobservations.org/GEOSS/EO_Vocabulary/ocean%20circulation"/>
		<skos:broader rdf:resource="http://www.earthobservations.org/GEOSS/EO_Vocabulary/coastal%20processes"/>
		<skos:broader rdf:resource="http://www.earthobservations.org/GEOSS/EO_Vocabulary/ocean%20circulation"/>
		<rdfs:seeAlso rdf:resource="http://oxforddictionaries.com/view/entry/m_en_gb0198340#m_en_gb0198340.003"/>
		<rdfs:seeAlso rdf:resource="http://gcmd.nasa.gov/Resources/valids/archives/keyword_list.html"/>
		<skos:inScheme rdf:resource="http://www.earthobservations.org/GEOSS/EO_Vocabulary"/>
	</skos:Concept>
	<skos:Concept rdf:about="http://www.earthobservations.org/GEOSS/EO_Vocabulary/glacier%2Fice%20cap%20elevation">
		<skos:prefLabel>Glacier/Ice Cap Elevation</skos:prefLabel>
		<skos:definition>Pertaining to the measured height of large thick, glaciers, with an area of at least 50,000 sq. km, covering a continuous stretch of land and growing in all directions.</skos:definition>
		<skos:scopeNote>GCMD</skos:scopeNote>
		<skos:broader rdf:resource="http://www.earthobservations.org/GEOSS/EO_Vocabulary/snow%2Fice"/>
		<skos:broader rdf:resource="http://www.earthobservations.org/GEOSS/EO_Vocabulary/glaciers%2Fice%20sheets"/>
		<skos:broader rdf:resource="http://www.earthobservations.org/GEOSS/EO_Vocabulary/glaciers%2Fice%20sheets"/>
		<rdfs:seeAlso rdf:resource="http://sweet.jpl.nasa.gov/"/>
		<skos:inScheme rdf:resource="http://www.earthobservations.org/GEOSS/EO_Vocabulary"/>
	</skos:Concept>
	<skos:Concept rdf:about="http://www.earthobservations.org/GEOSS/EO_Vocabulary/water%20use">
		<skos:prefLabel>Water Use</skos:prefLabel>
		<skos:definition>Take or consume (an amount) from a limited supply</skos:definition>
		<skos:scopeNote>Oxford Dictionaries</skos:scopeNote>
		<skos:broader rdf:resource="http://www.earthobservations.org/GEOSS/EO_Vocabulary/human%20dimensions"/>
		<rdfs:seeAlso rdf:resource="http://oxforddictionaries.com/view/entry/m_en_gb0917390#m_en_gb0917390"/>
		<skos:inScheme rdf:resource="http://www.earthobservations.org/GEOSS/EO_Vocabulary"/>
	</skos:Concept>
	<skos:Concept rdf:about="http://www.earthobservations.org/GEOSS/EO_Vocabulary/permafrost">
		<skos:prefLabel>Permafrost</skos:prefLabel>
		<skos:definition> Permanently frozen material underlying the solum.</skos:definition>
		<skos:scopeNote>GCMD</skos:scopeNote>
		<skos:broader rdf:resource="http://www.earthobservations.org/GEOSS/EO_Vocabulary/soils"/>
		<skos:broader rdf:resource="http://www.earthobservations.org/GEOSS/EO_Vocabulary/soils"/>
		<skos:broader rdf:resource="http://www.earthobservations.org/GEOSS/EO_Vocabulary/frozen%20ground"/>
		<skos:broader rdf:resource="http://www.earthobservations.org/GEOSS/EO_Vocabulary/frozen%20ground"/>
		<skos:broader rdf:resource="http://www.earthobservations.org/GEOSS/EO_Vocabulary/snow%2Fice"/>
		<skos:broader rdf:resource="http://www.earthobservations.org/GEOSS/EO_Vocabulary/snow%2Fice"/>
		<rdfs:seeAlso rdf:resource="http://sweet.jpl.nasa.gov/"/>
		<rdfs:seeAlso rdf:resource="http://webworld.unesco.org/water/ihp/db/glossary/glu/EN/GF0897EN.HTM"/>
		<rdfs:seeAlso rdf:resource="http://stommel.tamu.edu/~baum/paleo/paleogloss/node34.html#SECTION020300000000000000000"/>
		<rdfs:seeAlso rdf:resource="http://earthobservatory.nasa.gov/Glossary/?mode=alpha&amp;seg=p"/>
		<rdfs:seeAlso rdf:resource="http://gcmd.nasa.gov/Resources/valids/archives/keyword_list.html"/>
		<rdfs:seeAlso rdf:resource="http://gcmd.nasa.gov/Resources/valids/archives/keyword_list.html "/>
		<rdfs:seeAlso rdf:resource="http://gcmd.nasa.gov/Resources/valids/archives/keyword_list.html"/>
		<rdfs:seeAlso rdf:resource="http://gcmd.nasa.gov/Resources/valids/archives/keyword_list.html"/>
		<skos:inScheme rdf:resource="http://www.earthobservations.org/GEOSS/EO_Vocabulary"/>
	</skos:Concept>
	<skos:Concept rdf:about="http://www.earthobservations.org/GEOSS/EO_Vocabulary/ocean%20salinity">
		<skos:prefLabel>Ocean Salinity</skos:prefLabel>
		<skos:definition> A measure of the dissolved solids in seawater.</skos:definition>
		<skos:scopeNote>GCMD</skos:scopeNote>
		<skos:broader rdf:resource="http://www.earthobservations.org/GEOSS/EO_Vocabulary/sea%20ice"/>
		<skos:broader rdf:resource="http://www.earthobservations.org/GEOSS/EO_Vocabulary/sea%20ice"/>
		<skos:broader rdf:resource="http://www.earthobservations.org/GEOSS/EO_Vocabulary/salinity%2Fdensity"/>
		<rdfs:seeAlso rdf:resource="http://sweet.jpl.nasa.gov/"/>
		<rdfs:seeAlso rdf:resource="http://his.cuahsi.org/ontologyfiles.html"/>
		<rdfs:seeAlso rdf:resource="http://cf-pcmdi.llnl.gov/documents/cf-standard-names/"/>
		<rdfs:seeAlso rdf:resource="http://webworld.unesco.org/water/ihp/db/glossary/glu/EN/GF1054EN.HTM"/>
		<rdfs:seeAlso rdf:resource="http://stommel.tamu.edu/~baum/paleo/paleogloss/node39.html#SECTION020350000000000000000"/>
		<rdfs:seeAlso rdf:resource="http://earthobservatory.nasa.gov/Glossary/?mode=alpha&amp;seg=s"/>
		<rdfs:seeAlso rdf:resource="http://gcmd.nasa.gov/Resources/valids/archives/keyword_list.html"/>
		<rdfs:seeAlso rdf:resource="http://gcmd.nasa.gov/Resources/valids/archives/keyword_list.html"/>
		<skos:inScheme rdf:resource="http://www.earthobservations.org/GEOSS/EO_Vocabulary"/>
	</skos:Concept>
	<skos:Concept rdf:about="http://www.earthobservations.org/GEOSS/EO_Vocabulary/forest%20litter">
		<skos:prefLabel>Forest Litter</skos:prefLabel>
		<skos:definition>Straw, hay or similar material used as bedding by animals. (Source: CED)</skos:definition>
		<skos:scopeNote>GEMET</skos:scopeNote>
		<skos:broader rdf:resource="http://www.earthobservations.org/GEOSS/EO_Vocabulary/vegetation"/>
		<rdfs:seeAlso rdf:resource="http://sweet.jpl.nasa.gov/"/>
		<skos:inScheme rdf:resource="http://www.earthobservations.org/GEOSS/EO_Vocabulary"/>
	</skos:Concept>
	<skos:Concept rdf:about="http://www.earthobservations.org/GEOSS/EO_Vocabulary/direct%20normal%20irradiation%20%28dni%29">
		<skos:prefLabel>Direct Normal Irradiation (DNI)</skos:prefLabel>
		<skos:definition>To subject to or treat with light or other electromagnetic radiation or with beams of particles. (Source: CED)</skos:definition>
		<skos:scopeNote>GEMET</skos:scopeNote>
		<skos:broader rdf:resource="http://www.earthobservations.org/GEOSS/EO_Vocabulary/atmospheric%20radiation"/>
		<skos:inScheme rdf:resource="http://www.earthobservations.org/GEOSS/EO_Vocabulary"/>
	</skos:Concept>
	<skos:Concept rdf:about="http://www.earthobservations.org/GEOSS/EO_Vocabulary/column%20particulate%20matter%20concentration%20%28coarse%29">
		<skos:prefLabel>Column Particulate Matter Concentration (coarse)</skos:prefLabel>
		<skos:definition>Particulate matter in ice cores (continental dust, volcanic ash, diatoms, and pollen)can provide information on past climate conditions and climate variability.</skos:definition>
		<skos:scopeNote>GCMD</skos:scopeNote>
		<skos:broader rdf:resource="http://www.earthobservations.org/GEOSS/EO_Vocabulary/aerosols"/>
		<skos:broader rdf:resource="http://www.earthobservations.org/GEOSS/EO_Vocabulary/ice%20core%20records"/>
		<rdfs:seeAlso rdf:resource="http://gcmd.nasa.gov/Resources/valids/archives/keyword_list.html"/>
		<rdfs:seeAlso rdf:resource="http://gcmd.nasa.gov/Resources/valids/archives/keyword_list.html"/>
		<skos:inScheme rdf:resource="http://www.earthobservations.org/GEOSS/EO_Vocabulary"/>
	</skos:Concept>
	<skos:Concept rdf:about="http://www.earthobservations.org/GEOSS/EO_Vocabulary/population">
		<skos:prefLabel>Population</skos:prefLabel>
		<skos:definition>Refers to the total number of inhabitants constituting a particular race, class, or group in a specified area.</skos:definition>
		<skos:scopeNote>GCMD</skos:scopeNote>
		<skos:broader rdf:resource="http://www.earthobservations.org/GEOSS/EO_Vocabulary/human%20dimensions"/>
		<rdfs:seeAlso rdf:resource="http://gcmd.nasa.gov/Resources/valids/archives/keyword_list.html"/>
		<skos:inScheme rdf:resource="http://www.earthobservations.org/GEOSS/EO_Vocabulary"/>
	</skos:Concept>
	<skos:Concept rdf:about="http://www.earthobservations.org/GEOSS/EO_Vocabulary/carbon%20%28stores%2C%20uptake%2C%20flux%29">
		<skos:prefLabel>Carbon (stores, uptake, flux)</skos:prefLabel>
		<skos:definition>Carbon is one of three important elements that compose plants. The higher photosynthetic organisms need light, carbon dioxide, and water and these raw materials supply the carbon, oxygen, and hydrogen that are the predominant elements in the organic molecules they manufacture, as well as the energy needed to drive the synthetic reactions.</skos:definition>
		<skos:scopeNote>GCMD</skos:scopeNote>
		<skos:broader rdf:resource="http://www.earthobservations.org/GEOSS/EO_Vocabulary/soils"/>
		<skos:broader rdf:resource="http://www.earthobservations.org/GEOSS/EO_Vocabulary/soils"/>
		<skos:broader rdf:resource="http://www.earthobservations.org/GEOSS/EO_Vocabulary/vegetation"/>
		<skos:broader rdf:resource="http://www.earthobservations.org/GEOSS/EO_Vocabulary/ocean%20chemistry"/>
		<rdfs:seeAlso rdf:resource="http://sweet.jpl.nasa.gov/"/>
		<rdfs:seeAlso rdf:resource="http://gcmd.nasa.gov/Resources/valids/archives/keyword_list.html"/>
		<rdfs:seeAlso rdf:resource="http://gcmd.nasa.gov/Resources/valids/archives/keyword_list.html"/>
		<rdfs:seeAlso rdf:resource="http://gcmd.nasa.gov/Resources/valids/archives/keyword_list.html"/>
		<rdfs:seeAlso rdf:resource="http://gcmd.nasa.gov/Resources/valids/archives/keyword_list.html"/>
		<skos:inScheme rdf:resource="http://www.earthobservations.org/GEOSS/EO_Vocabulary"/>
	</skos:Concept>
	<skos:Concept rdf:about="http://www.earthobservations.org/GEOSS/EO_Vocabulary/contaminants%2Fpollutants%20%28inorganic%2Forganic%29">
		<skos:prefLabel>Contaminants/Pollutants (Inorganic/Organic)</skos:prefLabel>
		<skos:definition>Contaminants are foreign agent that are present, as in water or sediment which may produce a physical or chemical change.</skos:definition>
		<skos:scopeNote>GCMD</skos:scopeNote>
		<skos:broader rdf:resource="http://www.earthobservations.org/GEOSS/EO_Vocabulary/environmental%20impacts"/>
		<skos:broader rdf:resource="http://www.earthobservations.org/GEOSS/EO_Vocabulary/water%20quality%2Fwater%20chemistry"/>
		<skos:broader rdf:resource="http://www.earthobservations.org/GEOSS/EO_Vocabulary/ecological%20dynamics"/>
		<rdfs:seeAlso rdf:resource="http://gcmd.nasa.gov/Resources/valids/archives/keyword_list.html"/>
		<rdfs:seeAlso rdf:resource="http://webworld.unesco.org/water/ihp/db/glossary/glu/EN/GF0919EN.HTM"/>
		<rdfs:seeAlso rdf:resource="http://earthobservatory.nasa.gov/Glossary/?mode=alpha&amp;seg=p"/>
		<skos:inScheme rdf:resource="http://www.earthobservations.org/GEOSS/EO_Vocabulary"/>
	</skos:Concept>
	<skos:Concept rdf:about="http://www.earthobservations.org/GEOSS/EO_Vocabulary/nutrients%20%28phosphorous%2C%20nitrogen%2C%20potassium%2C%20nitrates%2Csulfates%29">
		<skos:prefLabel>Nutrients (Phosphorous, Nitrogen, Potassium, Nitrates,Sulfates)</skos:prefLabel>
		<skos:definition>Nutrients are elements essential for growth and survival of a given organism.Directly or indirectly, nutrients have roles in metabolism that no other nutrients fulfills.</skos:definition>
		<skos:scopeNote>GCMD</skos:scopeNote>
		<skos:broader rdf:resource="http://www.earthobservations.org/GEOSS/EO_Vocabulary/vegetation"/>
		<skos:broader rdf:resource="http://www.earthobservations.org/GEOSS/EO_Vocabulary/water%20quality%2Fwater%20chemistry"/>
		<skos:broader rdf:resource="http://www.earthobservations.org/GEOSS/EO_Vocabulary/ocean%20chemistry"/>
		<rdfs:seeAlso rdf:resource="http://sweet.jpl.nasa.gov/"/>
		<rdfs:seeAlso rdf:resource="http://dias.csis.u-tokyo.ac.jp/dict/gemet/index.php/Nutrient"/>
		<rdfs:seeAlso rdf:resource="http://webworld.unesco.org/water/ihp/db/glossary/glu/EN/GF0849EN.HTM"/>
		<rdfs:seeAlso rdf:resource="http://his.cuahsi.org/ontologyfiles.html"/>
		<rdfs:seeAlso rdf:resource="http://gcmd.nasa.gov/Resources/valids/archives/keyword_list.html"/>
		<rdfs:seeAlso rdf:resource="http://gcmd.nasa.gov/Resources/valids/archives/keyword_list.html"/>
		<skos:inScheme rdf:resource="http://www.earthobservations.org/GEOSS/EO_Vocabulary"/>
	</skos:Concept>
	<skos:Concept rdf:about="http://www.earthobservations.org/GEOSS/EO_Vocabulary/slope%20angle">
		<skos:prefLabel>Slope Angle</skos:prefLabel>
		<skos:definition>N/A</skos:definition>
		<skos:scopeNote>SWEET 2.0 </skos:scopeNote>
		<skos:broader rdf:resource="http://www.earthobservations.org/GEOSS/EO_Vocabulary/erosion%2Fsedimentation"/>
		<skos:broader rdf:resource="http://www.earthobservations.org/GEOSS/EO_Vocabulary/sea%20surface%20topography"/>
		<rdfs:seeAlso rdf:resource="http://sweet.jpl.nasa.gov/"/>
		<rdfs:seeAlso rdf:resource="http://webworld.unesco.org/water/ihp/db/glossary/glu/EN/GF1121EN.HTM"/>
		<rdfs:seeAlso rdf:resource="http://gcmd.nasa.gov/Resources/valids/archives/keyword_list.html"/>
		<skos:inScheme rdf:resource="http://www.earthobservations.org/GEOSS/EO_Vocabulary"/>
	</skos:Concept>
	<skos:Concept rdf:about="http://www.earthobservations.org/GEOSS/EO_Vocabulary/snow%20water%20equivalent%20%28swe%29">
		<skos:prefLabel>Snow Water Equivalent (SWE)</skos:prefLabel>
		<skos:definition>Pertaining to the measurement of the amount of water in a given snow pack.</skos:definition>
		<skos:scopeNote>GCMD</skos:scopeNote>
		<skos:broader rdf:resource="http://www.earthobservations.org/GEOSS/EO_Vocabulary/snow%2Fice"/>
		<skos:broader rdf:resource="http://www.earthobservations.org/GEOSS/EO_Vocabulary/snow%2Fice"/>
		<rdfs:seeAlso rdf:resource="http://gcmd.nasa.gov/Resources/valids/archives/keyword_list.html"/>
		<rdfs:seeAlso rdf:resource="http://his.cuahsi.org/ontologyfiles.html"/>
		<rdfs:seeAlso rdf:resource="http://his.cuahsi.org/ontologyfiles.html"/>
		<skos:inScheme rdf:resource="http://www.earthobservations.org/GEOSS/EO_Vocabulary"/>
	</skos:Concept>
	<skos:Concept rdf:about="http://www.earthobservations.org/GEOSS/EO_Vocabulary/water%20bodies%20%28location%29">
		<skos:prefLabel>Water Bodies (location)</skos:prefLabel>
		<skos:definition>Mass of water distinct from other masses of water.</skos:definition>
		<skos:scopeNote>UNESCO</skos:scopeNote>
		<skos:broader rdf:resource="http://www.earthobservations.org/GEOSS/EO_Vocabulary/terrestrial%20ecosystems"/>
		<skos:broader rdf:resource="http://www.earthobservations.org/GEOSS/EO_Vocabulary/aquatic%20ecosystems"/>
		<rdfs:seeAlso rdf:resource="http://webworld.unesco.org/water/ihp/db/glossary/glu/EN/GF1356EN.HTM"/>
		<skos:inScheme rdf:resource="http://www.earthobservations.org/GEOSS/EO_Vocabulary"/>
	</skos:Concept>
	<skos:Concept rdf:about="http://www.earthobservations.org/GEOSS/EO_Vocabulary/forest%20management%20practices">
		<skos:prefLabel>Forest Management Practices</skos:prefLabel>
		<skos:definition>The application of business methods and technical principles to the operation of a forest property for purposes of a predetermined objective (e.g. maximize revenue, conservation of biotic diversity, etc...).</skos:definition>
		<skos:scopeNote>GCMD</skos:scopeNote>
		<skos:broader rdf:resource="http://www.earthobservations.org/GEOSS/EO_Vocabulary/forest%20science"/>
		<rdfs:seeAlso rdf:resource="http://gcmd.nasa.gov/Resources/valids/archives/keyword_list.html"/>
		<skos:inScheme rdf:resource="http://www.earthobservations.org/GEOSS/EO_Vocabulary"/>
	</skos:Concept>
	<skos:Concept rdf:about="http://www.earthobservations.org/GEOSS/EO_Vocabulary/ice">
		<skos:prefLabel>Ice</skos:prefLabel>
		<skos:definition>The dense substance formed by the freezing of water to the solid state; it commonly occurs in the form of hexagonal crystals. (Source: MGH)</skos:definition>
		<skos:scopeNote>GEMET</skos:scopeNote>
		<skos:broader rdf:resource="http://www.earthobservations.org/GEOSS/EO_Vocabulary/sea%20ice"/>
		<rdfs:seeAlso rdf:resource="http://sweet.jpl.nasa.gov/"/>
		<rdfs:seeAlso rdf:resource="http://webworld.unesco.org/water/ihp/db/glossary/glu/EN/GF0639EN.HTM"/>
		<rdfs:seeAlso rdf:resource="http://stommel.tamu.edu/~baum/paleo/paleogloss/node21.html#SECTION020170000000000000000"/>
		<skos:inScheme rdf:resource="http://www.earthobservations.org/GEOSS/EO_Vocabulary"/>
	</skos:Concept>
	<skos:Concept rdf:about="http://www.earthobservations.org/GEOSS/EO_Vocabulary/column%20nitrogen%20dioxide%20concentration">
		<skos:prefLabel>Column Nitrogen Dioxide Concentration</skos:prefLabel>
		<skos:definition>A reddish-brown, highly poisonous gas, with the chemical formula NO2.</skos:definition>
		<skos:scopeNote>GCMD</skos:scopeNote>
		<skos:broader rdf:resource="http://www.earthobservations.org/GEOSS/EO_Vocabulary/atmospheric%20chemistry"/>
		<skos:broader rdf:resource="http://www.earthobservations.org/GEOSS/EO_Vocabulary/ocean%20chemistry"/>
		<rdfs:seeAlso rdf:resource="http://stommel.tamu.edu/~baum/paleo/paleogloss/node30.html#SECTION020260000000000000000"/>
		<rdfs:seeAlso rdf:resource="http://earthobservatory.nasa.gov/Glossary/?mode=alpha&amp;seg=n"/>
		<rdfs:seeAlso rdf:resource="http://gcmd.nasa.gov/Resources/valids/archives/keyword_list.html"/>
		<skos:inScheme rdf:resource="http://www.earthobservations.org/GEOSS/EO_Vocabulary"/>
	</skos:Concept>
	<skos:Concept rdf:about="http://www.earthobservations.org/GEOSS/EO_Vocabulary/snow%20depth">
		<skos:prefLabel>Snow Depth</skos:prefLabel>
		<skos:definition>Pertaining to the thickness of snow pack throughout the year.</skos:definition>
		<skos:scopeNote>GCMD</skos:scopeNote>
		<skos:broader rdf:resource="http://www.earthobservations.org/GEOSS/EO_Vocabulary/sea%20ice"/>
		<skos:broader rdf:resource="http://www.earthobservations.org/GEOSS/EO_Vocabulary/snow%2Fice"/>
		<skos:broader rdf:resource="http://www.earthobservations.org/GEOSS/EO_Vocabulary/sea%20ice"/>
		<skos:broader rdf:resource="http://www.earthobservations.org/GEOSS/EO_Vocabulary/snow%2Fice"/>
		<rdfs:seeAlso rdf:resource="http://webworld.unesco.org/water/ihp/db/glossary/glu/EN/GF1132EN.HTM"/>
		<rdfs:seeAlso rdf:resource="http://gcmd.nasa.gov/Resources/valids/archives/keyword_list.html"/>
		<rdfs:seeAlso rdf:resource="http://cf-pcmdi.llnl.gov/documents/cf-standard-names/"/>
		<rdfs:seeAlso rdf:resource="http://his.cuahsi.org/ontologyfiles.html"/>
		<rdfs:seeAlso rdf:resource="http://his.cuahsi.org/ontologyfiles.html"/>
		<skos:inScheme rdf:resource="http://www.earthobservations.org/GEOSS/EO_Vocabulary"/>
	</skos:Concept>
	<skos:Concept rdf:about="http://www.earthobservations.org/GEOSS/EO_Vocabulary/cloud%20parameters%20%28other%29">
		<skos:prefLabel>Cloud Parameters (Other)</skos:prefLabel>
		<skos:definition>Coefficient in some hydrological model, formula or other relationship which may be adjusted to apply the general model, etc. to particular cases. For example fitting a rainfall-runoff model to a particular catchment will involve determining parameter values appropriate to that catchment.</skos:definition>
		<skos:scopeNote>UNESCO</skos:scopeNote>
		<skos:broader rdf:resource="http://www.earthobservations.org/GEOSS/EO_Vocabulary/clouds"/>
		<rdfs:seeAlso rdf:resource="http://webworld.unesco.org/water/ihp/db/glossary/glu/EN/GF0878EN.HTM"/>
		<skos:inScheme rdf:resource="http://www.earthobservations.org/GEOSS/EO_Vocabulary"/>
	</skos:Concept>
	<skos:Concept rdf:about="http://www.earthobservations.org/GEOSS/EO_Vocabulary/forest%20structure">
		<skos:prefLabel>Forest Structure</skos:prefLabel>
		<skos:definition>Forest Composition refers to the tree species which make up the forest. Vegetation Structure refers to the vertical arrangement of canopy layers and plants of different life forms, or the horizontal variation in canopy closure and canopy layers, or both. Vegetation Structure also includes standing dead trees (snags) and decaying logs on the ground (coarse woody debris).</skos:definition>
		<skos:scopeNote>GCMD</skos:scopeNote>
		<skos:broader rdf:resource="http://www.earthobservations.org/GEOSS/EO_Vocabulary/forest%20science"/>
		<skos:broader rdf:resource="http://www.earthobservations.org/GEOSS/EO_Vocabulary/vegetation"/>
		<rdfs:seeAlso rdf:resource="http://sweet.jpl.nasa.gov/"/>
		<rdfs:seeAlso rdf:resource="http://gcmd.nasa.gov/Resources/valids/archives/keyword_list.html "/>
		<skos:inScheme rdf:resource="http://www.earthobservations.org/GEOSS/EO_Vocabulary"/>
	</skos:Concept>
	<skos:Concept rdf:about="http://www.earthobservations.org/GEOSS/EO_Vocabulary/sea%20ice%20cover">
		<skos:prefLabel>Sea Ice Cover</skos:prefLabel>
		<skos:definition> Pertaining to the study of frozen seawater over the ocean surface.</skos:definition>
		<skos:scopeNote>GCMD</skos:scopeNote>
		<skos:broader rdf:resource="http://www.earthobservations.org/GEOSS/EO_Vocabulary/sea%20ice"/>
		<skos:broader rdf:resource="http://www.earthobservations.org/GEOSS/EO_Vocabulary/sea%20ice"/>
		<rdfs:seeAlso rdf:resource="http://gcmd.nasa.gov/Resources/valids/archives/keyword_list.html"/>
		<skos:inScheme rdf:resource="http://www.earthobservations.org/GEOSS/EO_Vocabulary"/>
	</skos:Concept>
	<skos:Concept rdf:about="http://www.earthobservations.org/GEOSS/EO_Vocabulary/surface%20deformation">
		<skos:prefLabel>Surface Deformation</skos:prefLabel>
		<skos:definition>N/A</skos:definition>
		<skos:scopeNote>SWEET 2.0 </skos:scopeNote>
		<skos:broader rdf:resource="http://www.earthobservations.org/GEOSS/EO_Vocabulary/geodetics%2Fgravity"/>
		<skos:broader rdf:resource="http://www.earthobservations.org/GEOSS/EO_Vocabulary/geodetics%2Fgravity"/>
		<skos:broader rdf:resource="http://www.earthobservations.org/GEOSS/EO_Vocabulary/geomorphology"/>
		<skos:broader rdf:resource="http://www.earthobservations.org/GEOSS/EO_Vocabulary/geomorphology"/>
		<rdfs:seeAlso rdf:resource="http://sweet.jpl.nasa.gov/"/>
		<rdfs:seeAlso rdf:resource="http://gcmd.nasa.gov/Resources/valids/archives/keyword_list.html "/>
		<rdfs:seeAlso rdf:resource="http://gcmd.nasa.gov/Resources/valids/archives/keyword_list.html"/>
		<rdfs:seeAlso rdf:resource="http://gcmd.nasa.gov/Resources/valids/archives/keyword_list.html"/>
		<skos:inScheme rdf:resource="http://www.earthobservations.org/GEOSS/EO_Vocabulary"/>
	</skos:Concept>
	<skos:Concept rdf:about="http://www.earthobservations.org/GEOSS/EO_Vocabulary/surface%20radiation%20budget">
		<skos:prefLabel>Surface Radiation Budget</skos:prefLabel>
		<skos:definition>A measure of all the inputs and outputs of radiative energy relative to a system, such as Earth. See Earth Radiation Budget Experiment.</skos:definition>
		<skos:scopeNote>NASA</skos:scopeNote>
		<skos:broader rdf:resource="http://www.earthobservations.org/GEOSS/EO_Vocabulary/atmospheric%20pressure"/>
		<rdfs:seeAlso rdf:resource="http://earthobservatory.nasa.gov/Glossary/?mode=alpha&amp;seg=q&amp;segend=s"/>
		<skos:inScheme rdf:resource="http://www.earthobservations.org/GEOSS/EO_Vocabulary"/>
	</skos:Concept>
	<skos:Concept rdf:about="http://www.earthobservations.org/GEOSS/EO_Vocabulary/soil%20thickness">
		<skos:prefLabel>Soil Thickness</skos:prefLabel>
		<skos:definition>N/A</skos:definition>
		<skos:scopeNote>SWEET 2.0 </skos:scopeNote>
		<skos:broader rdf:resource="http://www.earthobservations.org/GEOSS/EO_Vocabulary/soils"/>
		<skos:broader rdf:resource="http://www.earthobservations.org/GEOSS/EO_Vocabulary/soils"/>
		<skos:broader rdf:resource="http://www.earthobservations.org/GEOSS/EO_Vocabulary/soils"/>
		<rdfs:seeAlso rdf:resource="http://sweet.jpl.nasa.gov/"/>
		<rdfs:seeAlso rdf:resource="http://cf-pcmdi.llnl.gov/documents/cf-standard-names/"/>
		<rdfs:seeAlso rdf:resource="http://gcmd.nasa.gov/Resources/valids/archives/keyword_list.html"/>
		<skos:inScheme rdf:resource="http://www.earthobservations.org/GEOSS/EO_Vocabulary"/>
	</skos:Concept>
	<skos:Concept rdf:about="http://www.earthobservations.org/GEOSS/EO_Vocabulary/ecosystem%20function%2Fdynamics">
		<skos:prefLabel>Ecosystem Function/Dynamics</skos:prefLabel>
		<skos:definition>Ecosystem functions are the physical, chemical, biological, and man-made processes that contribute to the self-maintenance of an ecosystem.</skos:definition>
		<skos:scopeNote>GCMD</skos:scopeNote>
		<skos:broader rdf:resource="http://www.earthobservations.org/GEOSS/EO_Vocabulary/ecological%20dynamics"/>
		<rdfs:seeAlso rdf:resource="http://gcmd.nasa.gov/Resources/valids/archives/keyword_list.html"/>
		<skos:inScheme rdf:resource="http://www.earthobservations.org/GEOSS/EO_Vocabulary"/>
	</skos:Concept>
	<skos:Concept rdf:about="http://www.earthobservations.org/GEOSS/EO_Vocabulary/species%20composition">
		<skos:prefLabel>Species Composition</skos:prefLabel>
		<skos:definition>N/A</skos:definition>
		<skos:scopeNote>SWEET 2.0 </skos:scopeNote>
		<skos:broader rdf:resource="http://www.earthobservations.org/GEOSS/EO_Vocabulary/vegetation"/>
		<rdfs:seeAlso rdf:resource="http://sweet.jpl.nasa.gov/"/>
		<skos:inScheme rdf:resource="http://www.earthobservations.org/GEOSS/EO_Vocabulary"/>
	</skos:Concept>
	<skos:Concept rdf:about="http://www.earthobservations.org/GEOSS/EO_Vocabulary/aerosol%20properties">
		<skos:prefLabel>Aerosol Properties</skos:prefLabel>
		<skos:definition>Particles of liquid or solid dispersed as a suspension in gas.</skos:definition>
		<skos:scopeNote>NASA</skos:scopeNote>
		<skos:broader rdf:resource="http://www.earthobservations.org/GEOSS/EO_Vocabulary/aerosols"/>
		<skos:broader rdf:resource="http://www.earthobservations.org/GEOSS/EO_Vocabulary/atmospheric%20water%20vapor"/>
		<skos:broader rdf:resource="http://www.earthobservations.org/GEOSS/EO_Vocabulary/aerosols"/>
		<rdfs:seeAlso rdf:resource="http://sweet.jpl.nasa.gov/"/>
		<rdfs:seeAlso rdf:resource="http://stommel.tamu.edu/~baum/paleo/paleogloss/node5.html#SECTION02010000000000000000"/>
		<rdfs:seeAlso rdf:resource="http://earthobservatory.nasa.gov/Glossary/?mode=alpha&amp;seg=a"/>
		<rdfs:seeAlso rdf:resource="http://gcmd.nasa.gov/Resources/valids/archives/keyword_list.html"/>
		<skos:inScheme rdf:resource="http://www.earthobservations.org/GEOSS/EO_Vocabulary"/>
	</skos:Concept>
	<skos:Concept rdf:about="http://www.earthobservations.org/GEOSS/EO_Vocabulary/ambient%20nitrogen%20dioxide%20concentration">
		<skos:prefLabel>Ambient Nitrogen Dioxide Concentration</skos:prefLabel>
		<skos:definition>GCMD</skos:definition>
		<skos:scopeNote>GCMD</skos:scopeNote>
		<skos:broader rdf:resource="http://www.earthobservations.org/GEOSS/EO_Vocabulary/atmospheric%20chemistry"/>
		<skos:broader rdf:resource="http://www.earthobservations.org/GEOSS/EO_Vocabulary/ocean%20chemistry"/>
		<rdfs:seeAlso rdf:resource="http://stommel.tamu.edu/~baum/paleo/paleogloss/node30.html#SECTION020260000000000000000"/>
		<rdfs:seeAlso rdf:resource="http://earthobservatory.nasa.gov/Glossary/?mode=alpha&amp;seg=n"/>
		<rdfs:seeAlso rdf:resource="http://gcmd.nasa.gov/Resources/valids/archives/keyword_list.html"/>
		<skos:inScheme rdf:resource="http://www.earthobservations.org/GEOSS/EO_Vocabulary"/>
	</skos:Concept>
	<skos:Concept rdf:about="http://www.earthobservations.org/GEOSS/EO_Vocabulary/ambient%20sulfur%20dioxide%20concentration">
		<skos:prefLabel>Ambient Sulfur Dioxide Concentration</skos:prefLabel>
		<skos:definition>Sulfur dioxide (SO2) is a non-inflammable colorless gas. SO2 is usually oxidized by ozone and hydrogen peroxide to form sulfur trioxide, a secondary pollutant that is extremely soluble in water. Droplets of sulfuric acid (acid rain) are formed when sulfur oxides are present in the atmosphere . The production of SO2 originating from coal-fired power plants and other fossil fuel combustion is largely responsible for the damage caused by acid rain. Volcanic eruptions also provide a source of sulfur dioxide in the atmosphere but are insignificant when compared to anthropogenic sources. [Science; v265; 497-9; 1994.] [Nature; v366;327-9; 1993.]</skos:definition>
		<skos:scopeNote>GCMD</skos:scopeNote>
		<skos:broader rdf:resource="http://www.earthobservations.org/GEOSS/EO_Vocabulary/atmospheric%20chemistry"/>
		<rdfs:seeAlso rdf:resource="http://his.cuahsi.org/ontologyfiles.html"/>
		<rdfs:seeAlso rdf:resource="http://earthobservatory.nasa.gov/Glossary/?mode=alpha&amp;seg=s"/>
		<rdfs:seeAlso rdf:resource="http://gcmd.nasa.gov/Resources/valids/archives/keyword_list.html"/>
		<skos:inScheme rdf:resource="http://www.earthobservations.org/GEOSS/EO_Vocabulary"/>
	</skos:Concept>
	<skos:Concept rdf:about="http://www.earthobservations.org/GEOSS/EO_Vocabulary/curvature">
		<skos:prefLabel>Curvature</skos:prefLabel>
		<skos:definition>The fact of being curved or the degree to which something is curved</skos:definition>
		<skos:scopeNote>Oxford Dictionaries</skos:scopeNote>
		<skos:broader rdf:resource="http://www.earthobservations.org/GEOSS/EO_Vocabulary/bathymetry%2Fseafloor%20topography"/>
		<rdfs:seeAlso rdf:resource="http://sweet.jpl.nasa.gov/"/>
		<rdfs:seeAlso rdf:resource="http://oxforddictionaries.com/view/entry/m_en_gb0198820#m_en_gb0198820"/>
		<skos:inScheme rdf:resource="http://www.earthobservations.org/GEOSS/EO_Vocabulary"/>
	</skos:Concept>
	<skos:Concept rdf:about="http://www.earthobservations.org/GEOSS/EO_Vocabulary/pore%20pressure">
		<skos:prefLabel>Pore Pressure</skos:prefLabel>
		<skos:definition>A type of stress which is exerted uniformly in all directions; its measure is the force exerted per unit area. (Source: MGH)</skos:definition>
		<skos:scopeNote>GEMET</skos:scopeNote>
		<skos:broader rdf:resource="http://www.earthobservations.org/GEOSS/EO_Vocabulary/marine%20sediments"/>
		<skos:inScheme rdf:resource="http://www.earthobservations.org/GEOSS/EO_Vocabulary"/>
	</skos:Concept>
	<skos:Concept rdf:about="http://www.earthobservations.org/GEOSS/EO_Vocabulary/rock%20strength%2C%20permeability%2C%20spacing%2C%20orientation">
		<skos:prefLabel>Rock Strength, Permeability, Spacing, Orientation</skos:prefLabel>
		<skos:definition>N/A</skos:definition>
		<skos:scopeNote>SWEET 2.0 </skos:scopeNote>
		<skos:broader rdf:resource="http://www.earthobservations.org/GEOSS/EO_Vocabulary/rocks%2Fminerals%C2%A0"/>
		<rdfs:seeAlso rdf:resource="http://sweet.jpl.nasa.gov/"/>
		<rdfs:seeAlso rdf:resource="http://sweet.jpl.nasa.gov/"/>
		<skos:inScheme rdf:resource="http://www.earthobservations.org/GEOSS/EO_Vocabulary"/>
	</skos:Concept>
	<skos:Concept rdf:about="http://www.earthobservations.org/GEOSS/EO_Vocabulary/slip">
		<skos:prefLabel>Slip</skos:prefLabel>
		<skos:definition>A creamy mixture of clay, water, and typically a pigment of some kind, used especially for decorating earthenware.</skos:definition>
		<skos:scopeNote>Oxford Dictionaries</skos:scopeNote>
		<skos:broader rdf:resource="http://www.earthobservations.org/GEOSS/EO_Vocabulary/seismology"/>
		<rdfs:seeAlso rdf:resource="http://sweet.jpl.nasa.gov/"/>
		<rdfs:seeAlso rdf:resource="http://oxforddictionaries.com/view/entry/m_en_gb0781600?rskey=IUZD0N&amp;result=3#m_en_gb0781600"/>
		<skos:inScheme rdf:resource="http://www.earthobservations.org/GEOSS/EO_Vocabulary"/>
	</skos:Concept>
	<skos:Concept rdf:about="http://www.earthobservations.org/GEOSS/EO_Vocabulary/slope%20movement">
		<skos:prefLabel>Slope Movement</skos:prefLabel>
		<skos:definition>An act of moving</skos:definition>
		<skos:scopeNote>Oxford Dictionaries</skos:scopeNote>
		<skos:broader rdf:resource="http://www.earthobservations.org/GEOSS/EO_Vocabulary/erosion%2Fsedimentation"/>
		<rdfs:seeAlso rdf:resource="http://oxforddictionaries.com/view/entry/m_en_gb0538270#m_en_gb0538270"/>
		<skos:inScheme rdf:resource="http://www.earthobservations.org/GEOSS/EO_Vocabulary"/>
	</skos:Concept>
	<skos:Concept rdf:about="http://www.earthobservations.org/GEOSS/EO_Vocabulary/strain">
		<skos:prefLabel>Strain</skos:prefLabel>
		<skos:definition> Pertaining to the measurement, analysis, or modeling of strain that has occurred in the Earth's crust, either through in-situ measurements, or through laboratory experiments.</skos:definition>
		<skos:scopeNote>GCMD</skos:scopeNote>
		<skos:broader rdf:resource="http://www.earthobservations.org/GEOSS/EO_Vocabulary/tectonics%C2%A0"/>
		<rdfs:seeAlso rdf:resource="http://gcmd.nasa.gov/Resources/valids/archives/keyword_list.html"/>
		<skos:inScheme rdf:resource="http://www.earthobservations.org/GEOSS/EO_Vocabulary"/>
	</skos:Concept>
	<skos:Concept rdf:about="http://www.earthobservations.org/GEOSS/EO_Vocabulary/carbon%20dioxide%20concentration">
		<skos:prefLabel>Carbon Dioxide Concentration</skos:prefLabel>
		<skos:definition>A gaseous compound of one carbon atom and two oxygen atoms, CO2. It is colorless, odorless, incombustible, and is soluble in water. Its dissolution in seawater is important to understanding the global carbon cycle.</skos:definition>
		<skos:scopeNote>GCMD</skos:scopeNote>
		<skos:broader rdf:resource="http://www.earthobservations.org/GEOSS/EO_Vocabulary/atmospheric%20chemistry"/>
		<skos:broader rdf:resource="http://www.earthobservations.org/GEOSS/EO_Vocabulary/water%20quality%2Fwater%20chemistry"/>
		<skos:broader rdf:resource="http://www.earthobservations.org/GEOSS/EO_Vocabulary/ocean%20chemistry"/>
		<skos:broader rdf:resource="http://www.earthobservations.org/GEOSS/EO_Vocabulary/ice%20core%20records"/>
		<rdfs:seeAlso rdf:resource="http://stommel.tamu.edu/~baum/paleo/paleogloss/node9.html#SECTION02050000000000000000"/>
		<rdfs:seeAlso rdf:resource="http://earthobservatory.nasa.gov/Glossary/?mode=alpha&amp;seg=b&amp;segend=d"/>
		<rdfs:seeAlso rdf:resource="http://gcmd.nasa.gov/Resources/valids/archives/keyword_list.html"/>
		<rdfs:seeAlso rdf:resource="http://gcmd.nasa.gov/Resources/valids/archives/keyword_list.html"/>
		<rdfs:seeAlso rdf:resource="http://gcmd.nasa.gov/Resources/valids/archives/keyword_list.html"/>
		<rdfs:seeAlso rdf:resource="http://cf-pcmdi.llnl.gov/documents/cf-standard-names/"/>
		<skos:inScheme rdf:resource="http://www.earthobservations.org/GEOSS/EO_Vocabulary"/>
	</skos:Concept>
	<skos:Concept rdf:about="http://www.earthobservations.org/GEOSS/EO_Vocabulary/ice%20depth">
		<skos:prefLabel>Ice Depth</skos:prefLabel>
		<skos:definition> Ice depth or thickness refers to the extent of the ice below the surface of the water. The term is also used in river and lake ice studies. Remote sensing techniques (particularly radar and microwave) have been used to estimate ice thickness as have recently declassified submarine measurements of polar ice thickness.</skos:definition>
		<skos:scopeNote>GCMD</skos:scopeNote>
		<skos:broader rdf:resource="http://www.earthobservations.org/GEOSS/EO_Vocabulary/sea%20ice"/>
		<skos:broader rdf:resource="http://www.earthobservations.org/GEOSS/EO_Vocabulary/sea%20ice"/>
		<skos:broader rdf:resource="http://www.earthobservations.org/GEOSS/EO_Vocabulary/snow%2Fice"/>
		<skos:broader rdf:resource="http://www.earthobservations.org/GEOSS/EO_Vocabulary/snow%2Fice"/>
		<rdfs:seeAlso rdf:resource="http://cf-pcmdi.llnl.gov/documents/cf-standard-names/"/>
		<rdfs:seeAlso rdf:resource="http://gcmd.nasa.gov/Resources/valids/archives/keyword_list.html"/>
		<rdfs:seeAlso rdf:resource="http://gcmd.nasa.gov/Resources/valids/archives/keyword_list.html"/>
		<skos:inScheme rdf:resource="http://www.earthobservations.org/GEOSS/EO_Vocabulary"/>
	</skos:Concept>
	<skos:Concept rdf:about="http://www.earthobservations.org/GEOSS/EO_Vocabulary/impervious%20surface%20extent">
		<skos:prefLabel>Impervious Surface Extent</skos:prefLabel>
		<skos:definition>The area covered by something</skos:definition>
		<skos:scopeNote>Oxford Dictionaries</skos:scopeNote>
		<skos:broader rdf:resource="http://www.earthobservations.org/GEOSS/EO_Vocabulary/sea%20ice"/>
		<skos:broader rdf:resource="http://www.earthobservations.org/GEOSS/EO_Vocabulary/snow%2Fice"/>
		<skos:broader rdf:resource="http://www.earthobservations.org/GEOSS/EO_Vocabulary/sea%20ice"/>
		<skos:broader rdf:resource="http://www.earthobservations.org/GEOSS/EO_Vocabulary/geomorphology"/>
		<skos:broader rdf:resource="http://www.earthobservations.org/GEOSS/EO_Vocabulary/geomorphology"/>
		<rdfs:seeAlso rdf:resource="http://stommel.tamu.edu/~baum/paleo/paleogloss/node40.html#SECTION020360000000000000000"/>
		<rdfs:seeAlso rdf:resource="http://gcmd.nasa.gov/Resources/valids/archives/keyword_list.html"/>
		<rdfs:seeAlso rdf:resource="http://gcmd.nasa.gov/Resources/valids/archives/keyword_list.html"/>
		<skos:inScheme rdf:resource="http://www.earthobservations.org/GEOSS/EO_Vocabulary"/>
	</skos:Concept>
	<skos:Concept rdf:about="http://www.earthobservations.org/GEOSS/EO_Vocabulary/surface%20albedo">
		<skos:prefLabel>Surface Albedo</skos:prefLabel>
		<skos:definition>The surface called "surface" means the lower boundary of the atmosphere. 1 84 E174</skos:definition>
		<skos:scopeNote>CF Standard</skos:scopeNote>
		<skos:broader rdf:resource="http://www.earthobservations.org/GEOSS/EO_Vocabulary/atmospheric%20temperature"/>
		<skos:broader rdf:resource="http://www.earthobservations.org/GEOSS/EO_Vocabulary/atmospheric%20radiation"/>
		<rdfs:seeAlso rdf:resource="http://cf-pcmdi.llnl.gov/documents/cf-standard-names/"/>
		<skos:inScheme rdf:resource="http://www.earthobservations.org/GEOSS/EO_Vocabulary"/>
	</skos:Concept>
	<skos:Concept rdf:about="http://www.earthobservations.org/GEOSS/EO_Vocabulary/wave%20direction">
		<skos:prefLabel>Wave Direction</skos:prefLabel>
		<skos:definition>Wave speed: Distance a wave travels per time. Wave direction: The line along which a wave travels with respect to its compass heading. Both Wave Speed and Wave Direction may be included as Detailed Variables under Wave Speed/Direction.</skos:definition>
		<skos:scopeNote>GCMD</skos:scopeNote>
		<skos:broader rdf:resource="http://www.earthobservations.org/GEOSS/EO_Vocabulary/ocean%20waves"/>
		<rdfs:seeAlso rdf:resource="http://gcmd.nasa.gov/Resources/valids/archives/keyword_list.html"/>
		<skos:inScheme rdf:resource="http://www.earthobservations.org/GEOSS/EO_Vocabulary"/>
	</skos:Concept>
	<skos:Concept rdf:about="http://www.earthobservations.org/GEOSS/EO_Vocabulary/wave%20height">
		<skos:prefLabel>Wave Height</skos:prefLabel>
		<skos:definition>Vertical distance between a wave crest and the adjacent wave troughs.</skos:definition>
		<skos:scopeNote>GCMD</skos:scopeNote>
		<skos:broader rdf:resource="http://www.earthobservations.org/GEOSS/EO_Vocabulary/ocean%20waves"/>
		<rdfs:seeAlso rdf:resource="http://his.cuahsi.org/ontologyfiles.html"/>
		<rdfs:seeAlso rdf:resource="http://gcmd.nasa.gov/Resources/valids/archives/keyword_list.html"/>
		<skos:inScheme rdf:resource="http://www.earthobservations.org/GEOSS/EO_Vocabulary"/>
	</skos:Concept>
	<skos:Concept rdf:about="http://www.earthobservations.org/GEOSS/EO_Vocabulary/wave%20period">
		<skos:prefLabel>Wave Period</skos:prefLabel>
		<skos:definition>The time for successive wave crests to pass a fixed point.</skos:definition>
		<skos:scopeNote>GCMD</skos:scopeNote>
		<skos:broader rdf:resource="http://www.earthobservations.org/GEOSS/EO_Vocabulary/ocean%20waves"/>
		<rdfs:seeAlso rdf:resource="http://his.cuahsi.org/ontologyfiles.html"/>
		<rdfs:seeAlso rdf:resource="http://gcmd.nasa.gov/Resources/valids/archives/keyword_list.html "/>
		<skos:inScheme rdf:resource="http://www.earthobservations.org/GEOSS/EO_Vocabulary"/>
	</skos:Concept>
	<skos:Concept rdf:about="http://www.earthobservations.org/GEOSS/EO_Vocabulary/vector%20population">
		<skos:prefLabel>Vector Population</skos:prefLabel>
		<skos:definition>N/A</skos:definition>
		<skos:scopeNote>SWEET 2.0 </skos:scopeNote>
		<skos:broader rdf:resource="http://www.earthobservations.org/GEOSS/EO_Vocabulary/boundaries"/>
		<skos:broader rdf:resource="http://www.earthobservations.org/GEOSS/EO_Vocabulary/land%20use%2Fland%20cover"/>
		<rdfs:seeAlso rdf:resource="http://sweet.jpl.nasa.gov/"/>
		<skos:inScheme rdf:resource="http://www.earthobservations.org/GEOSS/EO_Vocabulary"/>
	</skos:Concept>
	<skos:Concept rdf:about="http://www.earthobservations.org/GEOSS/EO_Vocabulary/fuel%20load%2Fcharacteristics">
		<skos:prefLabel>Fuel Load/Characteristics</skos:prefLabel>
		<skos:definition>N/A</skos:definition>
		<skos:scopeNote>SWEET 2.0 </skos:scopeNote>
		<skos:broader rdf:resource="http://www.earthobservations.org/GEOSS/EO_Vocabulary/natural%20resources"/>
		<skos:broader rdf:resource="http://www.earthobservations.org/GEOSS/EO_Vocabulary/environmental%20impacts"/>
		<rdfs:seeAlso rdf:resource="http://sweet.jpl.nasa.gov/"/>
		<rdfs:seeAlso rdf:resource="http://sweet.jpl.nasa.gov/"/>
		<skos:inScheme rdf:resource="http://www.earthobservations.org/GEOSS/EO_Vocabulary"/>
	</skos:Concept>
	<skos:Concept rdf:about="http://www.earthobservations.org/GEOSS/EO_Vocabulary/chlorophyll">
		<skos:prefLabel>Chlorophyll</skos:prefLabel>
		<skos:definition> Chlorophyll is the green pigment in plants responsible for absorbing the light energy required for photosynthesis.</skos:definition>
		<skos:scopeNote>GCMD</skos:scopeNote>
		<skos:broader rdf:resource="http://www.earthobservations.org/GEOSS/EO_Vocabulary/vegetation"/>
		<skos:broader rdf:resource="http://www.earthobservations.org/GEOSS/EO_Vocabulary/ocean%20chemistry"/>
		<skos:broader rdf:resource="http://www.earthobservations.org/GEOSS/EO_Vocabulary/water%20quality%2Fwater%20chemistry"/>
		<skos:broader rdf:resource="http://www.earthobservations.org/GEOSS/EO_Vocabulary/ocean%20chemistry"/>
		<rdfs:seeAlso rdf:resource="http://sweet.jpl.nasa.gov/"/>
		<rdfs:seeAlso rdf:resource="http://his.cuahsi.org/ontologyfiles.html"/>
		<rdfs:seeAlso rdf:resource="http://earthobservatory.nasa.gov/Glossary/?mode=alpha&amp;seg=b&amp;segend=d"/>
		<rdfs:seeAlso rdf:resource="http://gcmd.nasa.gov/Resources/valids/archives/keyword_list.html"/>
		<skos:inScheme rdf:resource="http://www.earthobservations.org/GEOSS/EO_Vocabulary"/>
	</skos:Concept>
	<skos:Concept rdf:about="http://www.earthobservations.org/GEOSS/EO_Vocabulary/erosion%20%28reefs%2C%20sandbars%29">
		<skos:prefLabel>Erosion (reefs, sandbars)</skos:prefLabel>
		<skos:definition>The process by which soil, rock or sand is gradually worn away by water or wind action.</skos:definition>
		<skos:scopeNote>GCMD</skos:scopeNote>
		<skos:broader rdf:resource="http://www.earthobservations.org/GEOSS/EO_Vocabulary/erosion%2Fsedimentation"/>
		<skos:broader rdf:resource="http://www.earthobservations.org/GEOSS/EO_Vocabulary/coastal%20processes"/>
		<rdfs:seeAlso rdf:resource="http://sweet.jpl.nasa.gov/"/>
		<rdfs:seeAlso rdf:resource="http://webworld.unesco.org/water/ihp/db/glossary/glu/EN/GF0414EN.HTM"/>
		<rdfs:seeAlso rdf:resource="http://gcmd.nasa.gov/Resources/valids/archives/keyword_list.html"/>
		<rdfs:seeAlso rdf:resource="http://gcmd.nasa.gov/Resources/valids/archives/keyword_list.html"/>
		<skos:inScheme rdf:resource="http://www.earthobservations.org/GEOSS/EO_Vocabulary"/>
	</skos:Concept>
	<skos:Concept rdf:about="http://www.earthobservations.org/GEOSS/EO_Vocabulary/fish%20harvest%20intensity">
		<skos:prefLabel>Fish Harvest Intensity</skos:prefLabel>
		<skos:definition>The measurable amount of a property, such as force , brightness, or a magnetic field</skos:definition>
		<skos:scopeNote>Oxford Dictionaries</skos:scopeNote>
		<skos:broader rdf:resource="http://www.earthobservations.org/GEOSS/EO_Vocabulary/aquatic%20ecosystems"/>
		<skos:broader rdf:resource="http://www.earthobservations.org/GEOSS/EO_Vocabulary/terrestrial%20ecosystems"/>
		<rdfs:seeAlso rdf:resource="http://sweet.jpl.nasa.gov/"/>
		<skos:inScheme rdf:resource="http://www.earthobservations.org/GEOSS/EO_Vocabulary"/>
	</skos:Concept>
	<skos:Concept rdf:about="http://www.earthobservations.org/GEOSS/EO_Vocabulary/water%20depth%20%28shallow%20near-shore%29">
		<skos:prefLabel>Water Depth (Shallow Near-Shore)</skos:prefLabel>
		<skos:definition>The measurement of the vertical distance from the surface of a body of water to the floor.</skos:definition>
		<skos:scopeNote>GCMD</skos:scopeNote>
		<skos:broader rdf:resource="http://www.earthobservations.org/GEOSS/EO_Vocabulary/bathymetry%2Fseafloor%20topography"/>
		<skos:broader rdf:resource="http://www.earthobservations.org/GEOSS/EO_Vocabulary/surface%20water"/>
		<rdfs:seeAlso rdf:resource="http://gcmd.nasa.gov/Resources/valids/archives/keyword_list.html"/>
		<rdfs:seeAlso rdf:resource="http://gcmd.nasa.gov/Resources/valids/archives/keyword_list.html"/>
		<skos:inScheme rdf:resource="http://www.earthobservations.org/GEOSS/EO_Vocabulary"/>
	</skos:Concept>
	<skos:Concept rdf:about="http://www.earthobservations.org/GEOSS/EO_Vocabulary/column%20sulfur%20dioxide%20concentration">
		<skos:prefLabel>Column Sulfur Dioxide Concentration</skos:prefLabel>
		<skos:definition>Sulfur dioxide (SO2) is a non-inflammable colorless gas. SO2 is usually oxidized by ozone and hydrogen peroxide to form sulfur trioxide, a secondary pollutant that is extremely soluble in water. Droplets of sulfuric acid (acid rain) are formed when sulfur oxides are present in the atmosphere. The production of SO2 originating from coal-fired power plants and other fossil fuel combustion is largely responsible for the damage caused by acid rain. Volcanic eruptions also provide a source of sulfur dioxide in the atmosphere but are insignificant when compared to anthropogenic sources. [Science; v265; 497-9; 1994.] [Nature; v366;327-9; 1993.]</skos:definition>
		<skos:scopeNote>GCMD</skos:scopeNote>
		<skos:broader rdf:resource="http://www.earthobservations.org/GEOSS/EO_Vocabulary/atmospheric%20chemistry"/>
		<rdfs:seeAlso rdf:resource="http://his.cuahsi.org/ontologyfiles.html"/>
		<rdfs:seeAlso rdf:resource="http://earthobservatory.nasa.gov/Glossary/?mode=alpha&amp;seg=s"/>
		<rdfs:seeAlso rdf:resource="http://gcmd.nasa.gov/Resources/valids/archives/keyword_list.html"/>
		<skos:inScheme rdf:resource="http://www.earthobservations.org/GEOSS/EO_Vocabulary"/>
	</skos:Concept>
	<skos:Concept rdf:about="http://www.earthobservations.org/GEOSS/EO_Vocabulary/source%20of%20drinking%20water">
		<skos:prefLabel>Source of Drinking Water</skos:prefLabel>
		<skos:definition>Water that is agreeable to drink, does not present health hazards and whose quality is normally regulated by legislation. (Source: GUNN)</skos:definition>
		<skos:scopeNote>GEMET</skos:scopeNote>
		<skos:broader rdf:resource="http://www.earthobservations.org/GEOSS/EO_Vocabulary/human%20health"/>
		<skos:broader rdf:resource="http://www.earthobservations.org/GEOSS/EO_Vocabulary/surface%20water"/>
		<skos:broader rdf:resource="http://www.earthobservations.org/GEOSS/EO_Vocabulary/water%C2%A0quality%2Fwater%20chemistry"/>
		<rdfs:seeAlso rdf:resource="http://sweet.jpl.nasa.gov/"/>
		<skos:inScheme rdf:resource="http://www.earthobservations.org/GEOSS/EO_Vocabulary"/>
	</skos:Concept>
	<skos:Concept rdf:about="http://www.earthobservations.org/GEOSS/EO_Vocabulary/hydrology">
		<skos:prefLabel>Hydrology</skos:prefLabel>
		<skos:definition>The science that treats the occurrence, circulation, distribution, and properties of the waters of the earth, and their reaction with the environment. (Source: MGH)</skos:definition>
		<skos:scopeNote>GEMET</skos:scopeNote>
		<skos:broader rdf:resource="http://www.earthobservations.org/GEOSS/EO_Vocabulary/surface%20water"/>
		<skos:inScheme rdf:resource="http://www.earthobservations.org/GEOSS/EO_Vocabulary"/>
	</skos:Concept>
	<skos:Concept rdf:about="http://www.earthobservations.org/GEOSS/EO_Vocabulary/methane%20concentration">
		<skos:prefLabel>Methane Concentration</skos:prefLabel>
		<skos:definition>Methane (CH4) is a greenhouse gas and is seen in polar ice cores. From the ice core record, it is known that methane rose rapidly whenever climate changed from glacial to interglacial conditions (during "deglaciation"). Warming of water bathing the seafloor could have led to large-scale release of methane from the melting of methane ice.</skos:definition>
		<skos:scopeNote>GCMD</skos:scopeNote>
		<skos:broader rdf:resource="http://www.earthobservations.org/GEOSS/EO_Vocabulary/atmospheric%20chemistry"/>
		<skos:broader rdf:resource="http://www.earthobservations.org/GEOSS/EO_Vocabulary/ice%20core%20records"/>
		<rdfs:seeAlso rdf:resource="http://sweet.jpl.nasa.gov/"/>
		<rdfs:seeAlso rdf:resource="http://stommel.tamu.edu/~baum/paleo/paleogloss/node28.html#SECTION020240000000000000000"/>
		<rdfs:seeAlso rdf:resource="http://earthobservatory.nasa.gov/Glossary/?mode=alpha&amp;seg=l&amp;segend=n"/>
		<rdfs:seeAlso rdf:resource="http://gcmd.nasa.gov/Resources/valids/archives/keyword_list.html"/>
		<rdfs:seeAlso rdf:resource="http://gcmd.nasa.gov/Resources/valids/archives/keyword_list.html"/>
		<skos:inScheme rdf:resource="http://www.earthobservations.org/GEOSS/EO_Vocabulary"/>
	</skos:Concept>
	<skos:Concept rdf:about="http://www.earthobservations.org/GEOSS/EO_Vocabulary/phenology">
		<skos:prefLabel>Phenology</skos:prefLabel>
		<skos:definition>The science that treats the periodic biological phenomena with relation to climate, especially seasonal changes. Phenological events are stages of plant growth. From a climatological viewpoint, these phenomena serve as bases for the interpretation of progress in local seasons and the climatic zones, and are considered to integrate the effects of a number of bioclimatic factors on rate of plant development. Phenology may be considered a branch of the science of bioclimatics, the sequence of plant or crop development stages through its life cycle. Growth stages may be defined by stage of physiological development such as germination, first true leaf, flowering, maturity, etc., and/or by physical stage such as planting, emergence, harvest, etc.</skos:definition>
		<skos:scopeNote>GCMD</skos:scopeNote>
		<skos:broader rdf:resource="http://www.earthobservations.org/GEOSS/EO_Vocabulary/vegetation"/>
		<skos:broader rdf:resource="http://www.earthobservations.org/GEOSS/EO_Vocabulary/vegetation"/>
		<rdfs:seeAlso rdf:resource="http://sweet.jpl.nasa.gov/"/>
		<rdfs:seeAlso rdf:resource="http://gcmd.nasa.gov/Resources/valids/archives/keyword_list.html"/>
		<skos:inScheme rdf:resource="http://www.earthobservations.org/GEOSS/EO_Vocabulary"/>
	</skos:Concept>
	<skos:Concept rdf:about="http://www.earthobservations.org/GEOSS/EO_Vocabulary/stand%20density%2Fheight%2Fvolume">
		<skos:prefLabel>Stand Density/Height/Volume</skos:prefLabel>
		<skos:definition>The mass per unit volume of a substance. Oceanographic shorthand for density, sigma-t, may be included as a Detailed Variable.</skos:definition>
		<skos:scopeNote>GCMD</skos:scopeNote>
		<skos:broader rdf:resource="http://www.earthobservations.org/GEOSS/EO_Vocabulary/vegetation"/>
		<skos:broader rdf:resource="http://www.earthobservations.org/GEOSS/EO_Vocabulary/salinity%2Fdensity"/>
		<rdfs:seeAlso rdf:resource="http://webworld.unesco.org/water/ihp/db/glossary/glu/EN/GF0304EN.HTM"/>
		<rdfs:seeAlso rdf:resource="http://gcmd.nasa.gov/Resources/valids/archives/keyword_list.html"/>
		<rdfs:seeAlso rdf:resource="http://cf-pcmdi.llnl.gov/documents/cf-standard-names/"/>
		<skos:inScheme rdf:resource="http://www.earthobservations.org/GEOSS/EO_Vocabulary"/>
	</skos:Concept>
	<skos:Concept rdf:about="http://www.earthobservations.org/GEOSS/EO_Vocabulary/suspended%20particulates%2Fturbidity%2Fwater%20attenuation%20coefficient">
		<skos:prefLabel>Suspended particulates/turbidity/water attenuation coefficient</skos:prefLabel>
		<skos:definition>Fine solids or liquid droplets suspended in the air.</skos:definition>
		<skos:scopeNote>GCMD</skos:scopeNote>
		<skos:broader rdf:resource="http://www.earthobservations.org/GEOSS/EO_Vocabulary/air%20quality"/>
		<skos:broader rdf:resource="http://www.earthobservations.org/GEOSS/EO_Vocabulary/air%20quality"/>
		<skos:broader rdf:resource="http://www.earthobservations.org/GEOSS/EO_Vocabulary/marine%20sediments"/>
		<skos:broader rdf:resource="http://www.earthobservations.org/GEOSS/EO_Vocabulary/ocean%20optics"/>
		<skos:broader rdf:resource="http://www.earthobservations.org/GEOSS/EO_Vocabulary/water%20quality%2Fwater%20chemistry"/>
		<skos:broader rdf:resource="http://www.earthobservations.org/GEOSS/EO_Vocabulary/ocean%20optics"/>
		<rdfs:seeAlso rdf:resource="http://gcmd.nasa.gov/Resources/valids/archives/keyword_list.html"/>
		<rdfs:seeAlso rdf:resource="http://sweet.jpl.nasa.gov/"/>
		<rdfs:seeAlso rdf:resource="http://his.cuahsi.org/ontologyfiles.html"/>
		<rdfs:seeAlso rdf:resource="http://gcmd.nasa.gov/Resources/valids/archives/keyword_list.html"/>
		<rdfs:seeAlso rdf:resource="http://gcmd.nasa.gov/Resources/valids/archives/keyword_list.html"/>
		<rdfs:seeAlso rdf:resource="http://gcmd.nasa.gov/Resources/valids/archives/keyword_list.html"/>
		<skos:inScheme rdf:resource="http://www.earthobservations.org/GEOSS/EO_Vocabulary"/>
	</skos:Concept>
	<skos:Concept rdf:about="http://www.earthobservations.org/GEOSS/EO_Vocabulary/ambient%20volatile%20organic%20compounds">
		<skos:prefLabel>Ambient Volatile Organic Compounds</skos:prefLabel>
		<skos:definition>Organic compounds (e.g. ethylene, propylene, benzene, styrene, acetone)which evaporate readily and contribute to air pollution directly or through chemical or photochemical reactions to produce secondary air pollutants.</skos:definition>
		<skos:scopeNote>GCMD</skos:scopeNote>
		<skos:broader rdf:resource="http://www.earthobservations.org/GEOSS/EO_Vocabulary/air%20quality"/>
		<rdfs:seeAlso rdf:resource="http://gcmd.nasa.gov/Resources/valids/archives/keyword_list.html"/>
		<skos:inScheme rdf:resource="http://www.earthobservations.org/GEOSS/EO_Vocabulary"/>
	</skos:Concept>
	<skos:Concept rdf:about="http://www.earthobservations.org/GEOSS/EO_Vocabulary/animal%20activity%20%28range%2C%20season%20length%2C%20migration%20patterns%29">
		<skos:prefLabel>Animal activity (range, season length, migration patterns)</skos:prefLabel>
		<skos:definition>A thing that a person or group does or has done</skos:definition>
		<skos:scopeNote>Oxford Dictionaries</skos:scopeNote>
		<skos:broader rdf:resource="http://www.earthobservations.org/GEOSS/EO_Vocabulary/aquatic%20ecosystems"/>
		<skos:broader rdf:resource="http://www.earthobservations.org/GEOSS/EO_Vocabulary/ecological%20dynamics"/>
		<skos:broader rdf:resource="http://www.earthobservations.org/GEOSS/EO_Vocabulary/aquatic%20ecosystems"/>
		<skos:broader rdf:resource="http://www.earthobservations.org/GEOSS/EO_Vocabulary/animals%2Fvertebrates"/>
		<skos:broader rdf:resource="http://www.earthobservations.org/GEOSS/EO_Vocabulary/animal%20science"/>
		<rdfs:seeAlso rdf:resource="http://gcmd.nasa.gov/Resources/valids/archives/keyword_list.html"/>
		<skos:inScheme rdf:resource="http://www.earthobservations.org/GEOSS/EO_Vocabulary"/>
	</skos:Concept>
	<skos:Concept rdf:about="http://www.earthobservations.org/GEOSS/EO_Vocabulary/aquatic%20ecosystem%20condition">
		<skos:prefLabel>Aquatic Ecosystem Condition</skos:prefLabel>
		<skos:definition>Any watery environment, from small to large, from pond to ocean, in which plants and animals interact with the chemical and physical features of the environment. (Source: GILP96)</skos:definition>
		<skos:scopeNote>GEMET</skos:scopeNote>
		<skos:broader rdf:resource="http://www.earthobservations.org/GEOSS/EO_Vocabulary/aquatic%20sciences"/>
		<skos:broader rdf:resource="http://www.earthobservations.org/GEOSS/EO_Vocabulary/agricultural%20aquatic%20sciences"/>
		<rdfs:seeAlso rdf:resource="http://sweet.jpl.nasa.gov/"/>
		<rdfs:seeAlso rdf:resource="http://his.cuahsi.org/ontologyfiles.html"/>
		<skos:inScheme rdf:resource="http://www.earthobservations.org/GEOSS/EO_Vocabulary"/>
	</skos:Concept>
	<skos:Concept rdf:about="http://www.earthobservations.org/GEOSS/EO_Vocabulary/ecosystem%20demand%20for%20water">
		<skos:prefLabel>Ecosystem Demand for Water</skos:prefLabel>
		<skos:definition>Liquid phase of a chemical compound consisting of approximately two parts by weight of hydrogen and 16 parts by weight of oxygen. In nature it contains small amounts of heavy water, gases and solids (mainly salts) in solution.</skos:definition>
		<skos:scopeNote>UNESCO</skos:scopeNote>
		<skos:broader rdf:resource="http://www.earthobservations.org/GEOSS/EO_Vocabulary/water%C2%A0quality%2Fwater%20chemistry"/>
		<rdfs:seeAlso rdf:resource="http://webworld.unesco.org/water/ihp/db/glossary/glu/EN/GF1353EN.HTM"/>
		<skos:inScheme rdf:resource="http://www.earthobservations.org/GEOSS/EO_Vocabulary"/>
	</skos:Concept>
	<skos:Concept rdf:about="http://www.earthobservations.org/GEOSS/EO_Vocabulary/emissivity">
		<skos:prefLabel>Emissivity</skos:prefLabel>
		<skos:definition>The ratio of the emittance of a given surface at a specified wavelength and emitting temperature to the emittance of an ideal black body at the same wavelength and temperature. Emissivity has a value between 0 (least) and one (greatest).</skos:definition>
		<skos:scopeNote>GCMD</skos:scopeNote>
		<skos:broader rdf:resource="http://www.earthobservations.org/GEOSS/EO_Vocabulary/atmospheric%20radiation"/>
		<skos:broader rdf:resource="http://www.earthobservations.org/GEOSS/EO_Vocabulary/surface%20radiative%20properties"/>
		<rdfs:seeAlso rdf:resource="http://sweet.jpl.nasa.gov/"/>
		<rdfs:seeAlso rdf:resource="http://stommel.tamu.edu/~baum/paleo/paleogloss/node13.html#SECTION02090000000000000000"/>
		<rdfs:seeAlso rdf:resource="http://gcmd.nasa.gov/Resources/valids/archives/keyword_list.html"/>
		<rdfs:seeAlso rdf:resource="http://gcmd.nasa.gov/Resources/valids/archives/keyword_list.html"/>
		<skos:inScheme rdf:resource="http://www.earthobservations.org/GEOSS/EO_Vocabulary"/>
	</skos:Concept>
	<skos:Concept rdf:about="http://www.earthobservations.org/GEOSS/EO_Vocabulary/outgoing%20longwave%20radiation%20%28top%20of%20atmosphere%20%29">
		<skos:prefLabel>Outgoing Longwave Radiation (Top of Atmosphere )</skos:prefLabel>
		<skos:definition>The outgoing longwave radiation (OLR) refers specifically to the radiation emitted by the Earth and its atmosphere (the terrestrial radiation). Satellite measurements of the OLR from terrestrial surfaces and clouds show that OLR is low over cold land and high clouds and high over hot land surface+E560s. Climate variations, such as El Nino Southern Oscillation (ENSO) can be measured from OLR anomalies from longer-term variations.</skos:definition>
		<skos:scopeNote>GCMD</skos:scopeNote>
		<skos:broader rdf:resource="http://www.earthobservations.org/GEOSS/EO_Vocabulary/atmospheric%20radiation"/>
		<rdfs:seeAlso rdf:resource="http://gcmd.nasa.gov/Resources/valids/archives/keyword_list.html"/>
		<skos:inScheme rdf:resource="http://www.earthobservations.org/GEOSS/EO_Vocabulary"/>
	</skos:Concept>
	<skos:Concept rdf:about="http://www.earthobservations.org/GEOSS/EO_Vocabulary/thermokarst">
		<skos:prefLabel>Thermokarst</skos:prefLabel>
		<skos:definition>A form of periglacial topography resembling karst, with hollows produced by the selective melting of permafrost.</skos:definition>
		<skos:scopeNote>Oxford Dictionaries</skos:scopeNote>
		<skos:broader rdf:resource="http://www.earthobservations.org/GEOSS/EO_Vocabulary/soils"/>
		<skos:broader rdf:resource="http://www.earthobservations.org/GEOSS/EO_Vocabulary/surface%20water"/>
		<rdfs:seeAlso rdf:resource="http://oxforddictionaries.com/view/entry/m_en_gb0858190#m_en_gb0858190"/>
		<skos:inScheme rdf:resource="http://www.earthobservations.org/GEOSS/EO_Vocabulary"/>
	</skos:Concept>
	<skos:Concept rdf:about="http://www.earthobservations.org/GEOSS/EO_Vocabulary/geologic%20stratification">
		<skos:prefLabel>Geologic Stratification</skos:prefLabel>
		<skos:definition>The arrangement of a body of water, as a lake, into two or more horizontal layers of different characteristics, especially densities. (Source: MGH)</skos:definition>
		<skos:scopeNote>GEMET</skos:scopeNote>
		<skos:broader rdf:resource="http://www.earthobservations.org/GEOSS/EO_Vocabulary/ecological%20dynamics"/>
		<skos:broader rdf:resource="http://www.earthobservations.org/GEOSS/EO_Vocabulary/vegetation"/>
		<rdfs:seeAlso rdf:resource="http://sweet.jpl.nasa.gov/ "/>
		<skos:inScheme rdf:resource="http://www.earthobservations.org/GEOSS/EO_Vocabulary"/>
	</skos:Concept>
	<skos:Concept rdf:about="http://www.earthobservations.org/GEOSS/EO_Vocabulary/carbon%20dioxide%20partial%20pressure">
		<skos:prefLabel>Carbon Dioxide Partial Pressure</skos:prefLabel>
		<skos:definition>A type of stress which is exerted uniformly in all directions; its measure is the force exerted per unit area. (Source: MGH) </skos:definition>
		<skos:scopeNote>GEMET</skos:scopeNote>
		<skos:broader rdf:resource="http://www.earthobservations.org/GEOSS/EO_Vocabulary/atmospheric%20chemistry"/>
		<skos:broader rdf:resource="http://www.earthobservations.org/GEOSS/EO_Vocabulary/ocean%20chemistry"/>
		<rdfs:seeAlso rdf:resource="http://cf-pcmdi.llnl.gov/documents/cf-standard-names/"/>
		<rdfs:seeAlso rdf:resource="http://cf-pcmdi.llnl.gov/documents/cf-standard-names/"/>
		<skos:inScheme rdf:resource="http://www.earthobservations.org/GEOSS/EO_Vocabulary"/>
	</skos:Concept>
	<skos:Concept rdf:about="http://www.earthobservations.org/GEOSS/EO_Vocabulary/carbon%20in%20subsurface%20ocean">
		<skos:prefLabel>Carbon in Subsurface Ocean</skos:prefLabel>
		<skos:definition>Any measure of the carbon content of the soil, in organic fractions or inorganic fractions.</skos:definition>
		<skos:scopeNote>GCMD</skos:scopeNote>
		<skos:broader rdf:resource="http://www.earthobservations.org/GEOSS/EO_Vocabulary/soils"/>
		<skos:broader rdf:resource="http://www.earthobservations.org/GEOSS/EO_Vocabulary/soils"/>
		<skos:broader rdf:resource="http://www.earthobservations.org/GEOSS/EO_Vocabulary/vegetation"/>
		<skos:broader rdf:resource="http://www.earthobservations.org/GEOSS/EO_Vocabulary/ocean%20chemistry"/>
		<rdfs:seeAlso rdf:resource="http://sweet.jpl.nasa.gov/"/>
		<rdfs:seeAlso rdf:resource="http://gcmd.nasa.gov/Resources/valids/archives/keyword_list.html"/>
		<rdfs:seeAlso rdf:resource="http://gcmd.nasa.gov/Resources/valids/archives/keyword_list.html"/>
		<rdfs:seeAlso rdf:resource="http://gcmd.nasa.gov/Resources/valids/archives/keyword_list.html"/>
		<rdfs:seeAlso rdf:resource="http://gcmd.nasa.gov/Resources/valids/archives/keyword_list.html"/>
		<skos:inScheme rdf:resource="http://www.earthobservations.org/GEOSS/EO_Vocabulary"/>
	</skos:Concept>
	<skos:Concept rdf:about="http://www.earthobservations.org/GEOSS/EO_Vocabulary/coral%20reef%20classification%2Fmetabolism">
		<skos:prefLabel>Coral Reef Classification/Metabolism</skos:prefLabel>
		<skos:definition></skos:definition>
		<skos:scopeNote>Glossary of Oceanography and the Related Geosciences with References</skos:scopeNote>
		<skos:broader rdf:resource="http://www.earthobservations.org/GEOSS/EO_Vocabulary/aquatic%20ecosystems"/>
		<rdfs:seeAlso rdf:resource="http://stommel.tamu.edu/~baum/paleo/paleogloss/node10.html#SECTION02060000000000000000"/>
		<skos:inScheme rdf:resource="http://www.earthobservations.org/GEOSS/EO_Vocabulary"/>
	</skos:Concept>
	<skos:Concept rdf:about="http://www.earthobservations.org/GEOSS/EO_Vocabulary/crop%20emergence">
		<skos:prefLabel>Crop Emergence</skos:prefLabel>
		<skos:definition>N/A</skos:definition>
		<skos:scopeNote>SWEET 2.0</skos:scopeNote>
		<skos:broader rdf:resource="http://www.earthobservations.org/GEOSS/EO_Vocabulary/agricultural%20plant%20science"/>
		<skos:broader rdf:resource="http://www.earthobservations.org/GEOSS/EO_Vocabulary/plant%20commodities"/>
		<skos:broader rdf:resource="http://www.earthobservations.org/GEOSS/EO_Vocabulary/ecological%20dynamics"/>
		<skos:broader rdf:resource="http://www.earthobservations.org/GEOSS/EO_Vocabulary/agricultural%20plant%20science"/>
		<rdfs:seeAlso rdf:resource="http://sweet.jpl.nasa.gov/"/>
		<rdfs:seeAlso rdf:resource="http://gcmd.nasa.gov/Resources/valids/archives/keyword_list.html"/>
		<skos:inScheme rdf:resource="http://www.earthobservations.org/GEOSS/EO_Vocabulary"/>
	</skos:Concept>
	<skos:Concept rdf:about="http://www.earthobservations.org/GEOSS/EO_Vocabulary/crop%20yield">
		<skos:prefLabel>Crop Yield</skos:prefLabel>
		<skos:definition>The quantity of plant materials resulting from cultivation or growth. Includes all comercial crops, as well as plant biomass yields (i.e. amount of grass produced per unit land in natural agroecosystems (e.g. rangeland)). Does not include PRODUCT yield (e.g. bushels of wheat vs. lbs. flour).</skos:definition>
		<skos:scopeNote>GCMD</skos:scopeNote>
		<skos:broader rdf:resource="http://www.earthobservations.org/GEOSS/EO_Vocabulary/agricultural%20plant%20science"/>
		<rdfs:seeAlso rdf:resource="http://gcmd.nasa.gov/Resources/valids/archives/keyword_list.html"/>
		<skos:inScheme rdf:resource="http://www.earthobservations.org/GEOSS/EO_Vocabulary"/>
	</skos:Concept>
	<skos:Concept rdf:about="http://www.earthobservations.org/GEOSS/EO_Vocabulary/density%20of%20animal%20hosts">
		<skos:prefLabel>Density of Animal hosts</skos:prefLabel>
		<skos:definition>The mass per unit volume of a substance. Oceanographic shorthand for density, sigma-t, may be included as a Detailed Variable.</skos:definition>
		<skos:scopeNote>GCMD</skos:scopeNote>
		<skos:broader rdf:resource="http://www.earthobservations.org/GEOSS/EO_Vocabulary/salinity%2Fdensity"/>
		<skos:broader rdf:resource="http://www.earthobservations.org/GEOSS/EO_Vocabulary/human%20health"/>
		<rdfs:seeAlso rdf:resource="http://webworld.unesco.org/water/ihp/db/glossary/glu/EN/GF0304EN.HTM"/>
		<rdfs:seeAlso rdf:resource="http://gcmd.nasa.gov/Resources/valids/archives/keyword_list.html"/>
		<skos:inScheme rdf:resource="http://www.earthobservations.org/GEOSS/EO_Vocabulary"/>
	</skos:Concept>
	<skos:Concept rdf:about="http://www.earthobservations.org/GEOSS/EO_Vocabulary/field%20cover%20%28continuous%29">
		<skos:prefLabel>Field Cover (Continuous)</skos:prefLabel>
		<skos:definition>N/A</skos:definition>
		<skos:scopeNote>SWEET 2.0 </skos:scopeNote>
		<skos:broader rdf:resource="http://www.earthobservations.org/GEOSS/EO_Vocabulary/land%20use%2Fland%C2%A0cover"/>
		<skos:broader rdf:resource="http://www.earthobservations.org/GEOSS/EO_Vocabulary/land%20use%2Fland%20cover"/>
		<rdfs:seeAlso rdf:resource="http://sweet.jpl.nasa.gov/"/>
		<rdfs:seeAlso rdf:resource="http://dias.csis.u-tokyo.ac.jp/dict/inspire/index.php/Land_cover"/>
		<rdfs:seeAlso rdf:resource="http://earthobservatory.nasa.gov/Glossary/?mode=alpha&amp;seg=l&amp;segend=n"/>
		<skos:inScheme rdf:resource="http://www.earthobservations.org/GEOSS/EO_Vocabulary"/>
	</skos:Concept>
	<skos:Concept rdf:about="http://www.earthobservations.org/GEOSS/EO_Vocabulary/gravity%20field">
		<skos:prefLabel>Gravity Field</skos:prefLabel>
		<skos:definition>Pertaining to the measurement, strength, size, etc. of the Earth's gravitational field.</skos:definition>
		<skos:scopeNote>GCMD</skos:scopeNote>
		<skos:broader rdf:resource="http://www.earthobservations.org/GEOSS/EO_Vocabulary/geodetics%2Fgravity"/>
		<skos:broader rdf:resource="http://www.earthobservations.org/GEOSS/EO_Vocabulary/geodetics%2Fgravity"/>
		<skos:broader rdf:resource="http://www.earthobservations.org/GEOSS/EO_Vocabulary/marine%20geophysics"/>
		<rdfs:seeAlso rdf:resource="http://gcmd.nasa.gov/Resources/valids/archives/keyword_list.html "/>
		<rdfs:seeAlso rdf:resource="http://gcmd.nasa.gov/Resources/valids/archives/keyword_list.html"/>
		<rdfs:seeAlso rdf:resource="http://gcmd.nasa.gov/Resources/valids/archives/keyword_list.html"/>
		<skos:inScheme rdf:resource="http://www.earthobservations.org/GEOSS/EO_Vocabulary"/>
	</skos:Concept>
	<skos:Concept rdf:about="http://www.earthobservations.org/GEOSS/EO_Vocabulary/health%20care%20access">
		<skos:prefLabel>Health Care Access</skos:prefLabel>
		<skos:definition>The means or opportunity to approach or enter a place</skos:definition>
		<skos:scopeNote>Oxford Dictionaries</skos:scopeNote>
		<skos:broader rdf:resource="http://www.earthobservations.org/GEOSS/EO_Vocabulary/attitudes%2Cpreferences%2Cbehavior"/>
		<skos:broader rdf:resource="http://www.earthobservations.org/GEOSS/EO_Vocabulary/human%20health"/>
		<rdfs:seeAlso rdf:resource="http://oxforddictionaries.com/view/entry/m_en_gb0003710#m_en_gb0003710"/>
		<skos:inScheme rdf:resource="http://www.earthobservations.org/GEOSS/EO_Vocabulary"/>
	</skos:Concept>
	<skos:Concept rdf:about="http://www.earthobservations.org/GEOSS/EO_Vocabulary/inundated%20vegetation">
		<skos:prefLabel>Inundated vegetation</skos:prefLabel>
		<skos:definition>Vegetation, as used, here are types of plants and vegetation structures.</skos:definition>
		<skos:scopeNote>GCMD</skos:scopeNote>
		<skos:broader rdf:resource="http://www.earthobservations.org/GEOSS/EO_Vocabulary/vegetation"/>
		<rdfs:seeAlso rdf:resource="http://his.cuahsi.org/ontologyfiles.html"/>
		<rdfs:seeAlso rdf:resource="http://gcmd.nasa.gov/Resources/valids/archives/keyword_list.html"/>
		<skos:inScheme rdf:resource="http://www.earthobservations.org/GEOSS/EO_Vocabulary"/>
	</skos:Concept>
	<skos:Concept rdf:about="http://www.earthobservations.org/GEOSS/EO_Vocabulary/magnetic%20field">
		<skos:prefLabel>Magnetic Field</skos:prefLabel>
		<skos:definition>Pertaining to the magnetic field generated by the Earth, consisting of both the dipole and non-dipole components.</skos:definition>
		<skos:scopeNote>GCMD</skos:scopeNote>
		<skos:broader rdf:resource="http://www.earthobservations.org/GEOSS/EO_Vocabulary/geomagnetism"/>
		<rdfs:seeAlso rdf:resource="http://gcmd.nasa.gov/Resources/valids/archives/keyword_list.html"/>
		<skos:inScheme rdf:resource="http://www.earthobservations.org/GEOSS/EO_Vocabulary"/>
	</skos:Concept>
	<skos:Concept rdf:about="http://www.earthobservations.org/GEOSS/EO_Vocabulary/other%20long-lived%20ghgs">
		<skos:prefLabel>Other long-lived GHGs</skos:prefLabel>
		<skos:definition>A gaseous component of the atmosphere contributing to the greenhouse effect. Greenhouse gases are transparent to certain wavelengths of the sun's radiant energy, allowing them to penetrate deep into the atmosphere or all the way into the Earth's surface. Greenhouse gases and clouds prevent some of infrared radiation from escaping, trapping the heat near the Earth's surface where it warms the lower atmosphere. Alteration of this natural barrier of atmospheric gases can raise or lower the mean global temperature of the Earth. Greenhouse gases include carbon dioxide, methane, nitrous oxide, chlorofluorocarbons, and water vapor. Carbon dioxide, methane, and nitrous oxide have significant natural and human sources while only industries produce chlorofluorocarbons. Water vapor has the largest greenhouse effect, but its concentration in the troposphere is determined within the climate system. Water vapor will increase in response to global warming, which in turn may further enhance global warming.</skos:definition>
		<skos:scopeNote>NASA</skos:scopeNote>
		<skos:broader rdf:resource="http://www.earthobservations.org/GEOSS/EO_Vocabulary/air%20quality"/>
		<rdfs:seeAlso rdf:resource="http://stommel.tamu.edu/~baum/paleo/paleogloss/node18.html#SECTION020140000000000000000"/>
		<rdfs:seeAlso rdf:resource="http://earthobservatory.nasa.gov/Glossary/index.php?mode=alpha&amp;seg=f&amp;segend=h"/>
		<skos:inScheme rdf:resource="http://www.earthobservations.org/GEOSS/EO_Vocabulary"/>
	</skos:Concept>
	<skos:Concept rdf:about="http://www.earthobservations.org/GEOSS/EO_Vocabulary/pathogen%20population%20dynamic">
		<skos:prefLabel>Pathogen Population Dynamic</skos:prefLabel>
		<skos:definition>Population dynamics is the study of the reasons for changes in population size.</skos:definition>
		<skos:scopeNote>GCMD</skos:scopeNote>
		<skos:broader rdf:resource="http://www.earthobservations.org/GEOSS/EO_Vocabulary/ecological%20dynamics"/>
		<skos:broader rdf:resource="http://www.earthobservations.org/GEOSS/EO_Vocabulary/human%20health"/>
		<rdfs:seeAlso rdf:resource="http://gcmd.nasa.gov/Resources/valids/archives/keyword_list.html"/>
		<skos:inScheme rdf:resource="http://www.earthobservations.org/GEOSS/EO_Vocabulary"/>
	</skos:Concept>
	<skos:Concept rdf:about="http://www.earthobservations.org/GEOSS/EO_Vocabulary/sea%20ice%20surface%20%28skin%29%20temperature">
		<skos:prefLabel>Sea Ice Surface (Skin) Temperature</skos:prefLabel>
		<skos:definition>The surface temperature is the (skin) temperature at the interface, not the bulk temperature of the medium above or below. "Sea ice surface temperature" is the temperature that exists at the interface of sea ice and an overlying medium which may be air or snow. In areas of snow covered sea ice, sea_ice_surface_temperature is not the same as the quantity with standard name surface_temperature. K</skos:definition>
		<skos:scopeNote>CF Standard</skos:scopeNote>
		<skos:broader rdf:resource="http://www.earthobservations.org/GEOSS/EO_Vocabulary/atmospheric%20temperature"/>
		<skos:broader rdf:resource="http://www.earthobservations.org/GEOSS/EO_Vocabulary/land%20temperature"/>
		<rdfs:seeAlso rdf:resource="http://cf-pcmdi.llnl.gov/documents/cf-standard-names/"/>
		<rdfs:seeAlso rdf:resource="http://gcmd.nasa.gov/Resources/valids/archives/keyword_list.html"/>
		<skos:inScheme rdf:resource="http://www.earthobservations.org/GEOSS/EO_Vocabulary"/>
	</skos:Concept>
	<skos:Concept rdf:about="http://www.earthobservations.org/GEOSS/EO_Vocabulary/soil%20thaw">
		<skos:prefLabel>Soil Thaw</skos:prefLabel>
		<skos:definition>Melting of snow and ice at the earth's surface, following a temperature rise above 0°C.</skos:definition>
		<skos:scopeNote>UNESCO</skos:scopeNote>
		<skos:broader rdf:resource="http://www.earthobservations.org/GEOSS/EO_Vocabulary/atmospheric%20temperature"/>
		<skos:broader rdf:resource="http://www.earthobservations.org/GEOSS/EO_Vocabulary/snow%2Fice"/>
		<rdfs:seeAlso rdf:resource="http://sweet.jpl.nasa.gov/"/>
		<rdfs:seeAlso rdf:resource="http://webworld.unesco.org/water/ihp/db/glossary/glu/EN/GF1269EN.HTM"/>
		<skos:inScheme rdf:resource="http://www.earthobservations.org/GEOSS/EO_Vocabulary"/>
	</skos:Concept>
	<skos:Concept rdf:about="http://www.earthobservations.org/GEOSS/EO_Vocabulary/stratospheric%20ozone">
		<skos:prefLabel>Stratospheric Ozone</skos:prefLabel>
		<skos:definition>Ozone (O3) is a molecule that consists of three oxygen atoms bonded together. The ozone layer in the stratosphere absorbs UV radiation and creates a warm layer of air high in the stratosphere. Ozone that is present in the troposphere is mostly a result of anthropogenic pollution and therefore higher concentrations are found in urban areas. Ozone is involved with NOx in the photochemical production of many of the constituents of pollution environments (see nitrogen oxides and hydroxyl definitions) [Chemical and Engineering News; v72; 6-7; 1994.] [Aviation Week and Space Technology; v140; 20-21; 1994.]</skos:definition>
		<skos:scopeNote>GCMD</skos:scopeNote>
		<skos:broader rdf:resource="http://www.earthobservations.org/GEOSS/EO_Vocabulary/atmospheric%20chemistry"/>
		<rdfs:seeAlso rdf:resource="http://sweet.jpl.nasa.gov/"/>
		<rdfs:seeAlso rdf:resource="http://stommel.tamu.edu/~baum/paleo/paleogloss/node33.html#SECTION020290000000000000000"/>
		<rdfs:seeAlso rdf:resource="http://earthobservatory.nasa.gov/Glossary/?mode=alpha&amp;seg=o"/>
		<rdfs:seeAlso rdf:resource="http://gcmd.nasa.gov/Resources/valids/archives/keyword_list.html"/>
		<skos:inScheme rdf:resource="http://www.earthobservations.org/GEOSS/EO_Vocabulary"/>
	</skos:Concept>
	<skos:Concept rdf:about="http://www.earthobservations.org/GEOSS/EO_Vocabulary/water%20algal%20blooms">
		<skos:prefLabel>Water Algal Blooms</skos:prefLabel>
		<skos:definition>Excessive and rapid growth of algae and other aquatic plants when they are stimulated to grow too quickly by pollution. It takes place when there are too many nutrients in the water and is aggravated when accompanied by a rise in temperature. Although the algae grow quickly they soon die because they have swallowed up all the water's nutrients. As they decompose they tend to rise to the surface and form a green slime. Algal bloom have increased because higher levels of nitrogen and phosphates from agricultural areas have leached from the fields into water courses. (Source: WRIGHT)</skos:definition>
		<skos:scopeNote>GEMET</skos:scopeNote>
		<skos:broader rdf:resource="http://www.earthobservations.org/GEOSS/EO_Vocabulary/bacteria%2Farchaea"/>
		<skos:broader rdf:resource="http://www.earthobservations.org/GEOSS/EO_Vocabulary/plants"/>
		<rdfs:seeAlso rdf:resource="http://webworld.unesco.org/water/ihp/db/glossary/glu/EN/GF0036EN.HTM"/>
		<rdfs:seeAlso rdf:resource="http://webworld.unesco.org/water/ihp/db/glossary/glu/EN/GF0036EN.HTM"/>
		<skos:inScheme rdf:resource="http://www.earthobservations.org/GEOSS/EO_Vocabulary"/>
	</skos:Concept>
	<skos:Concept rdf:about="http://www.earthobservations.org/GEOSS/EO_Vocabulary/water%20infiltration%2Fpercolation-land%20surface">
		<skos:prefLabel>Water Infiltration/Percolation-Land Surface</skos:prefLabel>
		<skos:definition> Pertaining to the process by which substances enter an aquifer.</skos:definition>
		<skos:scopeNote>GCMD</skos:scopeNote>
		<skos:broader rdf:resource="http://www.earthobservations.org/GEOSS/EO_Vocabulary/ground%20water"/>
		<skos:broader rdf:resource="http://www.earthobservations.org/GEOSS/EO_Vocabulary/ground%20water"/>
		<rdfs:seeAlso rdf:resource="http://sweet.jpl.nasa.gov/"/>
		<rdfs:seeAlso rdf:resource="http://webworld.unesco.org/water/ihp/db/glossary/glu/EN/GF0664EN.HTM"/>
		<rdfs:seeAlso rdf:resource="http://gcmd.nasa.gov/Resources/valids/archives/keyword_list.html"/>
		<skos:inScheme rdf:resource="http://www.earthobservations.org/GEOSS/EO_Vocabulary"/>
	</skos:Concept>
</rdf:RDF>